Source/Dafny/Parser.cs
@@ -22,13 +22,17 @@ public class Parser {
 	public const int _string = 6;
 	public const int _colon = 7;
 	public const int _semi = 8;
-	public const int _lbrace = 9;
-	public const int _rbrace = 10;
-	public const int _openparen = 11;
-	public const int _closeparen = 12;
-	public const int _star = 13;
-	public const int _notIn = 14;
-	public const int maxT = 126;
+	public const int _darrow = 9;
+	public const int _arrow = 10;
+	public const int _reads = 11;
+	public const int _requires = 12;
+	public const int _lbrace = 13;
+	public const int _rbrace = 14;
+	public const int _openparen = 15;
+	public const int _closeparen = 16;
+	public const int _star = 17;
+	public const int _notIn = 18;
+	public const int maxT = 127;
 
 	const bool T = true;
 	const bool x = false;
@@ -147,6 +151,13 @@ bool IsParenStar() {
   return la.kind == _openparen && x.kind == _star;
 }
 
+bool IsLambda(bool allowLambda)
+{
+  return allowLambda &&
+    (la.kind == _darrow || la.kind == _arrow
+    || la.kind == _reads || la.kind == _requires);
+}
+
 bool IsIdentParen() {
   Token x = scanner.Peek();
   return la.kind == _ident && x.kind == _openparen;
@@ -154,7 +165,7 @@ bool IsIdentParen() {
 
 bool SemiFollowsCall(bool allowSemi, Expression e) {
   return allowSemi && la.kind == _semi &&
-    (e is FunctionCallExpr ||
+    (e is FunctionCallExpr || e is ApplyExpr ||
      (e is IdentifierSequence && ((IdentifierSequence)e).OpenParen != null));
 }
 
@@ -165,6 +176,7 @@ bool CloseOptionalParen(bool usesOptionalParen) {
 bool CloseOptionalBrace(bool usesOptionalBrace) {
   return usesOptionalBrace && la.kind == _rbrace;
 }
+
 /*--------------------------------------------------------------------------*/
 
 
@@ -245,7 +257,7 @@ bool CloseOptionalBrace(bool usesOptionalBrace) {
 		// theModule should be a DefaultModuleDecl (actually, the singular DefaultModuleDecl)
 		Contract.Assert(defaultModule != null);
 		
-		while (la.kind == 15) {
+		while (la.kind == 19) {
 			Get();
 			Expect(6);
 			{
@@ -263,32 +275,32 @@ bool CloseOptionalBrace(bool usesOptionalBrace) {
 		}
 		while (StartOf(1)) {
 			switch (la.kind) {
-			case 16: case 17: case 19: {
+			case 20: case 21: case 23: {
 				SubModuleDecl(defaultModule, out submodule);
 				defaultModule.TopLevelDecls.Add(submodule); 
 				break;
 			}
-			case 24: {
+			case 28: {
 				ClassDecl(defaultModule, out c);
 				defaultModule.TopLevelDecls.Add(c); 
 				break;
 			}
-			case 27: case 28: {
+			case 31: case 32: {
 				DatatypeDecl(defaultModule, out dt);
 				defaultModule.TopLevelDecls.Add(dt); 
 				break;
 			}
-			case 32: {
+			case 36: {
 				OtherTypeDecl(defaultModule, out td);
 				defaultModule.TopLevelDecls.Add(td); 
 				break;
 			}
-			case 34: {
+			case 38: {
 				IteratorDecl(defaultModule, out iter);
 				defaultModule.TopLevelDecls.Add(iter); 
 				break;
 			}
-			case 25: case 26: case 30: case 40: case 41: case 42: case 43: case 44: case 62: case 63: case 64: {
+			case 29: case 30: case 34: case 44: case 45: case 46: case 47: case 48: case 64: case 65: case 66: {
 				ClassMemberDecl(membersDefaultClass, false);
 				break;
 			}
@@ -320,76 +332,76 @@ bool CloseOptionalBrace(bool usesOptionalBrace) {
 		bool isAbstract = false;
 		bool opened = false;
 		
-		if (la.kind == 16 || la.kind == 17) {
-			if (la.kind == 16) {
+		if (la.kind == 20 || la.kind == 21) {
+			if (la.kind == 20) {
 				Get();
 				isAbstract = true; 
 			}
-			Expect(17);
-			while (la.kind == 9) {
+			Expect(21);
+			while (la.kind == 13) {
 				Attribute(ref attrs);
 			}
 			NoUSIdent(out id);
-			if (la.kind == 18) {
+			if (la.kind == 22) {
 				Get();
 				QualifiedName(out idRefined);
 			}
 			module = new ModuleDefinition(id, id.val, isAbstract, false, idRefined == null ? null : idRefined, parent, attrs, false); 
-			Expect(9);
+			Expect(13);
 			module.BodyStartTok = t; 
 			while (StartOf(1)) {
 				switch (la.kind) {
-				case 16: case 17: case 19: {
+				case 20: case 21: case 23: {
 					SubModuleDecl(module, out sm);
 					module.TopLevelDecls.Add(sm); 
 					break;
 				}
-				case 24: {
+				case 28: {
 					ClassDecl(module, out c);
 					module.TopLevelDecls.Add(c); 
 					break;
 				}
-				case 27: case 28: {
+				case 31: case 32: {
 					DatatypeDecl(module, out dt);
 					module.TopLevelDecls.Add(dt); 
 					break;
 				}
-				case 32: {
+				case 36: {
 					OtherTypeDecl(module, out td);
 					module.TopLevelDecls.Add(td); 
 					break;
 				}
-				case 34: {
+				case 38: {
 					IteratorDecl(module, out iter);
 					module.TopLevelDecls.Add(iter); 
 					break;
 				}
-				case 25: case 26: case 30: case 40: case 41: case 42: case 43: case 44: case 62: case 63: case 64: {
+				case 29: case 30: case 34: case 44: case 45: case 46: case 47: case 48: case 64: case 65: case 66: {
 					ClassMemberDecl(namedModuleDefaultClassMembers, false);
 					break;
 				}
 				}
 			}
-			Expect(10);
+			Expect(14);
 			module.BodyEndTok = t;
 			module.TopLevelDecls.Add(new DefaultClassDecl(module, namedModuleDefaultClassMembers));
 			submodule = new LiteralModuleDecl(module, parent); 
-		} else if (la.kind == 19) {
+		} else if (la.kind == 23) {
 			Get();
-			if (la.kind == 20) {
+			if (la.kind == 24) {
 				Get();
 				opened = true;
 			}
 			NoUSIdent(out id);
-			if (la.kind == 21 || la.kind == 22) {
-				if (la.kind == 21) {
+			if (la.kind == 25 || la.kind == 26) {
+				if (la.kind == 25) {
 					Get();
 					QualifiedName(out idPath);
 					submodule = new AliasModuleDecl(idPath, id, parent, opened); 
 				} else {
 					Get();
 					QualifiedName(out idPath);
-					if (la.kind == 23) {
+					if (la.kind == 27) {
 						Get();
 						QualifiedName(out idAssignment);
 					}
@@ -397,7 +409,7 @@ bool CloseOptionalBrace(bool usesOptionalBrace) {
 				}
 			}
 			if (la.kind == 8) {
-				while (!(la.kind == 0 || la.kind == 8)) {SynErr(127); Get();}
+				while (!(la.kind == 0 || la.kind == 8)) {SynErr(128); Get();}
 				Get();
 			}
 			if (submodule == null) {
@@ -406,7 +418,7 @@ bool CloseOptionalBrace(bool usesOptionalBrace) {
 			 submodule = new AliasModuleDecl(idPath, id, parent, opened);
 			}
 			
-		} else SynErr(128);
+		} else SynErr(129);
 	}
 
 	void ClassDecl(ModuleDefinition/*!*/ module, out ClassDecl/*!*/ c) {
@@ -418,21 +430,21 @@ bool CloseOptionalBrace(bool usesOptionalBrace) {
 		List<MemberDecl/*!*/> members = new List<MemberDecl/*!*/>();
 		IToken bodyStart;
 		
-		while (!(la.kind == 0 || la.kind == 24)) {SynErr(129); Get();}
-		Expect(24);
-		while (la.kind == 9) {
+		while (!(la.kind == 0 || la.kind == 28)) {SynErr(130); Get();}
+		Expect(28);
+		while (la.kind == 13) {
 			Attribute(ref attrs);
 		}
 		NoUSIdent(out id);
-		if (la.kind == 38) {
+		if (la.kind == 42) {
 			GenericParameters(typeArgs);
 		}
-		Expect(9);
+		Expect(13);
 		bodyStart = t; 
 		while (StartOf(2)) {
 			ClassMemberDecl(members, true);
 		}
-		Expect(10);
+		Expect(14);
 		c = new ClassDecl(id, id.val, module, typeArgs, members, attrs);
 		c.BodyStartTok = bodyStart;
 		c.BodyEndTok = t;
@@ -449,29 +461,29 @@ bool CloseOptionalBrace(bool usesOptionalBrace) {
 		IToken bodyStart = Token.NoToken;  // dummy assignment
 		bool co = false;
 		
-		while (!(la.kind == 0 || la.kind == 27 || la.kind == 28)) {SynErr(130); Get();}
-		if (la.kind == 27) {
+		while (!(la.kind == 0 || la.kind == 31 || la.kind == 32)) {SynErr(131); Get();}
+		if (la.kind == 31) {
 			Get();
-		} else if (la.kind == 28) {
+		} else if (la.kind == 32) {
 			Get();
 			co = true; 
-		} else SynErr(131);
-		while (la.kind == 9) {
+		} else SynErr(132);
+		while (la.kind == 13) {
 			Attribute(ref attrs);
 		}
 		NoUSIdent(out id);
-		if (la.kind == 38) {
+		if (la.kind == 42) {
 			GenericParameters(typeArgs);
 		}
-		Expect(21);
+		Expect(25);
 		bodyStart = t; 
 		DatatypeMemberDecl(ctors);
-		while (la.kind == 29) {
+		while (la.kind == 33) {
 			Get();
 			DatatypeMemberDecl(ctors);
 		}
 		if (la.kind == 8) {
-			while (!(la.kind == 0 || la.kind == 8)) {SynErr(132); Get();}
+			while (!(la.kind == 0 || la.kind == 8)) {SynErr(133); Get();}
 			Get();
 		}
 		if (co) {
@@ -492,35 +504,35 @@ bool CloseOptionalBrace(bool usesOptionalBrace) {
 		td = null;
 		Type ty;
 		
-		Expect(32);
-		while (la.kind == 9) {
+		Expect(36);
+		while (la.kind == 13) {
 			Attribute(ref attrs);
 		}
 		NoUSIdent(out id);
-		if (la.kind == 11) {
+		if (la.kind == 15) {
 			Get();
-			Expect(33);
-			Expect(12);
+			Expect(37);
+			Expect(16);
 			eqSupport = TypeParameter.EqualitySupportValue.Required; 
-			if (la.kind == 38) {
+			if (la.kind == 42) {
 				GenericParameters(typeArgs);
 			}
 		} else if (StartOf(3)) {
-			if (la.kind == 38) {
+			if (la.kind == 42) {
 				GenericParameters(typeArgs);
 			}
-			if (la.kind == 21) {
+			if (la.kind == 25) {
 				Get();
 				Type(out ty);
 				td = new TypeSynonymDecl(id, id.val, typeArgs, module, ty, attrs); 
 			}
-		} else SynErr(133);
+		} else SynErr(134);
 		if (td == null) {
 		 td = new OpaqueTypeDecl(id, id.val, module, eqSupport, typeArgs, attrs);
 		}
 		
 		if (la.kind == 8) {
-			while (!(la.kind == 0 || la.kind == 8)) {SynErr(134); Get();}
+			while (!(la.kind == 0 || la.kind == 8)) {SynErr(135); Get();}
 			Get();
 		}
 	}
@@ -549,19 +561,19 @@ bool CloseOptionalBrace(bool usesOptionalBrace) {
 		IToken bodyStart = Token.NoToken;
 		IToken bodyEnd = Token.NoToken;
 		
-		while (!(la.kind == 0 || la.kind == 34)) {SynErr(135); Get();}
-		Expect(34);
-		while (la.kind == 9) {
+		while (!(la.kind == 0 || la.kind == 38)) {SynErr(136); Get();}
+		Expect(38);
+		while (la.kind == 13) {
 			Attribute(ref attrs);
 		}
 		NoUSIdent(out id);
-		if (la.kind == 11 || la.kind == 38) {
-			if (la.kind == 38) {
+		if (la.kind == 15 || la.kind == 42) {
+			if (la.kind == 42) {
 				GenericParameters(typeArgs);
 			}
 			Formals(true, true, ins, out openParen);
-			if (la.kind == 35 || la.kind == 36) {
-				if (la.kind == 35) {
+			if (la.kind == 39 || la.kind == 40) {
+				if (la.kind == 39) {
 					Get();
 				} else {
 					Get();
@@ -569,14 +581,14 @@ bool CloseOptionalBrace(bool usesOptionalBrace) {
 				}
 				Formals(false, true, outs, out openParen);
 			}
-		} else if (la.kind == 37) {
+		} else if (la.kind == 41) {
 			Get();
 			signatureEllipsis = t; openParen = Token.NoToken; 
-		} else SynErr(136);
+		} else SynErr(137);
 		while (StartOf(4)) {
 			IteratorSpec(reads, mod, decreases, req, ens, yieldReq, yieldEns, ref readsAttrs, ref modAttrs, ref decrAttrs);
 		}
-		if (la.kind == 9) {
+		if (la.kind == 13) {
 			BlockStmt(out body, out bodyStart, out bodyEnd);
 		}
 		iter = new IteratorDecl(id, id.val, module, typeArgs, ins, outs,
@@ -596,8 +608,8 @@ bool CloseOptionalBrace(bool usesOptionalBrace) {
 		Function/*!*/ f;
 		MemberModifiers mmod = new MemberModifiers();
 		
-		while (la.kind == 25 || la.kind == 26) {
-			if (la.kind == 25) {
+		while (la.kind == 29 || la.kind == 30) {
+			if (la.kind == 29) {
 				Get();
 				mmod.IsGhost = true; 
 			} else {
@@ -605,21 +617,21 @@ bool CloseOptionalBrace(bool usesOptionalBrace) {
 				mmod.IsStatic = true; 
 			}
 		}
-		if (la.kind == 30) {
+		if (la.kind == 34) {
 			FieldDecl(mmod, mm);
-		} else if (la.kind == 62 || la.kind == 63 || la.kind == 64) {
+		} else if (la.kind == 64 || la.kind == 65 || la.kind == 66) {
 			FunctionDecl(mmod, out f);
 			mm.Add(f); 
 		} else if (StartOf(5)) {
 			MethodDecl(mmod, allowConstructors, out m);
 			mm.Add(m); 
-		} else SynErr(137);
+		} else SynErr(138);
 	}
 
 	void Attribute(ref Attributes attrs) {
-		Expect(9);
+		Expect(13);
 		AttributeBody(ref attrs);
-		Expect(10);
+		Expect(14);
 	}
 
 	void NoUSIdent(out IToken/*!*/ x) {
@@ -636,7 +648,7 @@ bool CloseOptionalBrace(bool usesOptionalBrace) {
 		IToken id; IToken idPrime; ids = new List<IToken>(); 
 		Ident(out id);
 		ids.Add(id); 
-		while (la.kind == 61) {
+		while (la.kind == 63) {
 			IdentOrDigitsSuffix(out id, out idPrime);
 			ids.Add(id);
 			if (idPrime != null) { ids.Add(idPrime); }
@@ -655,7 +667,7 @@ bool CloseOptionalBrace(bool usesOptionalBrace) {
 		x = Token.NoToken;
 		y = null;
 		
-		Expect(61);
+		Expect(63);
 		if (la.kind == 1) {
 			Get();
 			x = t; 
@@ -683,7 +695,13 @@ bool CloseOptionalBrace(bool usesOptionalBrace) {
 			 }
 			}
 			
-		} else SynErr(138);
+		} else if (la.kind == 12) {
+			Get();
+			x = t; 
+		} else if (la.kind == 11) {
+			Get();
+			x = t; 
+		} else SynErr(139);
 	}
 
 	void GenericParameters(List<TypeParameter/*!*/>/*!*/ typeArgs) {
@@ -691,29 +709,29 @@ bool CloseOptionalBrace(bool usesOptionalBrace) {
 		IToken/*!*/ id;
 		TypeParameter.EqualitySupportValue eqSupport;
 		
-		Expect(38);
+		Expect(42);
 		NoUSIdent(out id);
 		eqSupport = TypeParameter.EqualitySupportValue.Unspecified; 
-		if (la.kind == 11) {
+		if (la.kind == 15) {
 			Get();
-			Expect(33);
-			Expect(12);
+			Expect(37);
+			Expect(16);
 			eqSupport = TypeParameter.EqualitySupportValue.Required; 
 		}
 		typeArgs.Add(new TypeParameter(id, id.val, eqSupport)); 
-		while (la.kind == 31) {
+		while (la.kind == 35) {
 			Get();
 			NoUSIdent(out id);
 			eqSupport = TypeParameter.EqualitySupportValue.Unspecified; 
-			if (la.kind == 11) {
+			if (la.kind == 15) {
 				Get();
-				Expect(33);
-				Expect(12);
+				Expect(37);
+				Expect(16);
 				eqSupport = TypeParameter.EqualitySupportValue.Required; 
 			}
 			typeArgs.Add(new TypeParameter(id, id.val, eqSupport)); 
 		}
-		Expect(39);
+		Expect(43);
 	}
 
 	void FieldDecl(MemberModifiers mmod, List<MemberDecl/*!*/>/*!*/ mm) {
@@ -721,21 +739,21 @@ bool CloseOptionalBrace(bool usesOptionalBrace) {
 		Attributes attrs = null;
 		IToken/*!*/ id;  Type/*!*/ ty;
 		
-		while (!(la.kind == 0 || la.kind == 30)) {SynErr(139); Get();}
-		Expect(30);
+		while (!(la.kind == 0 || la.kind == 34)) {SynErr(140); Get();}
+		Expect(34);
 		if (mmod.IsStatic) { SemErr(t, "fields cannot be declared 'static'"); }
 		
-		while (la.kind == 9) {
+		while (la.kind == 13) {
 			Attribute(ref attrs);
 		}
 		FIdentType(out id, out ty);
 		mm.Add(new Field(id, id.val, mmod.IsGhost, ty, attrs)); 
-		while (la.kind == 31) {
+		while (la.kind == 35) {
 			Get();
 			FIdentType(out id, out ty);
 			mm.Add(new Field(id, id.val, mmod.IsGhost, ty, attrs)); 
 		}
-		while (!(la.kind == 0 || la.kind == 8)) {SynErr(140); Get();}
+		while (!(la.kind == 0 || la.kind == 8)) {SynErr(141); Get();}
 		Expect(8);
 	}
 
@@ -758,90 +776,90 @@ bool CloseOptionalBrace(bool usesOptionalBrace) {
 		IToken bodyEnd = Token.NoToken;
 		IToken signatureEllipsis = null;
 		
-		if (la.kind == 62) {
+		if (la.kind == 64) {
 			Get();
-			if (la.kind == 40) {
+			if (la.kind == 44) {
 				Get();
 				isFunctionMethod = true; 
 			}
 			if (mmod.IsGhost) { SemErr(t, "functions cannot be declared 'ghost' (they are ghost by default)"); }
 			
-			while (la.kind == 9) {
+			while (la.kind == 13) {
 				Attribute(ref attrs);
 			}
 			NoUSIdent(out id);
-			if (la.kind == 11 || la.kind == 38) {
-				if (la.kind == 38) {
+			if (la.kind == 15 || la.kind == 42) {
+				if (la.kind == 42) {
 					GenericParameters(typeArgs);
 				}
 				Formals(true, isFunctionMethod, formals, out openParen);
 				Expect(7);
 				Type(out returnType);
-			} else if (la.kind == 37) {
+			} else if (la.kind == 41) {
 				Get();
 				signatureEllipsis = t;
 				openParen = Token.NoToken; 
-			} else SynErr(141);
-		} else if (la.kind == 63) {
+			} else SynErr(142);
+		} else if (la.kind == 65) {
 			Get();
 			isPredicate = true; 
-			if (la.kind == 40) {
+			if (la.kind == 44) {
 				Get();
 				isFunctionMethod = true; 
 			}
 			if (mmod.IsGhost) { SemErr(t, "predicates cannot be declared 'ghost' (they are ghost by default)"); }
 			
-			while (la.kind == 9) {
+			while (la.kind == 13) {
 				Attribute(ref attrs);
 			}
 			NoUSIdent(out id);
 			if (StartOf(6)) {
-				if (la.kind == 38) {
+				if (la.kind == 42) {
 					GenericParameters(typeArgs);
 				}
-				if (la.kind == 11) {
+				if (la.kind == 15) {
 					Formals(true, isFunctionMethod, formals, out openParen);
 					if (la.kind == 7) {
 						Get();
 						SemErr(t, "predicates do not have an explicitly declared return type; it is always bool"); 
 					}
 				}
-			} else if (la.kind == 37) {
+			} else if (la.kind == 41) {
 				Get();
 				signatureEllipsis = t;
 				openParen = Token.NoToken; 
-			} else SynErr(142);
-		} else if (la.kind == 64) {
+			} else SynErr(143);
+		} else if (la.kind == 66) {
 			Get();
 			isCoPredicate = true; 
 			if (mmod.IsGhost) { SemErr(t, "copredicates cannot be declared 'ghost' (they are ghost by default)"); }
 			
-			while (la.kind == 9) {
+			while (la.kind == 13) {
 				Attribute(ref attrs);
 			}
 			NoUSIdent(out id);
 			if (StartOf(6)) {
-				if (la.kind == 38) {
+				if (la.kind == 42) {
 					GenericParameters(typeArgs);
 				}
-				if (la.kind == 11) {
+				if (la.kind == 15) {
 					Formals(true, isFunctionMethod, formals, out openParen);
 					if (la.kind == 7) {
 						Get();
 						SemErr(t, "copredicates do not have an explicitly declared return type; it is always bool"); 
 					}
 				}
-			} else if (la.kind == 37) {
+			} else if (la.kind == 41) {
 				Get();
 				signatureEllipsis = t;
 				openParen = Token.NoToken; 
-			} else SynErr(143);
-		} else SynErr(144);
+			} else SynErr(144);
+		} else SynErr(145);
 		decreases = isCoPredicate ? null : new List<Expression/*!*/>(); 
 		while (StartOf(7)) {
 			FunctionSpec(reqs, reads, ens, decreases);
 		}
-		if (la.kind == 9) {
+		if (la.kind == 13) {
 			FunctionBody(out body, out bodyStart, out bodyEnd);
 		}
 		if (DafnyOptions.O.DisallowSoundnessCheating && body == null && ens.Count > 0 && !Attributes.Contains(attrs, "axiom")) {
@@ -887,21 +905,21 @@ bool CloseOptionalBrace(bool usesOptionalBrace) {
 		IToken bodyStart = Token.NoToken;
 		IToken bodyEnd = Token.NoToken;
 		
-		while (!(StartOf(8))) {SynErr(145); Get();}
-		if (la.kind == 40) {
+		while (!(StartOf(8))) {SynErr(146); Get();}
+		if (la.kind == 44) {
 			Get();
-		} else if (la.kind == 41) {
+		} else if (la.kind == 45) {
 			Get();
 			isLemma = true; 
-		} else if (la.kind == 42) {
+		} else if (la.kind == 46) {
 			Get();
 			isCoLemma = true; 
-		} else if (la.kind == 43) {
+		} else if (la.kind == 47) {
 			Get();
 			isCoLemma = true;
 			errors.Warning(t, "the 'comethod' keyword has been deprecated; it has been renamed to 'colemma'");
 			
-		} else if (la.kind == 44) {
+		} else if (la.kind == 48) {
 			Get();
 			if (allowConstructor) {
 			 isConstructor = true;
@@ -909,7 +927,7 @@ bool CloseOptionalBrace(bool usesOptionalBrace) {
 			 SemErr(t, "constructors are only allowed in classes");
 			}
 			
-		} else SynErr(146);
+		} else SynErr(147);
 		keywordToken = t; 
 		if (isLemma) {
 		 if (mmod.IsGhost) {
@@ -928,7 +946,7 @@ bool CloseOptionalBrace(bool usesOptionalBrace) {
 		 }
 		}
 		
-		while (la.kind == 9) {
+		while (la.kind == 13) {
 			Attribute(ref attrs);
 		}
 		if (la.kind == 1) {
@@ -942,24 +960,24 @@ bool CloseOptionalBrace(bool usesOptionalBrace) {
 		 }
 		}
 		
-		if (la.kind == 11 || la.kind == 38) {
-			if (la.kind == 38) {
+		if (la.kind == 15 || la.kind == 42) {
+			if (la.kind == 42) {
 				GenericParameters(typeArgs);
 			}
 			Formals(true, !mmod.IsGhost, ins, out openParen);
-			if (la.kind == 36) {
+			if (la.kind == 40) {
 				Get();
 				if (isConstructor) { SemErr(t, "constructors cannot have out-parameters"); } 
 				Formals(false, !mmod.IsGhost, outs, out openParen);
 			}
-		} else if (la.kind == 37) {
+		} else if (la.kind == 41) {
 			Get();
 			signatureEllipsis = t; openParen = Token.NoToken; 
-		} else SynErr(147);
+		} else SynErr(148);
 		while (StartOf(9)) {
 			MethodSpec(req, mod, ens, dec, ref decAttrs, ref modAttrs);
 		}
-		if (la.kind == 9) {
+		if (la.kind == 13) {
 			BlockStmt(out body, out bodyStart, out bodyEnd);
 		}
 		if (Attributes.Contains(attrs, "axiom") && !mmod.IsGhost && !isLemma) {
@@ -995,11 +1013,11 @@ bool CloseOptionalBrace(bool usesOptionalBrace) {
 		IToken/*!*/ id;
 		List<Formal/*!*/> formals = new List<Formal/*!*/>();
 		
-		while (la.kind == 9) {
+		while (la.kind == 13) {
 			Attribute(ref attrs);
 		}
 		NoUSIdent(out id);
-		if (la.kind == 11) {
+		if (la.kind == 15) {
 			FormalsOptionalIds(formals);
 		}
 		ctors.Add(new DatatypeCtor(id, id.val, formals, attrs)); 
@@ -1007,17 +1025,17 @@ bool CloseOptionalBrace(bool usesOptionalBrace) {
 
 	void FormalsOptionalIds(List<Formal/*!*/>/*!*/ formals) {
 		Contract.Requires(cce.NonNullElements(formals)); IToken/*!*/ id;  Type/*!*/ ty;  string/*!*/ name;  bool isGhost; 
-		Expect(11);
+		Expect(15);
 		if (StartOf(10)) {
 			TypeIdentOptional(out id, out name, out ty, out isGhost);
 			formals.Add(new Formal(id, name, ty, true, isGhost)); 
-			while (la.kind == 31) {
+			while (la.kind == 35) {
 				Get();
 				TypeIdentOptional(out id, out name, out ty, out isGhost);
 				formals.Add(new Formal(id, name, ty, true, isGhost)); 
 			}
 		}
-		Expect(12);
+		Expect(16);
 	}
 
 	void FIdentType(out IToken/*!*/ id, out Type/*!*/ ty) {
@@ -1029,12 +1047,12 @@ bool CloseOptionalBrace(bool usesOptionalBrace) {
 		} else if (la.kind == 2) {
 			Get();
 			id = t; 
-		} else SynErr(148);
+		} else SynErr(149);
 		Expect(7);
 		Type(out ty);
 	}
 
-	void Type(out Type/*!*/ ty) {
+	void Type(out Type ty) {
 		Contract.Ensures(Contract.ValueAtReturn(out ty) != null); IToken/*!*/ tok; 
 		TypeAndToken(out tok, out ty);
 	}
@@ -1043,7 +1061,7 @@ bool CloseOptionalBrace(bool usesOptionalBrace) {
 		Contract.Ensures(Contract.ValueAtReturn(out id)!=null);
 		Contract.Ensures(Contract.ValueAtReturn(out ty)!=null);
 		isGhost = false; 
-		if (la.kind == 25) {
+		if (la.kind == 29) {
 			Get();
 			if (allowGhostKeyword) { isGhost = true; } else { SemErr(t, "formal cannot be declared 'ghost' in this context"); } 
 		}
@@ -1101,7 +1119,7 @@ bool CloseOptionalBrace(bool usesOptionalBrace) {
 		Contract.Ensures(Contract.ValueAtReturn(out ty)!=null);
 		Contract.Ensures(Contract.ValueAtReturn(out identName)!=null);
 		string name = null; id = Token.NoToken; ty = new BoolType()/*dummy*/; isGhost = false; 
-		if (la.kind == 25) {
+		if (la.kind == 29) {
 			Get();
 			isGhost = true; 
 		}
@@ -1123,7 +1141,7 @@ bool CloseOptionalBrace(bool usesOptionalBrace) {
 			id = t; name = id.val;
 			Expect(7);
 			Type(out ty);
-		} else SynErr(149);
+		} else SynErr(150);
 		if (name != null) {
 		 identName = name;
 		} else {
@@ -1132,36 +1150,36 @@ bool CloseOptionalBrace(bool usesOptionalBrace) {
 		
 	}
 
-	void TypeAndToken(out IToken/*!*/ tok, out Type/*!*/ ty) {
+	void TypeAndToken(out IToken tok, out Type ty) {
 		Contract.Ensures(Contract.ValueAtReturn(out tok)!=null); Contract.Ensures(Contract.ValueAtReturn(out ty) != null);
 		tok = Token.NoToken;  ty = new BoolType();  /*keep compiler happy*/
-		List<Type> gt;
+		List<Type> gt = null;
 		
 		switch (la.kind) {
-		case 52: {
+		case 54: {
 			Get();
 			tok = t; 
 			break;
 		}
-		case 53: {
+		case 55: {
 			Get();
 			tok = t;  ty = new NatType(); 
 			break;
 		}
-		case 54: {
+		case 56: {
 			Get();
 			tok = t;  ty = new IntType(); 
 			break;
 		}
-		case 55: {
+		case 57: {
 			Get();
 			tok = t;  ty = new RealType(); 
 			break;
 		}
-		case 56: {
+		case 58: {
 			Get();
 			tok = t;  gt = new List<Type/*!*/>(); 
-			if (la.kind == 38) {
+			if (la.kind == 42) {
 				GenericInstantiation(gt);
 			}
 			if (gt.Count > 1) {
@@ -1171,10 +1189,10 @@ bool CloseOptionalBrace(bool usesOptionalBrace) {
 			
 			break;
 		}
-		case 57: {
+		case 59: {
 			Get();
 			tok = t;  gt = new List<Type/*!*/>(); 
-			if (la.kind == 38) {
+			if (la.kind == 42) {
 				GenericInstantiation(gt);
 			}
 			if (gt.Count > 1) {
@@ -1184,10 +1202,10 @@ bool CloseOptionalBrace(bool usesOptionalBrace) {
 			
 			break;
 		}
-		case 58: {
+		case 60: {
 			Get();
 			tok = t;  gt = new List<Type/*!*/>(); 
-			if (la.kind == 38) {
+			if (la.kind == 42) {
 				GenericInstantiation(gt);
 			}
 			if (gt.Count > 1) {
@@ -1197,10 +1215,10 @@ bool CloseOptionalBrace(bool usesOptionalBrace) {
 			
 			break;
 		}
-		case 59: {
+		case 61: {
 			Get();
 			tok = t;  gt = new List<Type/*!*/>(); 
-			if (la.kind == 38) {
+			if (la.kind == 42) {
 				GenericInstantiation(gt);
 			}
 			if (gt.Count == 0) {
@@ -1214,19 +1232,19 @@ bool CloseOptionalBrace(bool usesOptionalBrace) {
 			
 			break;
 		}
-		case 11: {
+		case 15: {
 			Get();
 			tok = t; gt = new List<Type>(); 
 			if (StartOf(11)) {
 				Type(out ty);
 				gt.Add(ty); 
-				while (la.kind == 31) {
+				while (la.kind == 35) {
 					Get();
 					Type(out ty);
 					gt.Add(ty); 
 				}
 			}
-			Expect(12);
+			Expect(16);
 			if (gt.Count == 1) {
 			 // just return the type 'ty'
 			} else {
@@ -1238,28 +1256,38 @@ bool CloseOptionalBrace(bool usesOptionalBrace) {
 			
 			break;
 		}
-		case 1: case 5: case 60: {
+		case 1: case 5: case 62: {
 			ReferenceType(out tok, out ty);
 			break;
 		}
-		default: SynErr(150); break;
+		default: SynErr(151); break;
+		}
+		if (la.kind == 10) {
+			Type t2; 
+			Get();
+			Type(out t2);
+			if (gt == null) {
+			 gt = new List<Type>{ ty };
+			}
+			ty = new ArrowType(gt, t2);
+			
 		}
 	}
 
 	void Formals(bool incoming, bool allowGhostKeyword, List<Formal/*!*/>/*!*/ formals, out IToken openParen) {
 		Contract.Requires(cce.NonNullElements(formals)); IToken/*!*/ id;  Type/*!*/ ty;  bool isGhost; 
-		Expect(11);
+		Expect(15);
 		openParen = t; 
-		if (la.kind == 1 || la.kind == 25) {
+		if (la.kind == 1 || la.kind == 29) {
 			GIdentType(allowGhostKeyword, out id, out ty, out isGhost);
 			formals.Add(new Formal(id, id.val, ty, incoming, isGhost)); 
-			while (la.kind == 31) {
+			while (la.kind == 35) {
 				Get();
 				GIdentType(allowGhostKeyword, out id, out ty, out isGhost);
 				formals.Add(new Formal(id, id.val, ty, incoming, isGhost)); 
 			}
 		}
-		Expect(12);
+		Expect(16);
 	}
 
 	void IteratorSpec(List<FrameExpression/*!*/>/*!*/ reads, List<FrameExpression/*!*/>/*!*/ mod, List<Expression/*!*/> decreases,
@@ -1268,8 +1296,8 @@ List<MaybeFreeExpression/*!*/>/*!*/ yieldReq, List<MaybeFreeExpression/*!*/>/*!*
 ref Attributes readsAttrs, ref Attributes modAttrs, ref Attributes decrAttrs) {
 		Expression/*!*/ e; FrameExpression/*!*/ fe; bool isFree = false; bool isYield = false; Attributes ensAttrs = null;
 		
-		while (!(StartOf(12))) {SynErr(151); Get();}
-		if (la.kind == 50) {
+		while (!(StartOf(12))) {SynErr(152); Get();}
+		if (la.kind == 11) {
 			Get();
 			while (IsAttribute()) {
 				Attribute(ref readsAttrs);
@@ -1277,15 +1305,15 @@ ref Attributes readsAttrs, ref Attributes modAttrs, ref Attributes decrAttrs) {
 			if (StartOf(13)) {
 				FrameExpression(out fe);
 				reads.Add(fe); 
-				while (la.kind == 31) {
+				while (la.kind == 35) {
 					Get();
 					FrameExpression(out fe);
 					reads.Add(fe); 
 				}
 			}
-			while (!(la.kind == 0 || la.kind == 8)) {SynErr(152); Get();}
+			while (!(la.kind == 0 || la.kind == 8)) {SynErr(153); Get();}
 			Expect(8);
-		} else if (la.kind == 45) {
+		} else if (la.kind == 49) {
 			Get();
 			while (IsAttribute()) {
 				Attribute(ref modAttrs);
@@ -1293,70 +1321,70 @@ ref Attributes readsAttrs, ref Attributes modAttrs, ref Attributes decrAttrs) {
 			if (StartOf(13)) {
 				FrameExpression(out fe);
 				mod.Add(fe); 
-				while (la.kind == 31) {
+				while (la.kind == 35) {
 					Get();
 					FrameExpression(out fe);
 					mod.Add(fe); 
 				}
 			}
-			while (!(la.kind == 0 || la.kind == 8)) {SynErr(153); Get();}
+			while (!(la.kind == 0 || la.kind == 8)) {SynErr(154); Get();}
 			Expect(8);
 		} else if (StartOf(14)) {
-			if (la.kind == 46) {
+			if (la.kind == 50) {
 				Get();
 				isFree = true; 
 			}
-			if (la.kind == 51) {
+			if (la.kind == 53) {
 				Get();
 				isYield = true; 
 			}
-			if (la.kind == 47) {
+			if (la.kind == 12) {
 				Get();
-				Expression(out e, false);
-				while (!(la.kind == 0 || la.kind == 8)) {SynErr(154); Get();}
+				Expression(out e, false, true);
+				while (!(la.kind == 0 || la.kind == 8)) {SynErr(155); Get();}
 				Expect(8);
 				if (isYield) {
-				 yieldReq.Add(new MaybeFreeExpression(e, isFree));
+				yieldReq.Add(new MaybeFreeExpression(e, isFree));
 				} else {
-				 req.Add(new MaybeFreeExpression(e, isFree));
+				req.Add(new MaybeFreeExpression(e, isFree));
 				}
 				
-			} else if (la.kind == 48) {
+			} else if (la.kind == 51) {
 				Get();
 				while (IsAttribute()) {
 					Attribute(ref ensAttrs);
 				}
-				Expression(out e, false);
-				while (!(la.kind == 0 || la.kind == 8)) {SynErr(155); Get();}
+				Expression(out e, false, true);
+				while (!(la.kind == 0 || la.kind == 8)) {SynErr(156); Get();}
 				Expect(8);
 				if (isYield) {
-				 yieldEns.Add(new MaybeFreeExpression(e, isFree, ensAttrs));
+				yieldEns.Add(new MaybeFreeExpression(e, isFree, ensAttrs));
 				} else {
-				 ens.Add(new MaybeFreeExpression(e, isFree, ensAttrs));
+				ens.Add(new MaybeFreeExpression(e, isFree, ensAttrs));
 				}
 				
-			} else SynErr(156);
-		} else if (la.kind == 49) {
+			} else SynErr(157);
+		} else if (la.kind == 52) {
 			Get();
 			while (IsAttribute()) {
 				Attribute(ref decrAttrs);
 			}
 			DecreasesList(decreases, false);
-			while (!(la.kind == 0 || la.kind == 8)) {SynErr(157); Get();}
+			while (!(la.kind == 0 || la.kind == 8)) {SynErr(158); Get();}
 			Expect(8);
-		} else SynErr(158);
+		} else SynErr(159);
 	}
 
 	void BlockStmt(out BlockStmt/*!*/ block, out IToken bodyStart, out IToken bodyEnd) {
 		Contract.Ensures(Contract.ValueAtReturn(out block) != null);
 		List<Statement/*!*/> body = new List<Statement/*!*/>();
 		
-		Expect(9);
+		Expect(13);
 		bodyStart = t; 
 		while (StartOf(15)) {
 			Stmt(body);
 		}
-		Expect(10);
+		Expect(14);
 		bodyEnd = t;
 		block = new BlockStmt(bodyStart, bodyEnd, body); 
 	}
@@ -1366,8 +1394,8 @@ List<Expression/*!*/>/*!*/ decreases, ref Attributes decAttrs, ref Attributes mo
 		Contract.Requires(cce.NonNullElements(req)); Contract.Requires(cce.NonNullElements(mod)); Contract.Requires(cce.NonNullElements(ens)); Contract.Requires(cce.NonNullElements(decreases));
 		Expression/*!*/ e;  FrameExpression/*!*/ fe;  bool isFree = false; Attributes ensAttrs = null;
 		
-		while (!(StartOf(16))) {SynErr(159); Get();}
-		if (la.kind == 45) {
+		while (!(StartOf(16))) {SynErr(160); Get();}
+		if (la.kind == 49) {
 			Get();
 			while (IsAttribute()) {
 				Attribute(ref modAttrs);
@@ -1375,44 +1403,44 @@ List<Expression/*!*/>/*!*/ decreases, ref Attributes decAttrs, ref Attributes mo
 			if (StartOf(13)) {
 				FrameExpression(out fe);
 				mod.Add(fe); 
-				while (la.kind == 31) {
+				while (la.kind == 35) {
 					Get();
 					FrameExpression(out fe);
 					mod.Add(fe); 
 				}
 			}
-			while (!(la.kind == 0 || la.kind == 8)) {SynErr(160); Get();}
+			while (!(la.kind == 0 || la.kind == 8)) {SynErr(161); Get();}
 			Expect(8);
-		} else if (la.kind == 46 || la.kind == 47 || la.kind == 48) {
-			if (la.kind == 46) {
+		} else if (la.kind == 12 || la.kind == 50 || la.kind == 51) {
+			if (la.kind == 50) {
 				Get();
 				isFree = true; 
 			}
-			if (la.kind == 47) {
+			if (la.kind == 12) {
 				Get();
-				Expression(out e, false);
-				while (!(la.kind == 0 || la.kind == 8)) {SynErr(161); Get();}
+				Expression(out e, false, true);
+				while (!(la.kind == 0 || la.kind == 8)) {SynErr(162); Get();}
 				Expect(8);
 				req.Add(new MaybeFreeExpression(e, isFree)); 
-			} else if (la.kind == 48) {
+			} else if (la.kind == 51) {
 				Get();
 				while (IsAttribute()) {
 					Attribute(ref ensAttrs);
 				}
-				Expression(out e, false);
-				while (!(la.kind == 0 || la.kind == 8)) {SynErr(162); Get();}
+				Expression(out e, false, true);
+				while (!(la.kind == 0 || la.kind == 8)) {SynErr(163); Get();}
 				Expect(8);
 				ens.Add(new MaybeFreeExpression(e, isFree, ensAttrs)); 
-			} else SynErr(163);
-		} else if (la.kind == 49) {
+			} else SynErr(164);
+		} else if (la.kind == 52) {
 			Get();
 			while (IsAttribute()) {
 				Attribute(ref decAttrs);
 			}
 			DecreasesList(decreases, true);
-			while (!(la.kind == 0 || la.kind == 8)) {SynErr(164); Get();}
+			while (!(la.kind == 0 || la.kind == 8)) {SynErr(165); Get();}
 			Expect(8);
-		} else SynErr(165);
+		} else SynErr(166);
 	}
 
 	void FrameExpression(out FrameExpression/*!*/ fe) {
@@ -1423,29 +1451,29 @@ List<Expression/*!*/>/*!*/ decreases, ref Attributes decAttrs, ref Attributes mo
 		fe = null;
 		
 		if (StartOf(17)) {
-			Expression(out e, false);
+			Expression(out e, false, false);
 			feTok = e.tok; 
-			if (la.kind == 65) {
+			if (la.kind == 67) {
 				Get();
 				Ident(out id);
 				fieldName = id.val;  feTok = id; 
 			}
 			fe = new FrameExpression(feTok, e, fieldName); 
-		} else if (la.kind == 65) {
+		} else if (la.kind == 67) {
 			Get();
 			Ident(out id);
 			fieldName = id.val; 
 			fe = new FrameExpression(id, new ImplicitThisExpr(id), fieldName); 
-		} else SynErr(166);
+		} else SynErr(167);
 	}
 
-	void Expression(out Expression e, bool allowSemi) {
+	void Expression(out Expression e, bool allowSemi, bool allowLambda) {
 		Expression e0; IToken endTok; 
-		EquivExpression(out e, allowSemi);
+		EquivExpression(out e, allowSemi, allowLambda);
 		if (SemiFollowsCall(allowSemi, e)) {
 			Expect(8);
 			endTok = t; 
-			Expression(out e0, allowSemi);
+			Expression(out e0, allowSemi, allowLambda);
 			e = new StmtExpr(e.tok,
 			     new UpdateStmt(e.tok, endTok, new List<Expression>(), new List<AssignmentRhs>() { new ExprRhs(e, null) }),
 			     e0);
@@ -1462,7 +1490,7 @@ List<Expression/*!*/>/*!*/ decreases, ref Attributes decAttrs, ref Attributes mo
 		 decreases.Add(e);
 		}
 		
-		while (la.kind == 31) {
+		while (la.kind == 35) {
 			Get();
 			PossiblyWildExpression(out e);
 			if (!allowWildcard && e is WildcardExpr) {
@@ -1476,15 +1504,15 @@ List<Expression/*!*/>/*!*/ decreases, ref Attributes decAttrs, ref Attributes mo
 
 	void GenericInstantiation(List<Type/*!*/>/*!*/ gt) {
 		Contract.Requires(cce.NonNullElements(gt)); Type/*!*/ ty; 
-		Expect(38);
+		Expect(42);
 		Type(out ty);
 		gt.Add(ty); 
-		while (la.kind == 31) {
+		while (la.kind == 35) {
 			Get();
 			Type(out ty);
 			gt.Add(ty); 
 		}
-		Expect(39);
+		Expect(43);
 	}
 
 	void ReferenceType(out IToken/*!*/ tok, out Type/*!*/ ty) {
@@ -1493,13 +1521,13 @@ List<Expression/*!*/>/*!*/ decreases, ref Attributes decAttrs, ref Attributes mo
 		List<Type> gt;
 		List<IToken> path;
 		
-		if (la.kind == 60) {
+		if (la.kind == 62) {
 			Get();
 			tok = t;  ty = new ObjectType(); 
 		} else if (la.kind == 5) {
 			Get();
 			tok = t;  gt = new List<Type>(); 
-			if (la.kind == 38) {
+			if (la.kind == 42) {
 				GenericInstantiation(gt);
 			}
 			int dims = tok.val.Length == 5 ? 1 : int.Parse(tok.val.Substring(5));
@@ -1509,16 +1537,16 @@ List<Expression/*!*/>/*!*/ decreases, ref Attributes decAttrs, ref Attributes mo
 			Ident(out tok);
 			gt = new List<Type>();
 			path = new List<IToken>(); 
-			while (la.kind == 61) {
+			while (la.kind == 63) {
 				path.Add(tok); 
 				Get();
 				Ident(out tok);
 			}
-			if (la.kind == 38) {
+			if (la.kind == 42) {
 				GenericInstantiation(gt);
 			}
 			ty = new UserDefinedType(tok, tok.val, gt, path); 
-		} else SynErr(167);
+		} else SynErr(168);
 	}
 
 	void FunctionSpec(List<Expression/*!*/>/*!*/ reqs, List<FrameExpression/*!*/>/*!*/ reads, List<Expression/*!*/>/*!*/ ens, List<Expression/*!*/> decreases) {
@@ -1526,33 +1554,33 @@ List<Expression/*!*/>/*!*/ decreases, ref Attributes decAttrs, ref Attributes mo
 		Contract.Requires(cce.NonNullElements(reads));
 		Contract.Requires(decreases == null || cce.NonNullElements(decreases));
 		Expression/*!*/ e;  FrameExpression/*!*/ fe; 
-		if (la.kind == 47) {
-			while (!(la.kind == 0 || la.kind == 47)) {SynErr(168); Get();}
+		if (la.kind == 12) {
+			while (!(la.kind == 0 || la.kind == 12)) {SynErr(169); Get();}
 			Get();
-			Expression(out e, false);
-			while (!(la.kind == 0 || la.kind == 8)) {SynErr(169); Get();}
+			Expression(out e, false, true);
+			while (!(la.kind == 0 || la.kind == 8)) {SynErr(170); Get();}
 			Expect(8);
 			reqs.Add(e); 
-		} else if (la.kind == 50) {
+		} else if (la.kind == 11) {
 			Get();
 			if (StartOf(18)) {
 				PossiblyWildFrameExpression(out fe);
 				reads.Add(fe); 
-				while (la.kind == 31) {
+				while (la.kind == 35) {
 					Get();
 					PossiblyWildFrameExpression(out fe);
 					reads.Add(fe); 
 				}
 			}
-			while (!(la.kind == 0 || la.kind == 8)) {SynErr(170); Get();}
-			Expect(8);
-		} else if (la.kind == 48) {
-			Get();
-			Expression(out e, false);
 			while (!(la.kind == 0 || la.kind == 8)) {SynErr(171); Get();}
 			Expect(8);
+		} else if (la.kind == 51) {
+			Get();
+			Expression(out e, false, true);
+			while (!(la.kind == 0 || la.kind == 8)) {SynErr(172); Get();}
+			Expect(8);
 			ens.Add(e); 
-		} else if (la.kind == 49) {
+		} else if (la.kind == 52) {
 			Get();
 			if (decreases == null) {
 			 SemErr(t, "'decreases' clauses are meaningless for copredicates, so they are not allowed");
@@ -1560,39 +1588,60 @@ List<Expression/*!*/>/*!*/ decreases, ref Attributes decAttrs, ref Attributes mo
 			}
 			
 			DecreasesList(decreases, false);
-			while (!(la.kind == 0 || la.kind == 8)) {SynErr(172); Get();}
+			while (!(la.kind == 0 || la.kind == 8)) {SynErr(173); Get();}
 			Expect(8);
-		} else SynErr(173);
+		} else SynErr(174);
 	}
 
 	void FunctionBody(out Expression/*!*/ e, out IToken bodyStart, out IToken bodyEnd) {
 		Contract.Ensures(Contract.ValueAtReturn(out e) != null); e = dummyExpr; 
-		Expect(9);
+		Expect(13);
 		bodyStart = t; 
-		Expression(out e, true);
-		Expect(10);
+		Expression(out e, true, true);
+		Expect(14);
 		bodyEnd = t; 
 	}
 
 	void PossiblyWildFrameExpression(out FrameExpression/*!*/ fe) {
 		Contract.Ensures(Contract.ValueAtReturn(out fe) != null); fe = dummyFrameExpr; 
-		if (la.kind == 13) {
+		if (la.kind == 17) {
 			Get();
 			fe = new FrameExpression(t, new WildcardExpr(t), null); 
 		} else if (StartOf(13)) {
 			FrameExpression(out fe);
-		} else SynErr(174);
+		} else SynErr(175);
+	}
+
+	void LambdaSpec(out Expression req, List<FrameExpression> reads) {
+		Contract.Requires(reads != null);
+		Expression e; req = null;  FrameExpression fe; 
+		while (la.kind == 11 || la.kind == 12) {
+			if (la.kind == 12) {
+				Get();
+				Expression(out e, false, false);
+				if (req == null) {
+				 req = e;
+				} else {
+				 req = new BinaryExpr(req.tok, BinaryExpr.Opcode.And, req, e);
+				}
+				
+			} else {
+				Get();
+				PossiblyWildFrameExpression(out fe);
+				reads.Add(fe); 
+			}
+		}
 	}
 
 	void PossiblyWildExpression(out Expression/*!*/ e) {
 		Contract.Ensures(Contract.ValueAtReturn(out e)!=null);
 		e = dummyExpr; 
-		if (la.kind == 13) {
+		if (la.kind == 17) {
 			Get();
 			e = new WildcardExpr(t); 
 		} else if (StartOf(17)) {
-			Expression(out e, false);
-		} else SynErr(175);
+			Expression(out e, false, false);
+		} else SynErr(176);
 	}
 
 	void Stmt(List<Statement/*!*/>/*!*/ ss) {
@@ -1609,58 +1658,58 @@ List<Expression/*!*/>/*!*/ decreases, ref Attributes decAttrs, ref Attributes mo
 		IToken bodyStart, bodyEnd;
 		int breakCount;
 		
-		while (!(StartOf(19))) {SynErr(176); Get();}
+		while (!(StartOf(19))) {SynErr(177); Get();}
 		switch (la.kind) {
-		case 9: {
+		case 13: {
 			BlockStmt(out bs, out bodyStart, out bodyEnd);
 			s = bs; 
 			break;
 		}
-		case 83: {
+		case 84: {
 			AssertStmt(out s);
 			break;
 		}
-		case 72: {
+		case 74: {
 			AssumeStmt(out s);
 			break;
 		}
-		case 84: {
+		case 85: {
 			PrintStmt(out s);
 			break;
 		}
-		case 1: case 2: case 3: case 4: case 11: case 29: case 54: case 55: case 113: case 114: case 115: case 116: case 117: case 118: {
+		case 1: case 2: case 3: case 4: case 15: case 33: case 56: case 57: case 114: case 115: case 116: case 117: case 118: case 119: {
 			UpdateStmt(out s);
 			break;
 		}
-		case 25: case 30: {
+		case 29: case 34: {
 			VarDeclStatement(out s);
 			break;
 		}
-		case 76: {
+		case 78: {
 			IfStmt(out s);
 			break;
 		}
-		case 80: {
+		case 81: {
 			WhileStmt(out s);
 			break;
 		}
-		case 82: {
+		case 83: {
 			MatchStmt(out s);
 			break;
 		}
-		case 85: case 86: {
+		case 86: case 87: {
 			ForallStmt(out s);
 			break;
 		}
-		case 88: {
+		case 89: {
 			CalcStmt(out s);
 			break;
 		}
-		case 87: {
+		case 88: {
 			ModifyStmt(out s);
 			break;
 		}
-		case 66: {
+		case 68: {
 			Get();
 			x = t; 
 			NoUSIdent(out id);
@@ -1669,32 +1718,32 @@ List<Expression/*!*/>/*!*/ decreases, ref Attributes decAttrs, ref Attributes mo
 			s.Labels = new LList<Label>(new Label(x, id.val), s.Labels); 
 			break;
 		}
-		case 67: {
+		case 69: {
 			Get();
 			x = t; breakCount = 1; label = null; 
 			if (la.kind == 1) {
 				NoUSIdent(out id);
 				label = id.val; 
-			} else if (la.kind == 8 || la.kind == 67) {
-				while (la.kind == 67) {
+			} else if (la.kind == 8 || la.kind == 69) {
+				while (la.kind == 69) {
 					Get();
 					breakCount++; 
 				}
-			} else SynErr(177);
-			while (!(la.kind == 0 || la.kind == 8)) {SynErr(178); Get();}
+			} else SynErr(178);
+			while (!(la.kind == 0 || la.kind == 8)) {SynErr(179); Get();}
 			Expect(8);
 			s = label != null ? new BreakStmt(x, t, label) : new BreakStmt(x, t, breakCount); 
 			break;
 		}
-		case 51: case 70: {
+		case 53: case 72: {
 			ReturnStmt(out s);
 			break;
 		}
-		case 37: {
+		case 41: {
 			SkeletonStmt(out s);
 			break;
 		}
-		default: SynErr(179); break;
+		default: SynErr(180); break;
 		}
 	}
 
@@ -1703,17 +1752,17 @@ List<Expression/*!*/>/*!*/ decreases, ref Attributes decAttrs, ref Attributes mo
 		Expression e = dummyExpr; Attributes attrs = null;
 		IToken dotdotdot = null;
 		
-		Expect(83);
+		Expect(84);
 		x = t; 
 		while (IsAttribute()) {
 			Attribute(ref attrs);
 		}
 		if (StartOf(17)) {
-			Expression(out e, false);
-		} else if (la.kind == 37) {
+			Expression(out e, false, true);
+		} else if (la.kind == 41) {
 			Get();
 			dotdotdot = t; 
-		} else SynErr(180);
+		} else SynErr(181);
 		Expect(8);
 		if (dotdotdot != null) {
 		 s = new SkeletonStatement(new AssertStmt(x, t, new LiteralExpr(x, true), attrs), dotdotdot, null);
@@ -1728,17 +1777,17 @@ List<Expression/*!*/>/*!*/ decreases, ref Attributes decAttrs, ref Attributes mo
 		Expression e = dummyExpr; Attributes attrs = null;
 		IToken dotdotdot = null;
 		
-		Expect(72);
+		Expect(74);
 		x = t; 
 		while (IsAttribute()) {
 			Attribute(ref attrs);
 		}
 		if (StartOf(17)) {
-			Expression(out e, false);
-		} else if (la.kind == 37) {
+			Expression(out e, false, true);
+		} else if (la.kind == 41) {
 			Get();
 			dotdotdot = t; 
-		} else SynErr(181);
+		} else SynErr(182);
 		Expect(8);
 		if (dotdotdot != null) {
 		 s = new SkeletonStatement(new AssumeStmt(x, t, new LiteralExpr(x, true), attrs), dotdotdot, null);
@@ -1752,11 +1801,11 @@ List<Expression/*!*/>/*!*/ decreases, ref Attributes decAttrs, ref Attributes mo
 		Contract.Ensures(Contract.ValueAtReturn(out s) != null); IToken/*!*/ x;  Attributes.Argument/*!*/ arg;
 		List<Attributes.Argument/*!*/> args = new List<Attributes.Argument/*!*/>();
 		
-		Expect(84);
+		Expect(85);
 		x = t; 
 		AttributeArg(out arg, false);
 		args.Add(arg); 
-		while (la.kind == 31) {
+		while (la.kind == 35) {
 			Get();
 			AttributeArg(out arg, false);
 			args.Add(arg); 
@@ -1777,44 +1826,44 @@ List<Expression/*!*/>/*!*/ decreases, ref Attributes decAttrs, ref Attributes mo
 		
 		Lhs(out e);
 		x = e.tok; 
-		if (la.kind == 8 || la.kind == 9) {
-			while (la.kind == 9) {
+		if (la.kind == 8 || la.kind == 13) {
+			while (la.kind == 13) {
 				Attribute(ref attrs);
 			}
 			Expect(8);
 			endTok = t; rhss.Add(new ExprRhs(e, attrs)); 
-		} else if (la.kind == 31 || la.kind == 69 || la.kind == 71) {
+		} else if (la.kind == 35 || la.kind == 71 || la.kind == 73) {
 			lhss.Add(e);  lhs0 = e; 
-			while (la.kind == 31) {
+			while (la.kind == 35) {
 				Get();
 				Lhs(out e);
 				lhss.Add(e); 
 			}
-			if (la.kind == 69) {
+			if (la.kind == 71) {
 				Get();
 				x = t; 
 				Rhs(out r, lhs0);
 				rhss.Add(r); 
-				while (la.kind == 31) {
+				while (la.kind == 35) {
 					Get();
 					Rhs(out r, lhs0);
 					rhss.Add(r); 
 				}
-			} else if (la.kind == 71) {
+			} else if (la.kind == 73) {
 				Get();
 				x = t; 
-				if (la.kind == 72) {
+				if (la.kind == 74) {
 					Get();
 					suchThatAssume = t; 
 				}
-				Expression(out suchThat, false);
-			} else SynErr(182);
+				Expression(out suchThat, false, true);
+			} else SynErr(183);
 			Expect(8);
 			endTok = t; 
 		} else if (la.kind == 7) {
 			Get();
 			SemErr(t, "invalid statement (did you forget the 'label' keyword?)"); 
-		} else SynErr(183);
+		} else SynErr(184);
 		if (suchThat != null) {
 		 s = new AssignSuchThatStmt(x, endTok, lhss, suchThat, suchThatAssume);
 		} else {
@@ -1838,34 +1887,34 @@ List<Expression/*!*/>/*!*/ decreases, ref Attributes decAttrs, ref Attributes mo
 		Attributes attrs = null;
 		IToken endTok;
 		
-		if (la.kind == 25) {
+		if (la.kind == 29) {
 			Get();
 			isGhost = true;  x = t; 
 		}
-		Expect(30);
+		Expect(34);
 		if (!isGhost) { x = t; } 
-		while (la.kind == 9) {
+		while (la.kind == 13) {
 			Attribute(ref attrs);
 		}
 		LocalIdentTypeOptional(out d, isGhost);
 		lhss.Add(d); d.Attributes = attrs; attrs = null; 
-		while (la.kind == 31) {
+		while (la.kind == 35) {
 			Get();
-			while (la.kind == 9) {
+			while (la.kind == 13) {
 				Attribute(ref attrs);
 			}
 			LocalIdentTypeOptional(out d, isGhost);
 			lhss.Add(d); d.Attributes = attrs; attrs = null; 
 		}
-		if (la.kind == 69 || la.kind == 71) {
-			if (la.kind == 69) {
+		if (la.kind == 71 || la.kind == 73) {
+			if (la.kind == 71) {
 				Get();
 				assignTok = t;
 				lhs0 = new IdentifierExpr(lhss[0].Tok, lhss[0].Name);
 				
 				Rhs(out r, lhs0);
 				rhss.Add(r); 
-				while (la.kind == 31) {
+				while (la.kind == 35) {
 					Get();
 					Rhs(out r, lhs0);
 					rhss.Add(r); 
@@ -1873,11 +1922,11 @@ List<Expression/*!*/>/*!*/ decreases, ref Attributes decAttrs, ref Attributes mo
 			} else {
 				Get();
 				assignTok = t; 
-				if (la.kind == 72) {
+				if (la.kind == 74) {
 					Get();
 					suchThatAssume = t; 
 				}
-				Expression(out suchThat, false);
+				Expression(out suchThat, false, true);
 			}
 		}
 		Expect(8);
@@ -1913,7 +1962,7 @@ List<Expression/*!*/>/*!*/ decreases, ref Attributes decAttrs, ref Attributes mo
 		List<GuardedAlternative> alternatives;
 		ifStmt = dummyStmt;  // to please the compiler
 		
-		Expect(76);
+		Expect(78);
 		x = t; 
 		if (IsAlternative()) {
 			AlternativeBlock(out alternatives, out endTok);
@@ -1927,15 +1976,15 @@ List<Expression/*!*/>/*!*/ decreases, ref Attributes decAttrs, ref Attributes mo
 			}
 			BlockStmt(out thn, out bodyStart, out bodyEnd);
 			endTok = thn.EndTok; 
-			if (la.kind == 77) {
+			if (la.kind == 79) {
 				Get();
-				if (la.kind == 76) {
+				if (la.kind == 78) {
 					IfStmt(out s);
 					els = s; endTok = s.EndTok; 
-				} else if (la.kind == 9) {
+				} else if (la.kind == 13) {
 					BlockStmt(out bs, out bodyStart, out bodyEnd);
 					els = bs; endTok = bs.EndTok; 
-				} else SynErr(184);
+				} else SynErr(185);
 			}
 			if (guardEllipsis != null) {
 			 ifStmt = new SkeletonStatement(new IfStmt(x, endTok, guard, thn, els), guardEllipsis, null);
@@ -1943,7 +1992,7 @@ List<Expression/*!*/>/*!*/ decreases, ref Attributes decAttrs, ref Attributes mo
 			 ifStmt = new IfStmt(x, endTok, guard, thn, els);
 			}
 			
-		} else SynErr(185);
+		} else SynErr(186);
 	}
 
 	void WhileStmt(out Statement/*!*/ stmt) {
@@ -1959,7 +2008,7 @@ List<Expression/*!*/>/*!*/ decreases, ref Attributes decAttrs, ref Attributes mo
 		List<GuardedAlternative> alternatives;
 		stmt = dummyStmt;  // to please the compiler
 		
-		Expect(80);
+		Expect(81);
 		x = t; 
 		if (IsLoopSpecOrAlternative()) {
 			LoopSpec(out invariants, out decreases, out mod, ref decAttrs, ref modAttrs);
@@ -1974,13 +2023,13 @@ List<Expression/*!*/>/*!*/ decreases, ref Attributes decAttrs, ref Attributes mo
 				guardEllipsis = t; 
 			}
 			LoopSpec(out invariants, out decreases, out mod, ref decAttrs, ref modAttrs);
-			if (la.kind == 9) {
+			if (la.kind == 13) {
 				BlockStmt(out body, out bodyStart, out bodyEnd);
 				endTok = body.EndTok; 
-			} else if (la.kind == 37) {
+			} else if (la.kind == 41) {
 				Get();
 				bodyEllipsis = t; endTok = t; 
-			} else SynErr(186);
+			} else SynErr(187);
 			if (guardEllipsis != null || bodyEllipsis != null) {
 			 if (mod != null) {
 			   SemErr(mod[0].E.tok, "'modifies' clauses are not allowed on refining loops");
@@ -1996,7 +2045,7 @@ List<Expression/*!*/>/*!*/ decreases, ref Attributes decAttrs, ref Attributes mo
 			 stmt = new WhileStmt(x, endTok, guard, invariants, new Specification<Expression>(decreases, decAttrs), new Specification<FrameExpression>(mod, modAttrs), body);
 			}
 			
-		} else SynErr(187);
+		} else SynErr(188);
 	}
 
 	void MatchStmt(out Statement/*!*/ s) {
@@ -2005,22 +2054,22 @@ List<Expression/*!*/>/*!*/ decreases, ref Attributes decAttrs, ref Attributes mo
 		List<MatchCaseStmt/*!*/> cases = new List<MatchCaseStmt/*!*/>();
 		bool usesOptionalBrace = false;
 		
-		Expect(82);
+		Expect(83);
 		x = t; 
-		Expression(out e, true);
-		if (la.kind == 9) {
+		Expression(out e, true, true);
+		if (la.kind == 13) {
 			Get();
 			usesOptionalBrace = true; 
 		}
-		while (la.kind == 78) {
+		while (la.kind == 80) {
 			CaseStatement(out c);
 			cases.Add(c); 
 		}
 		if (CloseOptionalBrace(usesOptionalBrace)) {
-			Expect(10);
+			Expect(14);
 		} else if (StartOf(22)) {
 			if (usesOptionalBrace) { SemErr(t, "expecting close curly brace"); } 
-		} else SynErr(188);
+		} else SynErr(189);
 		s = new MatchStmt(x, t, e, cases, usesOptionalBrace); 
 	}
 
@@ -2038,16 +2087,16 @@ List<Expression/*!*/>/*!*/ decreases, ref Attributes decAttrs, ref Attributes mo
 		IToken bodyStart, bodyEnd;
 		IToken tok = Token.NoToken;
 		
-		if (la.kind == 85) {
+		if (la.kind == 86) {
 			Get();
 			x = t; tok = x; 
-		} else if (la.kind == 86) {
+		} else if (la.kind == 87) {
 			Get();
 			x = t;
 			errors.Warning(t, "the 'parallel' keyword has been deprecated; the comprehension statement now uses the keyword 'forall' (and the parentheses around the bound variables are now optional)");
 			
-		} else SynErr(189);
-		if (la.kind == 11) {
+		} else SynErr(190);
+		if (la.kind == 15) {
 			Get();
 			usesOptionalParen = true; 
 		}
@@ -2061,23 +2110,23 @@ List<Expression/*!*/>/*!*/ decreases, ref Attributes decAttrs, ref Attributes mo
 		if (range == null) { range = new LiteralExpr(x, true); }
 		
 		if (CloseOptionalParen(usesOptionalParen)) {
-			Expect(12);
+			Expect(16);
 		} else if (StartOf(23)) {
 			if (usesOptionalParen) { SemErr(t, "expecting close parenthesis"); } 
-		} else SynErr(190);
-		while (la.kind == 46 || la.kind == 48) {
+		} else SynErr(191);
+		while (la.kind == 50 || la.kind == 51) {
 			isFree = false; 
-			if (la.kind == 46) {
+			if (la.kind == 50) {
 				Get();
 				isFree = true; 
 			}
-			Expect(48);
-			Expression(out e, false);
+			Expect(51);
+			Expression(out e, false, true);
 			ens.Add(new MaybeFreeExpression(e, isFree)); 
 			Expect(8);
 			tok = t; 
 		}
-		if (la.kind == 9) {
+		if (la.kind == 13) {
 			BlockStmt(out block, out bodyStart, out bodyEnd);
 		}
 		if (DafnyOptions.O.DisallowSoundnessCheating && block == null && 0 < ens.Count) {
@@ -2105,7 +2154,7 @@ List<Expression/*!*/>/*!*/ decreases, ref Attributes decAttrs, ref Attributes mo
 		IToken opTok;
 		IToken danglingOperator = null;
 		
-		Expect(88);
+		Expect(89);
 		x = t; 
 		if (StartOf(24)) {
 			CalcOp(out opTok, out calcOp);
@@ -2116,9 +2165,9 @@ List<Expression/*!*/>/*!*/ decreases, ref Attributes decAttrs, ref Attributes mo
 			resOp = calcOp;
 			
 		}
-		Expect(9);
+		Expect(13);
 		while (StartOf(17)) {
-			Expression(out e, false);
+			Expression(out e, false, true);
 			lines.Add(e); stepOp = calcOp; danglingOperator = null; 
 			Expect(8);
 			if (StartOf(24)) {
@@ -2139,7 +2188,7 @@ List<Expression/*!*/>/*!*/ decreases, ref Attributes decAttrs, ref Attributes mo
 			if (h.Body.Count != 0) { danglingOperator = null; }
 			
 		}
-		Expect(10);
+		Expect(14);
 		if (danglingOperator != null) {
 		 SemErr(danglingOperator, "a calculation cannot end with an operator");
 		}
@@ -2158,7 +2207,7 @@ List<Expression/*!*/>/*!*/ decreases, ref Attributes decAttrs, ref Attributes mo
 		BlockStmt body = null;  IToken bodyStart;
 		IToken ellipsisToken = null;
 		
-		Expect(87);
+		Expect(88);
 		tok = t; 
 		while (IsAttribute()) {
 			Attribute(ref attrs);
@@ -2167,7 +2216,7 @@ List<Expression/*!*/>/*!*/ decreases, ref Attributes decAttrs, ref Attributes mo
 			if (StartOf(13)) {
 				FrameExpression(out fe);
 				mod.Add(fe); 
-				while (la.kind == 31) {
+				while (la.kind == 35) {
 					Get();
 					FrameExpression(out fe);
 					mod.Add(fe); 
@@ -2177,13 +2226,13 @@ List<Expression/*!*/>/*!*/ decreases, ref Attributes decAttrs, ref Attributes mo
 				ellipsisToken = t; 
 			}
 		}
-		if (la.kind == 9) {
+		if (la.kind == 13) {
 			BlockStmt(out body, out bodyStart, out endTok);
 		} else if (la.kind == 8) {
-			while (!(la.kind == 0 || la.kind == 8)) {SynErr(191); Get();}
+			while (!(la.kind == 0 || la.kind == 8)) {SynErr(192); Get();}
 			Get();
 			endTok = t; 
-		} else SynErr(192);
+		} else SynErr(193);
 		s = new ModifyStmt(tok, endTok, mod, attrs, body);
 		if (ellipsisToken != null) {
 		 s = new SkeletonStatement(s, ellipsisToken, null);
@@ -2197,17 +2246,17 @@ List<Expression/*!*/>/*!*/ decreases, ref Attributes decAttrs, ref Attributes mo
 		AssignmentRhs r;
 		bool isYield = false;
 		
-		if (la.kind == 70) {
+		if (la.kind == 72) {
 			Get();
 			returnTok = t; 
-		} else if (la.kind == 51) {
+		} else if (la.kind == 53) {
 			Get();
 			returnTok = t; isYield = true; 
-		} else SynErr(193);
+		} else SynErr(194);
 		if (StartOf(26)) {
 			Rhs(out r, null);
 			rhss = new List<AssignmentRhs>(); rhss.Add(r); 
-			while (la.kind == 31) {
+			while (la.kind == 35) {
 				Get();
 				Rhs(out r, null);
 				rhss.Add(r); 
@@ -2227,24 +2276,24 @@ List<Expression/*!*/>/*!*/ decreases, ref Attributes decAttrs, ref Attributes mo
 		List<Expression> exprs = null;
 		IToken tok, dotdotdot, whereTok;
 		Expression e; 
-		Expect(37);
+		Expect(41);
 		dotdotdot = t; 
-		if (la.kind == 68) {
+		if (la.kind == 70) {
 			Get();
 			names = new List<IToken>(); exprs = new List<Expression>(); whereTok = t;
 			Ident(out tok);
 			names.Add(tok); 
-			while (la.kind == 31) {
+			while (la.kind == 35) {
 				Get();
 				Ident(out tok);
 				names.Add(tok); 
 			}
-			Expect(69);
-			Expression(out e, false);
+			Expect(71);
+			Expression(out e, false, true);
 			exprs.Add(e); 
-			while (la.kind == 31) {
+			while (la.kind == 35) {
 				Get();
-				Expression(out e, false);
+				Expression(out e, false, true);
 				exprs.Add(e); 
 			}
 			if (exprs.Count != names.Count) {
@@ -2266,29 +2315,29 @@ List<Expression/*!*/>/*!*/ decreases, ref Attributes decAttrs, ref Attributes mo
 		r = dummyRhs;  // to please compiler
 		Attributes attrs = null;
 		
-		if (la.kind == 73) {
+		if (la.kind == 75) {
 			Get();
 			newToken = t; 
 			TypeAndToken(out x, out ty);
-			if (la.kind == 11 || la.kind == 61 || la.kind == 74) {
-				if (la.kind == 74) {
+			if (la.kind == 15 || la.kind == 63 || la.kind == 76) {
+				if (la.kind == 76) {
 					Get();
 					ee = new List<Expression>(); 
 					Expressions(ee);
-					Expect(75);
+					Expect(77);
 					var tmp = theBuiltIns.ArrayType(ee.Count, new IntType(), true);
 					
 				} else {
 					x = null; args = new List<Expression/*!*/>(); 
-					if (la.kind == 61) {
+					if (la.kind == 63) {
 						Get();
 						Ident(out x);
 					}
-					Expect(11);
+					Expect(15);
 					if (StartOf(17)) {
 						Expressions(args);
 					}
-					Expect(12);
+					Expect(16);
 				}
 			}
 			if (ee != null) {
@@ -2299,14 +2348,14 @@ List<Expression/*!*/>/*!*/ decreases, ref Attributes decAttrs, ref Attributes mo
 			 r = new TypeRhs(newToken, ty);
 			}
 			
-		} else if (la.kind == 13) {
+		} else if (la.kind == 17) {
 			Get();
 			r = new HavocRhs(t); 
 		} else if (StartOf(17)) {
-			Expression(out e, false);
+			Expression(out e, false, true);
 			r = new ExprRhs(e); 
-		} else SynErr(194);
-		while (la.kind == 9) {
+		} else SynErr(195);
+		while (la.kind == 13) {
 			Attribute(ref attrs);
 		}
 		r.Attributes = attrs; 
@@ -2316,26 +2365,27 @@ List<Expression/*!*/>/*!*/ decreases, ref Attributes decAttrs, ref Attributes mo
 		e = dummyExpr;  // the assignment is to please the compiler, the dummy value to satisfy contracts in the event of a parse error
 		
 		if (la.kind == 1) {
-			DottedIdentifiersAndFunction(out e);
-			while (la.kind == 61 || la.kind == 74) {
+			DottedIdentifiersAndFunction(out e, false, false);
+			while (la.kind == 63 || la.kind == 76) {
 				Suffix(ref e);
 			}
+			ApplySuffix(ref e);
 		} else if (StartOf(27)) {
-			ConstAtomExpression(out e);
+			ConstAtomExpression(out e, false, false);
 			Suffix(ref e);
-			while (la.kind == 61 || la.kind == 74) {
+			while (la.kind == 63 || la.kind == 76) {
 				Suffix(ref e);
 			}
-		} else SynErr(195);
+		} else SynErr(196);
 	}
 
 	void Expressions(List<Expression/*!*/>/*!*/ args) {
 		Contract.Requires(cce.NonNullElements(args)); Expression/*!*/ e; 
-		Expression(out e, true);
+		Expression(out e, true, true);
 		args.Add(e); 
-		while (la.kind == 31) {
+		while (la.kind == 35) {
 			Get();
-			Expression(out e, true);
+			Expression(out e, true, true);
 			args.Add(e); 
 		}
 	}
@@ -2346,36 +2396,36 @@ List<Expression/*!*/>/*!*/ decreases, ref Attributes decAttrs, ref Attributes mo
 		Expression e;
 		List<Statement> body;
 		
-		Expect(9);
-		while (la.kind == 78) {
+		Expect(13);
+		while (la.kind == 80) {
 			Get();
 			x = t; 
-			Expression(out e, true);
-			Expect(79);
+			Expression(out e, true, false);
+			Expect(9);
 			body = new List<Statement>(); 
 			while (StartOf(15)) {
 				Stmt(body);
 			}
 			alternatives.Add(new GuardedAlternative(x, e, body)); 
 		}
-		Expect(10);
+		Expect(14);
 		endTok = t; 
 	}
 
 	void Guard(out Expression e) {
 		Expression/*!*/ ee;  e = null; 
-		if (la.kind == 13) {
+		if (la.kind == 17) {
 			Get();
 			e = null; 
 		} else if (IsParenStar()) {
-			Expect(11);
-			Expect(13);
-			Expect(12);
+			Expect(15);
+			Expect(17);
+			Expect(16);
 			e = null; 
 		} else if (StartOf(17)) {
-			Expression(out ee, true);
+			Expression(out ee, true, true);
 			e = ee; 
-		} else SynErr(196);
+		} else SynErr(197);
 	}
 
 	void LoopSpec(out List<MaybeFreeExpression/*!*/> invariants, out List<Expression/*!*/> decreases, out List<FrameExpression/*!*/> mod, ref Attributes decAttrs, ref Attributes modAttrs) {
@@ -2386,22 +2436,22 @@ List<Expression/*!*/>/*!*/ decreases, ref Attributes decAttrs, ref Attributes mo
 		mod = null;
 		
 		while (StartOf(28)) {
-			if (la.kind == 46 || la.kind == 81) {
+			if (la.kind == 50 || la.kind == 82) {
 				Invariant(out invariant);
-				while (!(la.kind == 0 || la.kind == 8)) {SynErr(197); Get();}
+				while (!(la.kind == 0 || la.kind == 8)) {SynErr(198); Get();}
 				Expect(8);
 				invariants.Add(invariant); 
-			} else if (la.kind == 49) {
-				while (!(la.kind == 0 || la.kind == 49)) {SynErr(198); Get();}
+			} else if (la.kind == 52) {
+				while (!(la.kind == 0 || la.kind == 52)) {SynErr(199); Get();}
 				Get();
 				while (IsAttribute()) {
 					Attribute(ref decAttrs);
 				}
 				DecreasesList(decreases, true);
-				while (!(la.kind == 0 || la.kind == 8)) {SynErr(199); Get();}
+				while (!(la.kind == 0 || la.kind == 8)) {SynErr(200); Get();}
 				Expect(8);
 			} else {
-				while (!(la.kind == 0 || la.kind == 45)) {SynErr(200); Get();}
+				while (!(la.kind == 0 || la.kind == 49)) {SynErr(201); Get();}
 				Get();
 				while (IsAttribute()) {
 					Attribute(ref modAttrs);
@@ -2410,13 +2460,13 @@ List<Expression/*!*/>/*!*/ decreases, ref Attributes decAttrs, ref Attributes mo
 				if (StartOf(13)) {
 					FrameExpression(out fe);
 					mod.Add(fe); 
-					while (la.kind == 31) {
+					while (la.kind == 35) {
 						Get();
 						FrameExpression(out fe);
 						mod.Add(fe); 
 					}
 				}
-				while (!(la.kind == 0 || la.kind == 8)) {SynErr(201); Get();}
+				while (!(la.kind == 0 || la.kind == 8)) {SynErr(202); Get();}
 				Expect(8);
 			}
 		}
@@ -2424,16 +2474,16 @@ List<Expression/*!*/>/*!*/ decreases, ref Attributes decAttrs, ref Attributes mo
 
 	void Invariant(out MaybeFreeExpression/*!*/ invariant) {
 		bool isFree = false; Expression/*!*/ e; List<string> ids = new List<string>(); invariant = null; Attributes attrs = null; 
-		while (!(la.kind == 0 || la.kind == 46 || la.kind == 81)) {SynErr(202); Get();}
-		if (la.kind == 46) {
+		while (!(la.kind == 0 || la.kind == 50 || la.kind == 82)) {SynErr(203); Get();}
+		if (la.kind == 50) {
 			Get();
 			isFree = true; 
 		}
-		Expect(81);
+		Expect(82);
 		while (IsAttribute()) {
 			Attribute(ref attrs);
 		}
-		Expression(out e, false);
+		Expression(out e, false, true);
 		invariant = new MaybeFreeExpression(e, isFree, attrs); 
 	}
 
@@ -2444,21 +2494,21 @@ List<Expression/*!*/>/*!*/ decreases, ref Attributes decAttrs, ref Attributes mo
 		BoundVar/*!*/ bv;
 		List<Statement/*!*/> body = new List<Statement/*!*/>();
 		
-		Expect(78);
+		Expect(80);
 		x = t; 
 		Ident(out id);
-		if (la.kind == 11) {
+		if (la.kind == 15) {
 			Get();
 			IdentTypeOptional(out bv);
 			arguments.Add(bv); 
-			while (la.kind == 31) {
+			while (la.kind == 35) {
 				Get();
 				IdentTypeOptional(out bv);
 				arguments.Add(bv); 
 			}
-			Expect(12);
+			Expect(16);
 		}
-		Expect(79);
+		Expect(9);
 		while (StartOf(15)) {
 			Stmt(body);
 		}
@@ -2471,9 +2521,9 @@ List<Expression/*!*/>/*!*/ decreases, ref Attributes decAttrs, ref Attributes mo
 			Get();
 			arg = new Attributes.Argument(t, t.val.Substring(1, t.val.Length-2)); 
 		} else if (StartOf(17)) {
-			Expression(out e, allowSemi);
+			Expression(out e, allowSemi, true);
 			arg = new Attributes.Argument(t, e); 
-		} else SynErr(203);
+		} else SynErr(204);
 	}
 
 	void QuantifierDomain(out List<BoundVar> bvars, out Attributes attrs, out Expression range) {
@@ -2484,7 +2534,7 @@ List<Expression/*!*/>/*!*/ decreases, ref Attributes decAttrs, ref Attributes mo
 		
 		IdentTypeOptional(out bv);
 		bvars.Add(bv); 
-		while (la.kind == 31) {
+		while (la.kind == 35) {
 			Get();
 			IdentTypeOptional(out bv);
 			bvars.Add(bv); 
@@ -2492,9 +2542,9 @@ List<Expression/*!*/>/*!*/ decreases, ref Attributes decAttrs, ref Attributes mo
 		while (IsAttribute()) {
 			Attribute(ref attrs);
 		}
-		if (la.kind == 29) {
+		if (la.kind == 33) {
 			Get();
-			Expression(out range, true);
+			Expression(out range, true, true);
 		}
 	}
 
@@ -2504,40 +2554,35 @@ List<Expression/*!*/>/*!*/ decreases, ref Attributes decAttrs, ref Attributes mo
 		x = null;
 		
 		switch (la.kind) {
-		case 33: {
+		case 37: {
 			Get();
 			x = t;  binOp = BinaryExpr.Opcode.Eq; 
-			if (la.kind == 89) {
+			if (la.kind == 90) {
 				Get();
-				Expect(74);
-				Expression(out k, true);
-				Expect(75);
+				Expect(76);
+				Expression(out k, true, true);
+				Expect(77);
 			}
 			break;
 		}
-		case 38: {
+		case 42: {
 			Get();
 			x = t;  binOp = BinaryExpr.Opcode.Lt; 
 			break;
 		}
-		case 39: {
+		case 43: {
 			Get();
 			x = t;  binOp = BinaryExpr.Opcode.Gt; 
 			break;
 		}
-		case 90: {
+		case 91: {
 			Get();
 			x = t;  binOp = BinaryExpr.Opcode.Le; 
 			break;
 		}
-		case 91: {
-			Get();
-			x = t;  binOp = BinaryExpr.Opcode.Ge; 
-			break;
-		}
 		case 92: {
 			Get();
-			x = t;  binOp = BinaryExpr.Opcode.Neq; 
+			x = t;  binOp = BinaryExpr.Opcode.Ge; 
 			break;
 		}
 		case 93: {
@@ -2547,30 +2592,35 @@ List<Expression/*!*/>/*!*/ decreases, ref Attributes decAttrs, ref Attributes mo
 		}
 		case 94: {
 			Get();
-			x = t;  binOp = BinaryExpr.Opcode.Le; 
+			x = t;  binOp = BinaryExpr.Opcode.Neq; 
 			break;
 		}
 		case 95: {
 			Get();
+			x = t;  binOp = BinaryExpr.Opcode.Le; 
+			break;
+		}
+		case 96: {
+			Get();
 			x = t;  binOp = BinaryExpr.Opcode.Ge; 
 			break;
 		}
-		case 96: case 97: {
+		case 97: case 98: {
 			EquivOp();
 			x = t;  binOp = BinaryExpr.Opcode.Iff; 
 			break;
 		}
-		case 98: case 99: {
+		case 99: case 100: {
 			ImpliesOp();
 			x = t;  binOp = BinaryExpr.Opcode.Imp; 
 			break;
 		}
-		case 100: case 101: {
+		case 101: case 102: {
 			ExpliesOp();
 			x = t;  binOp = BinaryExpr.Opcode.Exp; 
 			break;
 		}
-		default: SynErr(204); break;
+		default: SynErr(205); break;
 		}
 		if (k == null) {
 		 op = new Microsoft.Dafny.CalcStmt.BinaryCalcOp(binOp);
@@ -2589,8 +2639,8 @@ List<Expression/*!*/>/*!*/ decreases, ref Attributes decAttrs, ref Attributes mo
 		Token x = la;
 		IToken endTok = x;
 		
-		while (la.kind == 9 || la.kind == 88) {
-			if (la.kind == 9) {
+		while (la.kind == 13 || la.kind == 89) {
+			if (la.kind == 13) {
 				BlockStmt(out block, out bodyStart, out bodyEnd);
 				endTok = block.EndTok; subhints.Add(block); 
 			} else {
@@ -2603,106 +2653,106 @@ List<Expression/*!*/>/*!*/ decreases, ref Attributes decAttrs, ref Attributes mo
 	}
 
 	void EquivOp() {
-		if (la.kind == 96) {
+		if (la.kind == 97) {
 			Get();
-		} else if (la.kind == 97) {
-			Get();
-		} else SynErr(205);
-	}
-
-	void ImpliesOp() {
-		if (la.kind == 98) {
-			Get();
-		} else if (la.kind == 99) {
+		} else if (la.kind == 98) {
 			Get();
 		} else SynErr(206);
 	}
 
-	void ExpliesOp() {
-		if (la.kind == 100) {
+	void ImpliesOp() {
+		if (la.kind == 99) {
 			Get();
-		} else if (la.kind == 101) {
+		} else if (la.kind == 100) {
 			Get();
 		} else SynErr(207);
 	}
 
-	void EquivExpression(out Expression e0, bool allowSemi) {
+	void ExpliesOp() {
+		if (la.kind == 101) {
+			Get();
+		} else if (la.kind == 102) {
+			Get();
+		} else SynErr(208);
+	}
+
+	void EquivExpression(out Expression e0, bool allowSemi, bool allowLambda) {
 		Contract.Ensures(Contract.ValueAtReturn(out e0) != null); IToken/*!*/ x;  Expression/*!*/ e1; 
-		ImpliesExpliesExpression(out e0, allowSemi);
-		while (la.kind == 96 || la.kind == 97) {
+		ImpliesExpliesExpression(out e0, allowSemi, allowLambda);
+		while (la.kind == 97 || la.kind == 98) {
 			EquivOp();
 			x = t; 
-			ImpliesExpliesExpression(out e1, allowSemi);
+			ImpliesExpliesExpression(out e1, allowSemi, allowLambda);
 			e0 = new BinaryExpr(x, BinaryExpr.Opcode.Iff, e0, e1); 
 		}
 	}
 
-	void ImpliesExpliesExpression(out Expression e0, bool allowSemi) {
+	void ImpliesExpliesExpression(out Expression e0, bool allowSemi, bool allowLambda) {
 		Contract.Ensures(Contract.ValueAtReturn(out e0) != null); IToken/*!*/ x;  Expression/*!*/ e1; 
-		LogicalExpression(out e0, allowSemi);
+		LogicalExpression(out e0, allowSemi, allowLambda);
 		if (StartOf(29)) {
-			if (la.kind == 98 || la.kind == 99) {
+			if (la.kind == 99 || la.kind == 100) {
 				ImpliesOp();
 				x = t; 
-				ImpliesExpression(out e1, allowSemi);
+				ImpliesExpression(out e1, allowSemi, allowLambda);
 				e0 = new BinaryExpr(x, BinaryExpr.Opcode.Imp, e0, e1); 
 			} else {
 				ExpliesOp();
 				x = t; 
-				LogicalExpression(out e1, allowSemi);
+				LogicalExpression(out e1, allowSemi, allowLambda);
 				e0 = new BinaryExpr(x, BinaryExpr.Opcode.Exp, e0, e1); 
-				while (la.kind == 100 || la.kind == 101) {
+				while (la.kind == 101 || la.kind == 102) {
 					ExpliesOp();
 					x = t; 
-					LogicalExpression(out e1, allowSemi);
+					LogicalExpression(out e1, allowSemi, allowLambda);
 					e0 = new BinaryExpr(x, BinaryExpr.Opcode.Exp, e0, e1); 
 				}
 			}
 		}
 	}
 
-	void LogicalExpression(out Expression e0, bool allowSemi) {
+	void LogicalExpression(out Expression e0, bool allowSemi, bool allowLambda) {
 		Contract.Ensures(Contract.ValueAtReturn(out e0) != null); IToken/*!*/ x;  Expression/*!*/ e1; 
-		RelationalExpression(out e0, allowSemi);
+		RelationalExpression(out e0, allowSemi, allowLambda);
 		if (StartOf(30)) {
-			if (la.kind == 102 || la.kind == 103) {
+			if (la.kind == 103 || la.kind == 104) {
 				AndOp();
 				x = t; 
-				RelationalExpression(out e1, allowSemi);
+				RelationalExpression(out e1, allowSemi, allowLambda);
 				e0 = new BinaryExpr(x, BinaryExpr.Opcode.And, e0, e1); 
-				while (la.kind == 102 || la.kind == 103) {
+				while (la.kind == 103 || la.kind == 104) {
 					AndOp();
 					x = t; 
-					RelationalExpression(out e1, allowSemi);
+					RelationalExpression(out e1, allowSemi, allowLambda);
 					e0 = new BinaryExpr(x, BinaryExpr.Opcode.And, e0, e1); 
 				}
 			} else {
 				OrOp();
 				x = t; 
-				RelationalExpression(out e1, allowSemi);
+				RelationalExpression(out e1, allowSemi, allowLambda);
 				e0 = new BinaryExpr(x, BinaryExpr.Opcode.Or, e0, e1); 
-				while (la.kind == 104 || la.kind == 105) {
+				while (la.kind == 105 || la.kind == 106) {
 					OrOp();
 					x = t; 
-					RelationalExpression(out e1, allowSemi);
+					RelationalExpression(out e1, allowSemi, allowLambda);
 					e0 = new BinaryExpr(x, BinaryExpr.Opcode.Or, e0, e1); 
 				}
 			}
 		}
 	}
 
-	void ImpliesExpression(out Expression e0, bool allowSemi) {
+	void ImpliesExpression(out Expression e0, bool allowSemi, bool allowLambda) {
 		Contract.Ensures(Contract.ValueAtReturn(out e0) != null); IToken/*!*/ x;  Expression/*!*/ e1; 
-		LogicalExpression(out e0, allowSemi);
-		if (la.kind == 98 || la.kind == 99) {
+		LogicalExpression(out e0, allowSemi, allowLambda);
+		if (la.kind == 99 || la.kind == 100) {
 			ImpliesOp();
 			x = t; 
-			ImpliesExpression(out e1, allowSemi);
+			ImpliesExpression(out e1, allowSemi, allowLambda);
 			e0 = new BinaryExpr(x, BinaryExpr.Opcode.Imp, e0, e1); 
 		}
 	}
 
-	void RelationalExpression(out Expression e, bool allowSemi) {
+	void RelationalExpression(out Expression e, bool allowSemi, bool allowLambda) {
 		Contract.Ensures(Contract.ValueAtReturn(out e) != null);
 		IToken x, firstOpTok = null;  Expression e0, e1, acc = null;  BinaryExpr.Opcode op;
 		List<Expression> chain = null;
@@ -2716,12 +2766,12 @@ List<Expression/*!*/>/*!*/ decreases, ref Attributes decAttrs, ref Attributes mo
 		              // 4 ("disjoint")    indicates chain of disjoint set operators
 		bool hasSeenNeq = false;
 		
-		Term(out e0, allowSemi);
+		Term(out e0, allowSemi, allowLambda);
 		e = e0; 
 		if (StartOf(31)) {
 			RelOp(out x, out op, out k);
 			firstOpTok = x; 
-			Term(out e1, allowSemi);
+			Term(out e1, allowSemi, allowLambda);
 			if (k == null) {
 			 e = new BinaryExpr(x, op, e0, e1);
 			 if (op == BinaryExpr.Opcode.Disjoint)
@@ -2783,7 +2833,7 @@ List<Expression/*!*/>/*!*/ decreases, ref Attributes decAttrs, ref Attributes mo
 				   kind = 3;  break;
 				}
 				
-				Term(out e1, allowSemi);
+				Term(out e1, allowSemi, allowLambda);
 				ops.Add(op); prefixLimits.Add(k); chain.Add(e1);
 				if (k != null) {
 				 Contract.Assert(op == BinaryExpr.Opcode.Eq || op == BinaryExpr.Opcode.Neq);
@@ -2804,27 +2854,27 @@ List<Expression/*!*/>/*!*/ decreases, ref Attributes decAttrs, ref Attributes mo
 	}
 
 	void AndOp() {
-		if (la.kind == 102) {
+		if (la.kind == 103) {
 			Get();
-		} else if (la.kind == 103) {
-			Get();
-		} else SynErr(208);
-	}
-
-	void OrOp() {
-		if (la.kind == 104) {
-			Get();
-		} else if (la.kind == 105) {
+		} else if (la.kind == 104) {
 			Get();
 		} else SynErr(209);
 	}
 
-	void Term(out Expression e0, bool allowSemi) {
+	void OrOp() {
+		if (la.kind == 105) {
+			Get();
+		} else if (la.kind == 106) {
+			Get();
+		} else SynErr(210);
+	}
+
+	void Term(out Expression e0, bool allowSemi, bool allowLambda) {
 		Contract.Ensures(Contract.ValueAtReturn(out e0) != null); IToken/*!*/ x;  Expression/*!*/ e1;  BinaryExpr.Opcode op; 
-		Factor(out e0, allowSemi);
-		while (la.kind == 108 || la.kind == 109) {
+		Factor(out e0, allowSemi, allowLambda);
+		while (la.kind == 109 || la.kind == 110) {
 			AddOp(out x, out op);
-			Factor(out e1, allowSemi);
+			Factor(out e1, allowSemi, allowLambda);
 			e0 = new BinaryExpr(x, op, e0, e1); 
 		}
 	}
@@ -2836,62 +2886,62 @@ List<Expression/*!*/>/*!*/ decreases, ref Attributes decAttrs, ref Attributes mo
 		k = null;
 		
 		switch (la.kind) {
-		case 33: {
+		case 37: {
 			Get();
 			x = t;  op = BinaryExpr.Opcode.Eq; 
-			if (la.kind == 89) {
+			if (la.kind == 90) {
 				Get();
-				Expect(74);
-				Expression(out k, true);
-				Expect(75);
+				Expect(76);
+				Expression(out k, true, true);
+				Expect(77);
 			}
 			break;
 		}
-		case 38: {
+		case 42: {
 			Get();
 			x = t;  op = BinaryExpr.Opcode.Lt; 
 			break;
 		}
-		case 39: {
+		case 43: {
 			Get();
 			x = t;  op = BinaryExpr.Opcode.Gt; 
 			break;
 		}
-		case 90: {
+		case 91: {
 			Get();
 			x = t;  op = BinaryExpr.Opcode.Le; 
 			break;
 		}
-		case 91: {
+		case 92: {
 			Get();
 			x = t;  op = BinaryExpr.Opcode.Ge; 
 			break;
 		}
-		case 92: {
+		case 93: {
 			Get();
 			x = t;  op = BinaryExpr.Opcode.Neq; 
-			if (la.kind == 89) {
+			if (la.kind == 90) {
 				Get();
-				Expect(74);
-				Expression(out k, true);
-				Expect(75);
+				Expect(76);
+				Expression(out k, true, true);
+				Expect(77);
 			}
-			break;
-		}
-		case 106: {
-			Get();
-			x = t;  op = BinaryExpr.Opcode.In; 
-			break;
-		}
-		case 14: {
-			Get();
-			x = t;  op = BinaryExpr.Opcode.NotIn; 
 			break;
 		}
 		case 107: {
 			Get();
+			x = t;  op = BinaryExpr.Opcode.In; 
+			break;
+		}
+		case 18: {
+			Get();
+			x = t;  op = BinaryExpr.Opcode.NotIn; 
+			break;
+		}
+		case 108: {
+			Get();
 			x = t;  y = Token.NoToken; 
-			if (la.kind == 107) {
+			if (la.kind == 108) {
 				Get();
 				y = t; 
 			}
@@ -2906,215 +2956,243 @@ List<Expression/*!*/>/*!*/ decreases, ref Attributes decAttrs, ref Attributes mo
 			
 			break;
 		}
-		case 93: {
+		case 94: {
 			Get();
 			x = t;  op = BinaryExpr.Opcode.Neq; 
 			break;
 		}
-		case 94: {
+		case 95: {
 			Get();
 			x = t;  op = BinaryExpr.Opcode.Le; 
 			break;
 		}
-		case 95: {
+		case 96: {
 			Get();
 			x = t;  op = BinaryExpr.Opcode.Ge; 
 			break;
 		}
-		default: SynErr(210); break;
+		default: SynErr(211); break;
 		}
 	}
 
-	void Factor(out Expression e0, bool allowSemi) {
+	void Factor(out Expression e0, bool allowSemi, bool allowLambda) {
 		Contract.Ensures(Contract.ValueAtReturn(out e0) != null); IToken/*!*/ x;  Expression/*!*/ e1;  BinaryExpr.Opcode op; 
-		UnaryExpression(out e0, allowSemi);
-		while (la.kind == 13 || la.kind == 110 || la.kind == 111) {
+		UnaryExpression(out e0, allowSemi, allowLambda);
+		while (la.kind == 17 || la.kind == 111 || la.kind == 112) {
 			MulOp(out x, out op);
-			UnaryExpression(out e1, allowSemi);
+			UnaryExpression(out e1, allowSemi, allowLambda);
 			e0 = new BinaryExpr(x, op, e0, e1); 
 		}
 	}
 
 	void AddOp(out IToken x, out BinaryExpr.Opcode op) {
 		Contract.Ensures(Contract.ValueAtReturn(out x) != null); x = Token.NoToken;  op=BinaryExpr.Opcode.Add/*(dummy)*/; 
-		if (la.kind == 108) {
+		if (la.kind == 109) {
 			Get();
 			x = t;  op = BinaryExpr.Opcode.Add; 
-		} else if (la.kind == 109) {
+		} else if (la.kind == 110) {
 			Get();
 			x = t;  op = BinaryExpr.Opcode.Sub; 
-		} else SynErr(211);
+		} else SynErr(212);
 	}
 
-	void UnaryExpression(out Expression e, bool allowSemi) {
+	void UnaryExpression(out Expression e, bool allowSemi, bool allowLambda) {
 		Contract.Ensures(Contract.ValueAtReturn(out e) != null); IToken/*!*/ x;  e = dummyExpr; 
 		switch (la.kind) {
-		case 109: {
+		case 110: {
 			Get();
 			x = t; 
-			UnaryExpression(out e, allowSemi);
+			UnaryExpression(out e, allowSemi, allowLambda);
 			e = new NegationExpression(x, e); 
 			break;
 		}
-		case 107: case 112: {
+		case 108: case 113: {
 			NegOp();
 			x = t; 
-			UnaryExpression(out e, allowSemi);
+			UnaryExpression(out e, allowSemi, allowLambda);
 			e = new UnaryOpExpr(x, UnaryOpExpr.Opcode.Not, e); 
 			break;
 		}
-		case 25: case 30: case 56: case 66: case 72: case 76: case 82: case 83: case 85: case 88: case 121: case 122: case 123: {
-			EndlessExpression(out e, allowSemi);
+		case 29: case 34: case 58: case 68: case 74: case 78: case 83: case 84: case 86: case 89: case 122: case 123: case 124: {
+			EndlessExpression(out e, allowSemi, allowLambda);
 			break;
 		}
 		case 1: {
-			DottedIdentifiersAndFunction(out e);
-			while (la.kind == 61 || la.kind == 74) {
+			DottedIdentifiersAndFunction(out e, allowSemi, allowLambda);
+			while (la.kind == 63 || la.kind == 76) {
 				Suffix(ref e);
 			}
+			ApplySuffix(ref e);
 			break;
 		}
-		case 9: case 74: {
+		case 13: case 76: {
 			DisplayExpr(out e);
-			while (la.kind == 61 || la.kind == 74) {
-				Suffix(ref e);
-			}
-			break;
-		}
-		case 57: {
-			MultiSetExpr(out e);
-			while (la.kind == 61 || la.kind == 74) {
+			while (la.kind == 63 || la.kind == 76) {
 				Suffix(ref e);
 			}
 			break;
 		}
 		case 59: {
+			MultiSetExpr(out e);
+			while (la.kind == 63 || la.kind == 76) {
+				Suffix(ref e);
+			}
+			break;
+		}
+		case 61: {
 			Get();
 			x = t; 
-			if (la.kind == 74) {
+			if (la.kind == 76) {
 				MapDisplayExpr(x, out e);
-				while (la.kind == 61 || la.kind == 74) {
+				while (la.kind == 63 || la.kind == 76) {
 					Suffix(ref e);
 				}
 			} else if (la.kind == 1) {
 				MapComprehensionExpr(x, out e, allowSemi);
 			} else if (StartOf(32)) {
 				SemErr("map must be followed by literal in brackets or comprehension."); 
-			} else SynErr(212);
+			} else SynErr(213);
 			break;
 		}
-		case 2: case 3: case 4: case 11: case 29: case 54: case 55: case 113: case 114: case 115: case 116: case 117: case 118: {
-			ConstAtomExpression(out e);
-			while (la.kind == 61 || la.kind == 74) {
+		case 2: case 3: case 4: case 15: case 33: case 56: case 57: case 114: case 115: case 116: case 117: case 118: case 119: {
+			ConstAtomExpression(out e, allowSemi, allowLambda);
+			while (la.kind == 63 || la.kind == 76) {
 				Suffix(ref e);
 			}
 			break;
 		}
-		default: SynErr(213); break;
+		default: SynErr(214); break;
 		}
 	}
 
 	void MulOp(out IToken x, out BinaryExpr.Opcode op) {
 		Contract.Ensures(Contract.ValueAtReturn(out x) != null); x = Token.NoToken;  op = BinaryExpr.Opcode.Add/*(dummy)*/; 
-		if (la.kind == 13) {
+		if (la.kind == 17) {
 			Get();
 			x = t;  op = BinaryExpr.Opcode.Mul; 
-		} else if (la.kind == 110) {
-			Get();
-			x = t;  op = BinaryExpr.Opcode.Div; 
 		} else if (la.kind == 111) {
 			Get();
-			x = t;  op = BinaryExpr.Opcode.Mod; 
-		} else SynErr(214);
-	}
-
-	void NegOp() {
-		if (la.kind == 107) {
-			Get();
+			x = t;  op = BinaryExpr.Opcode.Div; 
 		} else if (la.kind == 112) {
 			Get();
+			x = t;  op = BinaryExpr.Opcode.Mod; 
 		} else SynErr(215);
 	}
 
-	void EndlessExpression(out Expression e, bool allowSemi) {
+	void NegOp() {
+		if (la.kind == 108) {
+			Get();
+		} else if (la.kind == 113) {
+			Get();
+		} else SynErr(216);
+	}
+
+	void EndlessExpression(out Expression e, bool allowSemi, bool allowLambda) {
 		IToken/*!*/ x;
 		Expression e0, e1;
 		Statement s;
 		e = dummyExpr;
 		
 		switch (la.kind) {
-		case 76: {
+		case 78: {
 			Get();
 			x = t; 
-			Expression(out e, true);
-			Expect(119);
-			Expression(out e0, true);
-			Expect(77);
-			Expression(out e1, allowSemi);
+			Expression(out e, true, true);
+			Expect(120);
+			Expression(out e0, true, true);
+			Expect(79);
+			Expression(out e1, allowSemi, allowLambda);
 			e = new ITEExpr(x, e, e0, e1); 
 			break;
 		}
-		case 82: {
-			MatchExpression(out e, allowSemi);
+		case 83: {
+			MatchExpression(out e, allowSemi, allowLambda);
 			break;
 		}
-		case 85: case 121: case 122: case 123: {
-			QuantifierGuts(out e, allowSemi);
+		case 86: case 122: case 123: case 124: {
+			QuantifierGuts(out e, allowSemi, allowLambda);
 			break;
 		}
-		case 56: {
-			ComprehensionExpr(out e, allowSemi);
+		case 58: {
+			ComprehensionExpr(out e, allowSemi, allowLambda);
 			break;
 		}
-		case 72: case 83: case 88: {
+		case 74: case 84: case 89: {
 			StmtInExpr(out s);
-			Expression(out e, allowSemi);
+			Expression(out e, allowSemi, allowLambda);
 			e = new StmtExpr(s.Tok, s, e); 
 			break;
 		}
-		case 25: case 30: {
-			LetExpr(out e, allowSemi);
+		case 29: case 34: {
+			LetExpr(out e, allowSemi, allowLambda);
 			break;
 		}
-		case 66: {
-			NamedExpr(out e, allowSemi);
+		case 68: {
+			NamedExpr(out e, allowSemi, allowLambda);
 			break;
 		}
-		default: SynErr(216); break;
+		default: SynErr(217); break;
 		}
 	}
 
-	void DottedIdentifiersAndFunction(out Expression e) {
+	void DottedIdentifiersAndFunction(out Expression e, bool allowSemi, bool allowLambda) {
 		IToken id, idPrime;  IToken openParen = null;
 		List<Expression> args = null;
 		List<IToken> idents = new List<IToken>();
+		e = null;
+		var applyArgLists = new List<List<Expression>>();
 		
 		Ident(out id);
 		idents.Add(id); 
-		while (la.kind == 61) {
+		while (la.kind == 63) {
 			IdentOrDigitsSuffix(out id, out idPrime);
 			idents.Add(id);
 			if (idPrime != null) { idents.Add(idPrime); id = idPrime; }
 			
 		}
-		if (la.kind == 11 || la.kind == 89) {
+		if (la.kind == 15 || la.kind == 90) {
 			args = new List<Expression>(); 
-			if (la.kind == 89) {
+			if (la.kind == 90) {
 				Get();
 				id.val = id.val + "#";  Expression k; 
-				Expect(74);
-				Expression(out k, true);
-				Expect(75);
+				Expect(76);
+				Expression(out k, true, true);
+				Expect(77);
 				args.Add(k); 
 			}
-			Expect(11);
+			Expect(15);
 			openParen = t; 
 			if (StartOf(17)) {
 				Expressions(args);
 			}
-			Expect(12);
+			Expect(16);
 		}
-		e = new IdentifierSequence(idents, openParen, args); 
+		if (IsLambda(allowLambda)) {
+			Expression body = null;
+			Expression req = null;
+			bool oneShot;
+			var reads = new List<FrameExpression>();
+			
+			LambdaSpec(out req, reads);
+			LambdaArrow(out oneShot);
+			Expression(out body, allowSemi, true);
+			if (idents.Count != 1) {
+			 SemErr(id, "Invalid variable binding in lambda.");
+			}
+			if (args != null) {
+			 SemErr(openParen, "Expected variable binding.");
+			}
+			BoundVar bv = new BoundVar(id, id.val,  new InferredTypeProxy());
+			e = new LambdaExpr(id, oneShot, new List<BoundVar>{ bv }, req, reads, body);
+			
+		}
+		if (e == null) {
+		 e = new IdentifierSequence(idents, openParen, args);
+		 foreach (var args_ in applyArgLists) {
+		   e = new ApplyExpr(id, openParen, e, args_);
+		 }
+		}
+		
 	}
 
 	void Suffix(ref Expression e) {
@@ -3123,7 +3201,7 @@ List<Expression/*!*/>/*!*/ decreases, ref Attributes decAttrs, ref Attributes mo
 		List<Expression> multipleIndices = null;
 		bool func = false;
 		
-		if (la.kind == 61) {
+		if (la.kind == 63) {
 			IdentOrDigitsSuffix(out id, out x);
 			if (x != null) {
 			 // process id as a Suffix in its own right
@@ -3131,43 +3209,43 @@ List<Expression/*!*/>/*!*/ decreases, ref Attributes decAttrs, ref Attributes mo
 			 id = x;  // move to the next Suffix
 			}
 			
-			if (la.kind == 11 || la.kind == 89) {
+			if (la.kind == 15 || la.kind == 90) {
 				args = new List<Expression/*!*/>();  func = true; 
-				if (la.kind == 89) {
+				if (la.kind == 90) {
 					Get();
 					id.val = id.val + "#";  Expression k; 
-					Expect(74);
-					Expression(out k, true);
-					Expect(75);
+					Expect(76);
+					Expression(out k, true, true);
+					Expect(77);
 					args.Add(k); 
 				}
-				Expect(11);
+				Expect(15);
 				IToken openParen = t; 
 				if (StartOf(17)) {
 					Expressions(args);
 				}
-				Expect(12);
+				Expect(16);
 				e = new FunctionCallExpr(id, id.val, e, openParen, args); 
 			}
 			if (!func) { e = new ExprDotName(id, e, id.val); } 
-		} else if (la.kind == 74) {
+		} else if (la.kind == 76) {
 			Get();
 			x = t; 
 			if (StartOf(17)) {
-				Expression(out ee, true);
+				Expression(out ee, true, true);
 				e0 = ee; 
-				if (la.kind == 120) {
+				if (la.kind == 121) {
 					Get();
 					anyDots = true; 
 					if (StartOf(17)) {
-						Expression(out ee, true);
+						Expression(out ee, true, true);
 						e1 = ee; 
 					}
-				} else if (la.kind == 69) {
+				} else if (la.kind == 71) {
 					Get();
-					Expression(out ee, true);
+					Expression(out ee, true, true);
 					e1 = ee; 
-				} else if (la.kind == 7 || la.kind == 75) {
+				} else if (la.kind == 7 || la.kind == 77) {
 					while (la.kind == 7) {
 						Get();
 						if (multipleLengths == null) {
@@ -3177,32 +3255,32 @@ List<Expression/*!*/>/*!*/ decreases, ref Attributes decAttrs, ref Attributes mo
 						takeRest = true;
 						
 						if (StartOf(17)) {
-							Expression(out ee, true);
+							Expression(out ee, true, true);
 							multipleLengths.Add(ee);
 							takeRest = false;
 							
 						}
 					}
-				} else if (la.kind == 31 || la.kind == 75) {
-					while (la.kind == 31) {
+				} else if (la.kind == 35 || la.kind == 77) {
+					while (la.kind == 35) {
 						Get();
-						Expression(out ee, true);
+						Expression(out ee, true, true);
 						if (multipleIndices == null) {
-						 multipleIndices = new List<Expression>();
-						 multipleIndices.Add(e0);
+						multipleIndices = new List<Expression>();
+						multipleIndices.Add(e0);
 						}
 						multipleIndices.Add(ee);
 						
 					}
-				} else SynErr(217);
-			} else if (la.kind == 120) {
+				} else SynErr(218);
+			} else if (la.kind == 121) {
 				Get();
 				anyDots = true; 
 				if (StartOf(17)) {
-					Expression(out ee, true);
+					Expression(out ee, true, true);
 					e1 = ee; 
 				}
-			} else SynErr(218);
+			} else SynErr(219);
 			if (multipleIndices != null) {
 			 e = new MultiSelectExpr(x, e, multipleIndices);
 			 // make sure an array class with this dimensionality exists
@@ -3242,8 +3320,21 @@ List<Expression/*!*/>/*!*/ decreases, ref Attributes decAttrs, ref Attributes mo
 			 }
 			}
 			
-			Expect(75);
-		} else SynErr(219);
+			Expect(77);
+		} else SynErr(220);
+		ApplySuffix(ref e);
+	}
+
+	void ApplySuffix(ref Expression e) {
+		while (la.kind == 15) {
+			Get();
+			IToken openParen = t; var args = new List<Expression>(); 
+			if (StartOf(17)) {
+				Expressions(args);
+			}
+			Expect(16);
+			e = new ApplyExpr(e.tok, openParen, e, args); 
+		}
 	}
 
 	void DisplayExpr(out Expression e) {
@@ -3251,23 +3342,23 @@ List<Expression/*!*/>/*!*/ decreases, ref Attributes decAttrs, ref Attributes mo
 		IToken/*!*/ x = null;  List<Expression/*!*/>/*!*/ elements;
 		e = dummyExpr;
 		
-		if (la.kind == 9) {
+		if (la.kind == 13) {
 			Get();
 			x = t;  elements = new List<Expression/*!*/>(); 
 			if (StartOf(17)) {
 				Expressions(elements);
 			}
 			e = new SetDisplayExpr(x, elements);
-			Expect(10);
-		} else if (la.kind == 74) {
+			Expect(14);
+		} else if (la.kind == 76) {
 			Get();
 			x = t;  elements = new List<Expression/*!*/>(); 
 			if (StartOf(17)) {
 				Expressions(elements);
 			}
 			e = new SeqDisplayExpr(x, elements); 
-			Expect(75);
-		} else SynErr(220);
+			Expect(77);
+		} else SynErr(221);
 	}
 
 	void MultiSetExpr(out Expression e) {
@@ -3275,25 +3366,25 @@ List<Expression/*!*/>/*!*/ decreases, ref Attributes decAttrs, ref Attributes mo
 		IToken/*!*/ x = null;  List<Expression/*!*/>/*!*/ elements;
 		e = dummyExpr;
 		
-		Expect(57);
+		Expect(59);
 		x = t; 
-		if (la.kind == 9) {
+		if (la.kind == 13) {
 			Get();
 			elements = new List<Expression/*!*/>(); 
 			if (StartOf(17)) {
 				Expressions(elements);
 			}
 			e = new MultiSetDisplayExpr(x, elements);
-			Expect(10);
-		} else if (la.kind == 11) {
+			Expect(14);
+		} else if (la.kind == 15) {
 			Get();
 			x = t;  elements = new List<Expression/*!*/>(); 
-			Expression(out e, true);
+			Expression(out e, true, true);
 			e = new MultiSetFormingExpr(x, e); 
-			Expect(12);
-		} else if (StartOf(33)) {
+			Expect(16);
+		} else if (StartOf(32)) {
 			SemErr("multiset must be followed by multiset literal or expression to coerce in parentheses."); 
-		} else SynErr(221);
+		} else SynErr(222);
 	}
 
 	void MapDisplayExpr(IToken/*!*/ mapToken, out Expression e) {
@@ -3301,12 +3392,12 @@ List<Expression/*!*/>/*!*/ decreases, ref Attributes decAttrs, ref Attributes mo
 		List<ExpressionPair/*!*/>/*!*/ elements= new List<ExpressionPair/*!*/>() ;
 		e = dummyExpr;
 		
-		Expect(74);
+		Expect(76);
 		if (StartOf(17)) {
 			MapLiteralExpressions(out elements);
 		}
 		e = new MapDisplayExpr(mapToken, elements);
-		Expect(75);
+		Expect(77);
 	}
 
 	void MapComprehensionExpr(IToken mapToken, out Expression e, bool allowSemi) {
@@ -3318,33 +3409,33 @@ List<Expression/*!*/>/*!*/ decreases, ref Attributes decAttrs, ref Attributes mo
 		
 		IdentTypeOptional(out bv);
 		bvars.Add(bv); 
-		if (la.kind == 29) {
+		if (la.kind == 33) {
 			Get();
-			Expression(out range, true);
+			Expression(out range, true, true);
 		}
 		QSep();
-		Expression(out body, allowSemi);
+		Expression(out body, allowSemi, true);
 		e = new MapComprehension(mapToken, bvars, range ?? new LiteralExpr(mapToken, true), body);
 		
 	}
 
-	void ConstAtomExpression(out Expression e) {
+	void ConstAtomExpression(out Expression e, bool allowSemi, bool allowLambda) {
 		Contract.Ensures(Contract.ValueAtReturn(out e) != null);
 		IToken/*!*/ x;  BigInteger n;   Basetypes.BigDec d;
 		e = dummyExpr;  Type toType = null;
 		
 		switch (la.kind) {
-		case 113: {
+		case 114: {
 			Get();
 			e = new LiteralExpr(t, false); 
 			break;
 		}
-		case 114: {
+		case 115: {
 			Get();
 			e = new LiteralExpr(t, true); 
 			break;
 		}
-		case 115: {
+		case 116: {
 			Get();
 			e = new LiteralExpr(t); 
 			break;
@@ -3359,56 +3450,56 @@ List<Expression/*!*/>/*!*/ decreases, ref Attributes decAttrs, ref Attributes mo
 			e = new LiteralExpr(t, d); 
 			break;
 		}
-		case 116: {
-			Get();
-			e = new ThisExpr(t); 
-			break;
-		}
 		case 117: {
 			Get();
-			x = t; 
-			Expect(11);
-			Expression(out e, true);
-			Expect(12);
-			e = new UnaryOpExpr(x, UnaryOpExpr.Opcode.Fresh, e); 
+			e = new ThisExpr(t); 
 			break;
 		}
 		case 118: {
 			Get();
 			x = t; 
-			Expect(11);
-			Expression(out e, true);
-			Expect(12);
+			Expect(15);
+			Expression(out e, true, true);
+			Expect(16);
+			e = new UnaryOpExpr(x, UnaryOpExpr.Opcode.Fresh, e); 
+			break;
+		}
+		case 119: {
+			Get();
+			x = t; 
+			Expect(15);
+			Expression(out e, true, true);
+			Expect(16);
 			e = new OldExpr(x, e); 
 			break;
 		}
-		case 29: {
+		case 33: {
 			Get();
 			x = t; 
-			Expression(out e, true);
+			Expression(out e, true, true);
 			e = new UnaryOpExpr(x, UnaryOpExpr.Opcode.Cardinality, e); 
-			Expect(29);
+			Expect(33);
 			break;
 		}
-		case 54: case 55: {
-			if (la.kind == 54) {
+		case 56: case 57: {
+			if (la.kind == 56) {
 				Get();
 				x = t; toType = new IntType(); 
 			} else {
 				Get();
 				x = t; toType = new RealType(); 
 			}
-			Expect(11);
-			Expression(out e, true);
-			Expect(12);
+			Expect(15);
+			Expression(out e, true, true);
+			Expect(16);
 			e = new ConversionExpr(x, e, toType); 
 			break;
 		}
-		case 11: {
-			ParensExpression(out e);
+		case 15: {
+			ParensExpression(out e, allowSemi, allowLambda);
 			break;
 		}
-		default: SynErr(222); break;
+		default: SynErr(223); break;
 		}
 	}
 
@@ -3433,7 +3524,7 @@ List<Expression/*!*/>/*!*/ decreases, ref Attributes decAttrs, ref Attributes mo
 			 n = BigInteger.Zero;
 			}
 			
-		} else SynErr(223);
+		} else SynErr(224);
 	}
 
 	void Dec(out Basetypes.BigDec d) {
@@ -3448,90 +3539,160 @@ List<Expression/*!*/>/*!*/ decreases, ref Attributes decAttrs, ref Attributes mo
 		
 	}
 
-	void ParensExpression(out Expression e) {
+	void ParensExpression(out Expression e, bool allowSemi, bool allowLambda) {
 		IToken x;
-		List<Expression> args = null;
+		Expression ee;
+		e = null;
+		List<Expression> args = new List<Expression>();
+		List<Type> types = new List<Type>();
+		Type tt;
+		bool isLambda = false;
 		
-		Expect(11);
-		x = t; e = null; 
-		if (la.kind == 12) {
-			Get();
-			var tmp = theBuiltIns.TupleType(x, 0, true);
-			e = new DatatypeValue(x, BuiltIns.TupleTypeName(0), BuiltIns.TupleTypeCtorName, new List<Expression>());
-			
-		} else if (StartOf(17)) {
-			Expression(out e, true);
-			while (la.kind == 31) {
+		Expect(15);
+		x = t; 
+		if (StartOf(17)) {
+			OptTypedExpr(out ee, out tt, true);
+			args.Add(ee); types.Add(tt); 
+			while (la.kind == 35) {
 				Get();
-				if (args == null) {
-				 args = new List<Expression>();
-				 args.Add(e);  // add the first argument, which was parsed above
-				}
-				
-				Expression(out e, true);
-				args.Add(e); 
+				OptTypedExpr(out ee, out tt, true);
+				args.Add(ee); types.Add(tt); 
 			}
-			Expect(12);
-			if (args == null) {
-			 e = new ParensExpression(x, e);
-			} else {
-			 // make sure the corresponding tuple type exists
-			 var tmp = theBuiltIns.TupleType(x, args.Count, true);
-			 e = new DatatypeValue(x, BuiltIns.TupleTypeName(args.Count), BuiltIns.TupleTypeCtorName, args);
-			}
+		}
+		Expect(16);
+		if (IsLambda(allowLambda)) {
+			Expression body = null;
+			Expression req = null;
+			bool oneShot;
+			var reads = new List<FrameExpression>();
+			x = t;
 			
-		} else SynErr(224);
+			LambdaSpec(out req, reads);
+			LambdaArrow(out oneShot);
+			Expression(out body, allowSemi, true);
+			List<BoundVar> bvs = new List<BoundVar>();
+			for (int i = 0; i < args.Count; i++) {
+			 ee = args[i];
+			 tt = types[i];
+			 if (ee is IdentifierSequence) {
+			   IdentifierSequence ise = (IdentifierSequence)ee;
+			   List<IToken> idents = ise.Tokens;
+			   Contract.Assert(idents != null);
+			   Contract.Assert(idents.Count > 0);
+			   IToken id = idents[0];
+			   if (idents.Count != 1) {
+			     SemErr(id, "Expected variable binding.");
+			   }
+			   if (ise.Arguments != null) {
+			     SemErr(ise.OpenParen, "Expected variable binding.");
+			   }
+			   bvs.Add(new BoundVar(id, id.val, tt ?? new InferredTypeProxy()));
+			 } else {
+			   SemErr(ee.tok, "Expected variable binding.");
+			 }
+			}
+			e = new LambdaExpr(x, oneShot, bvs, req, reads, body);
+			isLambda = true;
+			
+		}
+		if (!isLambda) {
+		 for (int i = 0; i < args.Count; i++) {
+		   if (types[i] != null) {
+		     SemErr(args[i].tok, "Type specification not allowed here, comma separator was expected.");
+		   }
+		 }
+		 if (args.Count == 1) {
+		   e = new ParensExpression(x, args[0]);
+		 } else {
+		   // make sure the corresponding tuple type exists
+		   var tmp = theBuiltIns.TupleType(x, args.Count, true);
+		   e = new DatatypeValue(x, BuiltIns.TupleTypeName(args.Count), BuiltIns.TupleTypeCtorName, args);
+		 }
+		}
+		
+		if (!isLambda && args.Count == 1 && la.kind == _openparen) {
+			IToken openParen; 
+			while (la.kind == 15) {
+				Get();
+				openParen = t; args = new List<Expression>(); 
+				if (StartOf(17)) {
+					Expressions(args);
+				}
+				Expect(16);
+				e = new ApplyExpr(x, openParen, e, args); 
+			}
+		}
+	}
+
+	void LambdaArrow(out bool oneShot) {
+		oneShot = true; 
+		if (la.kind == 9) {
+			Get();
+			oneShot = false; 
+		} else if (la.kind == 10) {
+			Get();
+			oneShot = true; 
+		} else SynErr(225);
+	}
+
+	void OptTypedExpr(out Expression e, out Type tt, bool allowSemi) {
+		tt = null; 
+		Expression(out e, allowSemi, true);
+		if (la.kind == 7) {
+			Get();
+			Type(out tt);
+		}
 	}
 
 	void MapLiteralExpressions(out List<ExpressionPair> elements) {
 		Expression/*!*/ d, r;
 		elements = new List<ExpressionPair/*!*/>(); 
-		Expression(out d, true);
-		Expect(69);
-		Expression(out r, true);
+		Expression(out d, true, true);
+		Expect(71);
+		Expression(out r, true, true);
 		elements.Add(new ExpressionPair(d,r)); 
-		while (la.kind == 31) {
+		while (la.kind == 35) {
 			Get();
-			Expression(out d, true);
-			Expect(69);
-			Expression(out r, true);
+			Expression(out d, true, true);
+			Expect(71);
+			Expression(out r, true, true);
 			elements.Add(new ExpressionPair(d,r)); 
 		}
 	}
 
 	void QSep() {
-		if (la.kind == 124) {
+		if (la.kind == 125) {
 			Get();
-		} else if (la.kind == 125) {
+		} else if (la.kind == 126) {
 			Get();
-		} else SynErr(225);
+		} else SynErr(226);
 	}
 
-	void MatchExpression(out Expression e, bool allowSemi) {
+	void MatchExpression(out Expression e, bool allowSemi, bool allowLambda) {
 		Contract.Ensures(Contract.ValueAtReturn(out e) != null); IToken/*!*/ x;  MatchCaseExpr/*!*/ c;
 		List<MatchCaseExpr/*!*/> cases = new List<MatchCaseExpr/*!*/>();
 		bool usesOptionalBrace = false;
 		
-		Expect(82);
+		Expect(83);
 		x = t; 
-		Expression(out e, allowSemi);
-		if (la.kind == 9) {
+		Expression(out e, allowSemi, true);
+		if (la.kind == 13) {
 			Get();
 			usesOptionalBrace = true; 
 		}
-		while (la.kind == 78) {
-			CaseExpression(out c, allowSemi);
+		while (la.kind == 80) {
+			CaseExpression(out c, allowSemi, usesOptionalBrace || allowLambda);
 			cases.Add(c); 
 		}
 		if (CloseOptionalBrace(usesOptionalBrace)) {
-			Expect(10);
+			Expect(14);
 		} else if (StartOf(32)) {
 			if (usesOptionalBrace) { SemErr(t, "expecting close curly brace"); } 
-		} else SynErr(226);
+		} else SynErr(227);
 		e = new MatchExpr(x, e, cases, usesOptionalBrace); 
 	}
 
-	void QuantifierGuts(out Expression q, bool allowSemi) {
+	void QuantifierGuts(out Expression q, bool allowSemi, bool allowLambda) {
 		Contract.Ensures(Contract.ValueAtReturn(out q) != null); IToken/*!*/ x = Token.NoToken;
 		bool univ = false;
 		List<BoundVar/*!*/> bvars;
@@ -3539,16 +3700,16 @@ List<Expression/*!*/>/*!*/ decreases, ref Attributes decAttrs, ref Attributes mo
 		Expression range;
 		Expression/*!*/ body;
 		
-		if (la.kind == 85 || la.kind == 121) {
+		if (la.kind == 86 || la.kind == 122) {
 			Forall();
 			x = t;  univ = true; 
-		} else if (la.kind == 122 || la.kind == 123) {
+		} else if (la.kind == 123 || la.kind == 124) {
 			Exists();
 			x = t; 
-		} else SynErr(227);
+		} else SynErr(228);
 		QuantifierDomain(out bvars, out attrs, out range);
 		QSep();
-		Expression(out body, allowSemi);
+		Expression(out body, allowSemi, allowLambda);
 		if (univ) {
 		 q = new ForallExpr(x, bvars, range, body, attrs);
 		} else {
@@ -3557,7 +3718,7 @@ List<Expression/*!*/>/*!*/ decreases, ref Attributes decAttrs, ref Attributes mo
 		
 	}
 
-	void ComprehensionExpr(out Expression q, bool allowSemi) {
+	void ComprehensionExpr(out Expression q, bool allowSemi, bool allowLambda) {
 		Contract.Ensures(Contract.ValueAtReturn(out q) != null);
 		IToken x = Token.NoToken;
 		BoundVar bv;
@@ -3565,20 +3726,20 @@ List<Expression/*!*/>/*!*/ decreases, ref Attributes decAttrs, ref Attributes mo
 		Expression range;
 		Expression body = null;
 		
-		Expect(56);
+		Expect(58);
 		x = t; 
 		IdentTypeOptional(out bv);
 		bvars.Add(bv); 
-		while (la.kind == 31) {
+		while (la.kind == 35) {
 			Get();
 			IdentTypeOptional(out bv);
 			bvars.Add(bv); 
 		}
-		Expect(29);
-		Expression(out range, allowSemi);
-		if (la.kind == 124 || la.kind == 125) {
+		Expect(33);
+		Expression(out range, allowSemi, allowLambda);
+		if (la.kind == 125 || la.kind == 126) {
 			QSep();
-			Expression(out body, allowSemi);
+			Expression(out body, allowSemi, allowLambda);
 		}
 		if (body == null && bvars.Count != 1) { SemErr(t, "a set comprehension with more than one bound variable must have a term expression"); }
 		q = new SetComprehension(x, bvars, range, body);
@@ -3587,16 +3748,16 @@ List<Expression/*!*/>/*!*/ decreases, ref Attributes decAttrs, ref Attributes mo
 
 	void StmtInExpr(out Statement s) {
 		s = dummyStmt; 
-		if (la.kind == 83) {
+		if (la.kind == 84) {
 			AssertStmt(out s);
-		} else if (la.kind == 72) {
+		} else if (la.kind == 74) {
 			AssumeStmt(out s);
-		} else if (la.kind == 88) {
+		} else if (la.kind == 89) {
 			CalcStmt(out s);
-		} else SynErr(228);
+		} else SynErr(229);
 	}
 
-	void LetExpr(out Expression e, bool allowSemi) {
+	void LetExpr(out Expression e, bool allowSemi, bool allowLambda) {
 		IToken x = null;
 		bool isGhost = false;
 		var letLHSs = new List<CasePattern>();
@@ -3605,26 +3766,26 @@ List<Expression/*!*/>/*!*/ decreases, ref Attributes decAttrs, ref Attributes mo
 		bool exact = true;
 		e = dummyExpr;
 		
-		if (la.kind == 25) {
+		if (la.kind == 29) {
 			Get();
 			isGhost = true;  x = t; 
 		}
-		Expect(30);
+		Expect(34);
 		if (!isGhost) { x = t; } 
 		CasePattern(out pat);
 		if (isGhost) { pat.Vars.Iter(bv => bv.IsGhost = true); }
 		letLHSs.Add(pat);
 		
-		while (la.kind == 31) {
+		while (la.kind == 35) {
 			Get();
 			CasePattern(out pat);
 			if (isGhost) { pat.Vars.Iter(bv => bv.IsGhost = true); }
 			letLHSs.Add(pat);
 			
 		}
-		if (la.kind == 69) {
+		if (la.kind == 71) {
 			Get();
-		} else if (la.kind == 71) {
+		} else if (la.kind == 73) {
 			Get();
 			exact = false;
 			foreach (var lhs in letLHSs) {
@@ -3633,29 +3794,29 @@ List<Expression/*!*/>/*!*/ decreases, ref Attributes decAttrs, ref Attributes mo
 			 }
 			}
 			
-		} else SynErr(229);
-		Expression(out e, false);
+		} else SynErr(230);
+		Expression(out e, false, true);
 		letRHSs.Add(e); 
-		while (la.kind == 31) {
+		while (la.kind == 35) {
 			Get();
-			Expression(out e, false);
+			Expression(out e, false, true);
 			letRHSs.Add(e); 
 		}
 		Expect(8);
-		Expression(out e, allowSemi);
+		Expression(out e, allowSemi, allowLambda);
 		e = new LetExpr(x, letLHSs, letRHSs, e, exact); 
 	}
 
-	void NamedExpr(out Expression e, bool allowSemi) {
+	void NamedExpr(out Expression e, bool allowSemi, bool allowLambda) {
 		IToken/*!*/ x, d;
 		e = dummyExpr;
 		Expression expr;
 		
-		Expect(66);
+		Expect(68);
 		x = t; 
 		NoUSIdent(out d);
 		Expect(7);
-		Expression(out e, allowSemi);
+		Expression(out e, allowSemi, allowLambda);
 		expr = e;
 		e = new NamedExpr(x, d.val, expr); 
 	}
@@ -3667,65 +3828,65 @@ List<Expression/*!*/>/*!*/ decreases, ref Attributes decAttrs, ref Attributes mo
 		
 		if (IsIdentParen()) {
 			Ident(out id);
-			Expect(11);
+			Expect(15);
 			arguments = new List<CasePattern>(); 
 			if (la.kind == 1) {
 				CasePattern(out pat);
 				arguments.Add(pat); 
-				while (la.kind == 31) {
+				while (la.kind == 35) {
 					Get();
 					CasePattern(out pat);
 					arguments.Add(pat); 
 				}
 			}
-			Expect(12);
+			Expect(16);
 			pat = new CasePattern(id, id.val, arguments); 
 		} else if (la.kind == 1) {
 			IdentTypeOptional(out bv);
 			pat = new CasePattern(bv.tok, bv);
 			
-		} else SynErr(230);
+		} else SynErr(231);
 	}
 
-	void CaseExpression(out MatchCaseExpr c, bool allowSemi) {
+	void CaseExpression(out MatchCaseExpr c, bool allowSemi, bool allowLambda) {
 		Contract.Ensures(Contract.ValueAtReturn(out c) != null); IToken/*!*/ x, id;
 		List<BoundVar/*!*/> arguments = new List<BoundVar/*!*/>();
 		BoundVar/*!*/ bv;
 		Expression/*!*/ body;
 		
-		Expect(78);
+		Expect(80);
 		x = t; 
 		Ident(out id);
-		if (la.kind == 11) {
+		if (la.kind == 15) {
 			Get();
 			IdentTypeOptional(out bv);
 			arguments.Add(bv); 
-			while (la.kind == 31) {
+			while (la.kind == 35) {
 				Get();
 				IdentTypeOptional(out bv);
 				arguments.Add(bv); 
 			}
-			Expect(12);
+			Expect(16);
 		}
-		Expect(79);
-		Expression(out body, allowSemi);
+		Expect(9);
+		Expression(out body, allowSemi, allowLambda);
 		c = new MatchCaseExpr(x, id.val, arguments, body); 
 	}
 
 	void Forall() {
-		if (la.kind == 85) {
+		if (la.kind == 86) {
 			Get();
-		} else if (la.kind == 121) {
+		} else if (la.kind == 122) {
 			Get();
-		} else SynErr(231);
+		} else SynErr(232);
 	}
 
 	void Exists() {
-		if (la.kind == 122) {
+		if (la.kind == 123) {
 			Get();
-		} else if (la.kind == 123) {
+		} else if (la.kind == 124) {
 			Get();
-		} else SynErr(232);
+		} else SynErr(233);
 	}
 
 	void AttributeBody(ref Attributes attrs) {
@@ -3736,10 +3897,10 @@ List<Expression/*!*/>/*!*/ decreases, ref Attributes decAttrs, ref Attributes mo
 		Expect(7);
 		Expect(1);
 		aName = t.val; 
-		if (StartOf(34)) {
+		if (StartOf(33)) {
 			AttributeArg(out aArg, true);
 			aArgs.Add(aArg); 
-			while (la.kind == 31) {
+			while (la.kind == 35) {
 				Get();
 				AttributeArg(out aArg, true);
 				aArgs.Add(aArg); 
@@ -3761,41 +3922,40 @@ List<Expression/*!*/>/*!*/ decreases, ref Attributes decAttrs, ref Attributes mo
 	}
 
 	static readonly bool[,]/*!*/ set = {
-		{T,T,T,T, T,x,x,x, T,T,x,T, x,x,x,x, x,x,x,x, x,x,x,x, T,T,x,T, T,T,T,x, x,x,T,x, x,T,x,x, T,T,T,T, T,T,T,T, T,T,T,T, x,x,T,T, x,x,x,x, x,x,x,x, x,x,T,T, x,x,T,x, T,x,x,x, T,x,x,x, T,T,T,T, T,T,T,T, T,x,x,x, x,x,x,x, x,x,x,x, x,x,x,x, x,x,x,x, x,x,x,x, x,T,T,T, T,T,T,x, x,x,x,x, x,x,x,x},
-		{x,x,x,x, x,x,x,x, x,x,x,x, x,x,x,x, T,T,x,T, x,x,x,x, T,T,T,T, T,x,T,x, T,x,T,x, x,x,x,x, T,T,T,T, T,x,x,x, x,x,x,x, x,x,x,x, x,x,x,x, x,x,T,T, T,x,x,x, x,x,x,x, x,x,x,x, x,x,x,x, x,x,x,x, x,x,x,x, x,x,x,x, x,x,x,x, x,x,x,x, x,x,x,x, x,x,x,x, x,x,x,x, x,x,x,x, x,x,x,x, x,x,x,x, x,x,x,x},
-		{x,x,x,x, x,x,x,x, x,x,x,x, x,x,x,x, x,x,x,x, x,x,x,x, x,T,T,x, x,x,T,x, x,x,x,x, x,x,x,x, T,T,T,T, T,x,x,x, x,x,x,x, x,x,x,x, x,x,x,x, x,x,T,T, T,x,x,x, x,x,x,x, x,x,x,x, x,x,x,x, x,x,x,x, x,x,x,x, x,x,x,x, x,x,x,x, x,x,x,x, x,x,x,x, x,x,x,x, x,x,x,x, x,x,x,x, x,x,x,x, x,x,x,x, x,x,x,x},
-		{T,x,x,x, x,x,x,x, T,x,T,x, x,x,x,x, T,T,x,T, x,T,x,x, T,T,T,T, T,x,T,x, T,x,T,x, x,x,T,x, T,T,T,T, T,x,x,x, x,x,x,x, x,x,x,x, x,x,x,x, x,x,T,T, T,x,x,x, x,x,x,x, x,x,x,x, x,x,x,x, x,x,x,x, x,x,x,x, x,x,x,x, x,x,x,x, x,x,x,x, x,x,x,x, x,x,x,x, x,x,x,x, x,x,x,x, x,x,x,x, x,x,x,x, x,x,x,x},
-		{x,x,x,x, x,x,x,x, x,x,x,x, x,x,x,x, x,x,x,x, x,x,x,x, x,x,x,x, x,x,x,x, x,x,x,x, x,x,x,x, x,x,x,x, x,T,T,T, T,T,T,T, x,x,x,x, x,x,x,x, x,x,x,x, x,x,x,x, x,x,x,x, x,x,x,x, x,x,x,x, x,x,x,x, x,x,x,x, x,x,x,x, x,x,x,x, x,x,x,x, x,x,x,x, x,x,x,x, x,x,x,x, x,x,x,x, x,x,x,x, x,x,x,x, x,x,x,x},
-		{x,x,x,x, x,x,x,x, x,x,x,x, x,x,x,x, x,x,x,x, x,x,x,x, x,x,x,x, x,x,x,x, x,x,x,x, x,x,x,x, T,T,T,T, T,x,x,x, x,x,x,x, x,x,x,x, x,x,x,x, x,x,x,x, x,x,x,x, x,x,x,x, x,x,x,x, x,x,x,x, x,x,x,x, x,x,x,x, x,x,x,x, x,x,x,x, x,x,x,x, x,x,x,x, x,x,x,x, x,x,x,x, x,x,x,x, x,x,x,x, x,x,x,x, x,x,x,x},
-		{T,x,x,x, x,x,x,x, x,T,T,T, x,x,x,x, T,T,x,T, x,x,x,x, T,T,T,T, T,x,T,x, T,x,T,x, x,x,T,x, T,T,T,T, T,x,x,T, T,T,T,x, x,x,x,x, x,x,x,x, x,x,T,T, T,x,x,x, x,x,x,x, x,x,x,x, x,x,x,x, x,x,x,x, x,x,x,x, x,x,x,x, x,x,x,x, x,x,x,x, x,x,x,x, x,x,x,x, x,x,x,x, x,x,x,x, x,x,x,x, x,x,x,x, x,x,x,x},
-		{x,x,x,x, x,x,x,x, x,x,x,x, x,x,x,x, x,x,x,x, x,x,x,x, x,x,x,x, x,x,x,x, x,x,x,x, x,x,x,x, x,x,x,x, x,x,x,T, T,T,T,x, x,x,x,x, x,x,x,x, x,x,x,x, x,x,x,x, x,x,x,x, x,x,x,x, x,x,x,x, x,x,x,x, x,x,x,x, x,x,x,x, x,x,x,x, x,x,x,x, x,x,x,x, x,x,x,x, x,x,x,x, x,x,x,x, x,x,x,x, x,x,x,x, x,x,x,x},
-		{T,x,x,x, x,x,x,x, x,x,x,x, x,x,x,x, x,x,x,x, x,x,x,x, x,x,x,x, x,x,x,x, x,x,x,x, x,x,x,x, T,T,T,T, T,x,x,x, x,x,x,x, x,x,x,x, x,x,x,x, x,x,x,x, x,x,x,x, x,x,x,x, x,x,x,x, x,x,x,x, x,x,x,x, x,x,x,x, x,x,x,x, x,x,x,x, x,x,x,x, x,x,x,x, x,x,x,x, x,x,x,x, x,x,x,x, x,x,x,x, x,x,x,x, x,x,x,x},
-		{x,x,x,x, x,x,x,x, x,x,x,x, x,x,x,x, x,x,x,x, x,x,x,x, x,x,x,x, x,x,x,x, x,x,x,x, x,x,x,x, x,x,x,x, x,T,T,T, T,T,x,x, x,x,x,x, x,x,x,x, x,x,x,x, x,x,x,x, x,x,x,x, x,x,x,x, x,x,x,x, x,x,x,x, x,x,x,x, x,x,x,x, x,x,x,x, x,x,x,x, x,x,x,x, x,x,x,x, x,x,x,x, x,x,x,x, x,x,x,x, x,x,x,x, x,x,x,x},
-		{x,T,T,x, x,T,x,x, x,x,x,T, x,x,x,x, x,x,x,x, x,x,x,x, x,T,x,x, x,x,x,x, x,x,x,x, x,x,x,x, x,x,x,x, x,x,x,x, x,x,x,x, T,T,T,T, T,T,T,T, T,x,x,x, x,x,x,x, x,x,x,x, x,x,x,x, x,x,x,x, x,x,x,x, x,x,x,x, x,x,x,x, x,x,x,x, x,x,x,x, x,x,x,x, x,x,x,x, x,x,x,x, x,x,x,x, x,x,x,x, x,x,x,x, x,x,x,x},
-		{x,T,x,x, x,T,x,x, x,x,x,T, x,x,x,x, x,x,x,x, x,x,x,x, x,x,x,x, x,x,x,x, x,x,x,x, x,x,x,x, x,x,x,x, x,x,x,x, x,x,x,x, T,T,T,T, T,T,T,T, T,x,x,x, x,x,x,x, x,x,x,x, x,x,x,x, x,x,x,x, x,x,x,x, x,x,x,x, x,x,x,x, x,x,x,x, x,x,x,x, x,x,x,x, x,x,x,x, x,x,x,x, x,x,x,x, x,x,x,x, x,x,x,x, x,x,x,x},
-		{T,x,x,x, x,x,x,x, x,x,x,x, x,x,x,x, x,x,x,x, x,x,x,x, x,x,x,x, x,x,x,x, x,x,x,x, x,x,x,x, x,x,x,x, x,T,T,T, T,T,T,T, x,x,x,x, x,x,x,x, x,x,x,x, x,x,x,x, x,x,x,x, x,x,x,x, x,x,x,x, x,x,x,x, x,x,x,x, x,x,x,x, x,x,x,x, x,x,x,x, x,x,x,x, x,x,x,x, x,x,x,x, x,x,x,x, x,x,x,x, x,x,x,x, x,x,x,x},
-		{x,T,T,T, T,x,x,x, x,T,x,T, x,x,x,x, x,x,x,x, x,x,x,x, x,T,x,x, x,T,T,x, x,x,x,x, x,x,x,x, x,x,x,x, x,x,x,x, x,x,x,x, x,x,T,T, T,T,x,T, x,x,x,x, x,T,T,x, x,x,x,x, T,x,T,x, T,x,x,x, x,x,T,T, x,T,x,x, T,x,x,x, x,x,x,x, x,x,x,x, x,x,x,x, x,x,x,T, x,T,x,x, T,T,T,T, T,T,T,x, x,T,T,T, x,x,x,x},
-		{x,x,x,x, x,x,x,x, x,x,x,x, x,x,x,x, x,x,x,x, x,x,x,x, x,x,x,x, x,x,x,x, x,x,x,x, x,x,x,x, x,x,x,x, x,x,T,T, T,x,x,T, x,x,x,x, x,x,x,x, x,x,x,x, x,x,x,x, x,x,x,x, x,x,x,x, x,x,x,x, x,x,x,x, x,x,x,x, x,x,x,x, x,x,x,x, x,x,x,x, x,x,x,x, x,x,x,x, x,x,x,x, x,x,x,x, x,x,x,x, x,x,x,x, x,x,x,x},
-		{x,T,T,T, T,x,x,x, x,T,x,T, x,x,x,x, x,x,x,x, x,x,x,x, x,T,x,x, x,T,T,x, x,x,x,x, x,T,x,x, x,x,x,x, x,x,x,x, x,x,x,T, x,x,T,T, x,x,x,x, x,x,x,x, x,x,T,T, x,x,T,x, T,x,x,x, T,x,x,x, T,x,T,T, T,T,T,T, T,x,x,x, x,x,x,x, x,x,x,x, x,x,x,x, x,x,x,x, x,x,x,x, x,T,T,T, T,T,T,x, x,x,x,x, x,x,x,x},
-		{T,x,x,x, x,x,x,x, x,x,x,x, x,x,x,x, x,x,x,x, x,x,x,x, x,x,x,x, x,x,x,x, x,x,x,x, x,x,x,x, x,x,x,x, x,T,T,T, T,T,x,x, x,x,x,x, x,x,x,x, x,x,x,x, x,x,x,x, x,x,x,x, x,x,x,x, x,x,x,x, x,x,x,x, x,x,x,x, x,x,x,x, x,x,x,x, x,x,x,x, x,x,x,x, x,x,x,x, x,x,x,x, x,x,x,x, x,x,x,x, x,x,x,x, x,x,x,x},
-		{x,T,T,T, T,x,x,x, x,T,x,T, x,x,x,x, x,x,x,x, x,x,x,x, x,T,x,x, x,T,T,x, x,x,x,x, x,x,x,x, x,x,x,x, x,x,x,x, x,x,x,x, x,x,T,T, T,T,x,T, x,x,x,x, x,x,T,x, x,x,x,x, T,x,T,x, T,x,x,x, x,x,T,T, x,T,x,x, T,x,x,x, x,x,x,x, x,x,x,x, x,x,x,x, x,x,x,T, x,T,x,x, T,T,T,T, T,T,T,x, x,T,T,T, x,x,x,x},
-		{x,T,T,T, T,x,x,x, x,T,x,T, x,T,x,x, x,x,x,x, x,x,x,x, x,T,x,x, x,T,T,x, x,x,x,x, x,x,x,x, x,x,x,x, x,x,x,x, x,x,x,x, x,x,T,T, T,T,x,T, x,x,x,x, x,T,T,x, x,x,x,x, T,x,T,x, T,x,x,x, x,x,T,T, x,T,x,x, T,x,x,x, x,x,x,x, x,x,x,x, x,x,x,x, x,x,x,T, x,T,x,x, T,T,T,T, T,T,T,x, x,T,T,T, x,x,x,x},
-		{T,T,T,T, T,x,x,x, x,T,x,T, x,x,x,x, x,x,x,x, x,x,x,x, x,T,x,x, x,T,T,x, x,x,x,x, x,T,x,x, x,x,x,x, x,x,x,x, x,x,x,T, x,x,T,T, x,x,x,x, x,x,x,x, x,x,T,T, x,x,T,x, T,x,x,x, T,x,x,x, T,x,T,T, T,T,T,T, T,x,x,x, x,x,x,x, x,x,x,x, x,x,x,x, x,x,x,x, x,x,x,x, x,T,T,T, T,T,T,x, x,x,x,x, x,x,x,x},
-		{x,T,T,T, T,x,x,x, x,T,x,T, x,T,x,x, x,x,x,x, x,x,x,x, x,T,x,x, x,T,T,x, x,x,x,x, x,T,x,x, x,x,x,x, x,x,x,x, x,x,x,x, x,x,T,T, T,T,x,T, x,x,x,x, x,x,T,x, x,x,x,x, T,x,T,x, T,x,x,x, x,x,T,T, x,T,x,x, T,x,x,x, x,x,x,x, x,x,x,x, x,x,x,x, x,x,x,T, x,T,x,x, T,T,T,T, T,T,T,x, x,T,T,T, x,x,x,x},
-		{x,T,T,T, T,x,x,x, x,T,x,T, x,T,x,x, x,x,x,x, x,x,x,x, x,T,x,x, x,T,T,x, x,x,x,x, x,x,x,x, x,x,x,x, x,x,x,x, x,x,x,x, x,x,T,T, T,T,x,T, x,x,x,x, x,x,T,x, x,x,x,x, T,x,T,x, T,x,x,x, x,x,T,T, x,T,x,x, T,x,x,x, x,x,x,x, x,x,x,x, x,x,x,x, x,x,x,T, x,T,x,x, T,T,T,T, T,T,T,x, x,T,T,T, x,x,x,x},
-		{x,T,T,T, T,x,x,x, x,T,T,T, x,x,x,x, x,x,x,x, x,x,x,x, x,T,x,x, x,T,T,x, x,x,x,x, x,T,x,x, x,x,x,x, x,x,x,x, x,x,x,T, x,x,T,T, x,x,x,x, x,x,x,x, x,x,T,T, x,x,T,x, T,x,x,x, T,x,T,x, T,x,T,T, T,T,T,T, T,x,x,x, x,x,x,x, x,x,x,x, x,x,x,x, x,x,x,x, x,x,x,x, x,T,T,T, T,T,T,x, x,x,x,x, x,x,x,x},
-		{x,T,T,T, T,x,x,x, x,T,T,T, x,x,x,x, x,x,x,x, x,x,x,x, x,T,x,x, x,T,T,x, x,x,x,x, x,T,x,x, x,x,x,x, x,x,T,x, T,x,x,T, x,x,T,T, x,x,x,x, x,x,x,x, x,x,T,T, x,x,T,x, T,x,x,x, T,x,T,x, T,x,T,T, T,T,T,T, T,x,x,x, x,x,x,x, x,x,x,x, x,x,x,x, x,x,x,x, x,x,x,x, x,T,T,T, T,T,T,x, x,x,x,x, x,x,x,x},
-		{x,x,x,x, x,x,x,x, x,x,x,x, x,x,x,x, x,x,x,x, x,x,x,x, x,x,x,x, x,x,x,x, x,T,x,x, x,x,T,T, x,x,x,x, x,x,x,x, x,x,x,x, x,x,x,x, x,x,x,x, x,x,x,x, x,x,x,x, x,x,x,x, x,x,x,x, x,x,x,x, x,x,x,x, x,x,x,x, x,x,T,T, T,T,T,T, T,T,T,T, T,T,x,x, x,x,x,x, x,x,x,x, x,x,x,x, x,x,x,x, x,x,x,x, x,x,x,x},
-		{x,T,T,T, T,x,x,x, x,T,x,T, x,x,x,x, x,x,x,x, x,x,x,x, x,T,x,x, x,T,T,x, x,x,x,x, x,T,x,x, x,x,x,x, x,x,x,x, x,x,x,x, x,x,T,T, T,T,x,T, x,x,x,x, x,T,T,x, x,x,x,x, T,x,T,x, T,x,x,x, x,x,T,T, x,T,x,x, T,x,x,x, x,x,x,x, x,x,x,x, x,x,x,x, x,x,x,T, x,T,x,x, T,T,T,T, T,T,T,x, x,T,T,T, x,x,x,x},
-		{x,T,T,T, T,x,x,x, x,T,x,T, x,T,x,x, x,x,x,x, x,x,x,x, x,T,x,x, x,T,T,x, x,x,x,x, x,x,x,x, x,x,x,x, x,x,x,x, x,x,x,x, x,x,T,T, T,T,x,T, x,x,x,x, x,x,T,x, x,x,x,x, T,T,T,x, T,x,x,x, x,x,T,T, x,T,x,x, T,x,x,x, x,x,x,x, x,x,x,x, x,x,x,x, x,x,x,T, x,T,x,x, T,T,T,T, T,T,T,x, x,T,T,T, x,x,x,x},
-		{x,x,T,T, T,x,x,x, x,x,x,T, x,x,x,x, x,x,x,x, x,x,x,x, x,x,x,x, x,T,x,x, x,x,x,x, x,x,x,x, x,x,x,x, x,x,x,x, x,x,x,x, x,x,T,T, x,x,x,x, x,x,x,x, x,x,x,x, x,x,x,x, x,x,x,x, x,x,x,x, x,x,x,x, x,x,x,x, x,x,x,x, x,x,x,x, x,x,x,x, x,x,x,x, x,x,x,x, x,x,x,x, x,T,T,T, T,T,T,x, x,x,x,x, x,x,x,x},
-		{x,x,x,x, x,x,x,x, x,x,x,x, x,x,x,x, x,x,x,x, x,x,x,x, x,x,x,x, x,x,x,x, x,x,x,x, x,x,x,x, x,x,x,x, x,T,T,x, x,T,x,x, x,x,x,x, x,x,x,x, x,x,x,x, x,x,x,x, x,x,x,x, x,x,x,x, x,x,x,x, x,T,x,x, x,x,x,x, x,x,x,x, x,x,x,x, x,x,x,x, x,x,x,x, x,x,x,x, x,x,x,x, x,x,x,x, x,x,x,x, x,x,x,x, x,x,x,x},
-		{x,x,x,x, x,x,x,x, x,x,x,x, x,x,x,x, x,x,x,x, x,x,x,x, x,x,x,x, x,x,x,x, x,x,x,x, x,x,x,x, x,x,x,x, x,x,x,x, x,x,x,x, x,x,x,x, x,x,x,x, x,x,x,x, x,x,x,x, x,x,x,x, x,x,x,x, x,x,x,x, x,x,x,x, x,x,x,x, x,x,x,x, x,x,x,x, x,x,T,T, T,T,x,x, x,x,x,x, x,x,x,x, x,x,x,x, x,x,x,x, x,x,x,x, x,x,x,x},
-		{x,x,x,x, x,x,x,x, x,x,x,x, x,x,x,x, x,x,x,x, x,x,x,x, x,x,x,x, x,x,x,x, x,x,x,x, x,x,x,x, x,x,x,x, x,x,x,x, x,x,x,x, x,x,x,x, x,x,x,x, x,x,x,x, x,x,x,x, x,x,x,x, x,x,x,x, x,x,x,x, x,x,x,x, x,x,x,x, x,x,x,x, x,x,x,x, x,x,x,x, x,x,T,T, T,T,x,x, x,x,x,x, x,x,x,x, x,x,x,x, x,x,x,x, x,x,x,x},
-		{x,x,x,x, x,x,x,x, x,x,x,x, x,x,T,x, x,x,x,x, x,x,x,x, x,x,x,x, x,x,x,x, x,T,x,x, x,x,T,T, x,x,x,x, x,x,x,x, x,x,x,x, x,x,x,x, x,x,x,x, x,x,x,x, x,x,x,x, x,x,x,x, x,x,x,x, x,x,x,x, x,x,x,x, x,x,x,x, x,x,T,T, T,T,T,T, x,x,x,x, x,x,x,x, x,x,T,T, x,x,x,x, x,x,x,x, x,x,x,x, x,x,x,x, x,x,x,x},
-		{x,T,T,T, T,x,x,T, T,T,T,T, T,T,T,x, x,x,x,x, x,x,x,x, x,T,x,x, x,T,T,T, x,T,x,x, x,T,T,T, x,x,x,x, x,T,T,x, T,T,x,T, x,x,T,T, x,x,x,x, x,x,x,x, x,T,T,T, x,T,T,x, T,x,x,T, T,T,T,T, T,T,T,T, T,T,T,T, T,x,T,T, T,T,T,T, T,T,T,T, T,T,T,T, T,T,T,T, T,T,T,T, x,T,T,T, T,T,T,T, T,x,x,x, T,T,x,x},
-		{x,T,T,T, T,x,x,T, T,T,T,T, T,T,T,x, x,x,x,x, x,x,x,x, x,T,x,x, x,T,T,T, x,T,x,x, x,T,T,T, x,x,x,x, x,T,T,x, T,T,x,T, x,x,T,T, x,x,x,x, x,T,x,x, x,T,T,T, x,T,T,x, T,x,T,T, T,T,T,T, T,T,T,T, T,T,T,T, T,x,T,T, T,T,T,T, T,T,T,T, T,T,T,T, T,T,T,T, T,T,T,T, x,T,T,T, T,T,T,T, T,x,x,x, T,T,x,x},
-		{x,T,T,T, T,x,T,x, x,T,x,T, x,x,x,x, x,x,x,x, x,x,x,x, x,T,x,x, x,T,T,x, x,x,x,x, x,x,x,x, x,x,x,x, x,x,x,x, x,x,x,x, x,x,T,T, T,T,x,T, x,x,x,x, x,x,T,x, x,x,x,x, T,x,T,x, T,x,x,x, x,x,T,T, x,T,x,x, T,x,x,x, x,x,x,x, x,x,x,x, x,x,x,x, x,x,x,T, x,T,x,x, T,T,T,T, T,T,T,x, x,T,T,T, x,x,x,x}
+		{T,T,T,T, T,x,x,x, T,x,x,T, T,T,x,T, x,x,x,x, x,x,x,x, x,x,x,x, T,T,x,T, T,T,T,x, x,x,T,x, x,T,x,x, T,T,T,T, T,T,T,T, T,T,x,x, T,T,x,x, x,x,x,x, x,x,x,x, T,T,x,x, T,x,T,x, x,x,T,x, x,T,T,T, T,T,T,T, T,T,x,x, x,x,x,x, x,x,x,x, x,x,x,x, x,x,x,x, x,x,x,x, x,x,T,T, T,T,T,T, x,x,x,x, x,x,x,x, x},
+		{x,x,x,x, x,x,x,x, x,x,x,x, x,x,x,x, x,x,x,x, T,T,x,T, x,x,x,x, T,T,T,T, T,x,T,x, T,x,T,x, x,x,x,x, T,T,T,T, T,x,x,x, x,x,x,x, x,x,x,x, x,x,x,x, T,T,T,x, x,x,x,x, x,x,x,x, x,x,x,x, x,x,x,x, x,x,x,x, x,x,x,x, x,x,x,x, x,x,x,x, x,x,x,x, x,x,x,x, x,x,x,x, x,x,x,x, x,x,x,x, x,x,x,x, x,x,x,x, x},
+		{x,x,x,x, x,x,x,x, x,x,x,x, x,x,x,x, x,x,x,x, x,x,x,x, x,x,x,x, x,T,T,x, x,x,T,x, x,x,x,x, x,x,x,x, T,T,T,T, T,x,x,x, x,x,x,x, x,x,x,x, x,x,x,x, T,T,T,x, x,x,x,x, x,x,x,x, x,x,x,x, x,x,x,x, x,x,x,x, x,x,x,x, x,x,x,x, x,x,x,x, x,x,x,x, x,x,x,x, x,x,x,x, x,x,x,x, x,x,x,x, x,x,x,x, x,x,x,x, x},
+		{T,x,x,x, x,x,x,x, T,x,x,x, x,x,T,x, x,x,x,x, T,T,x,T, x,T,x,x, T,T,T,T, T,x,T,x, T,x,T,x, x,x,T,x, T,T,T,T, T,x,x,x, x,x,x,x, x,x,x,x, x,x,x,x, T,T,T,x, x,x,x,x, x,x,x,x, x,x,x,x, x,x,x,x, x,x,x,x, x,x,x,x, x,x,x,x, x,x,x,x, x,x,x,x, x,x,x,x, x,x,x,x, x,x,x,x, x,x,x,x, x,x,x,x, x,x,x,x, x},
+		{x,x,x,x, x,x,x,x, x,x,x,T, T,x,x,x, x,x,x,x, x,x,x,x, x,x,x,x, x,x,x,x, x,x,x,x, x,x,x,x, x,x,x,x, x,x,x,x, x,T,T,T, T,T,x,x, x,x,x,x, x,x,x,x, x,x,x,x, x,x,x,x, x,x,x,x, x,x,x,x, x,x,x,x, x,x,x,x, x,x,x,x, x,x,x,x, x,x,x,x, x,x,x,x, x,x,x,x, x,x,x,x, x,x,x,x, x,x,x,x, x,x,x,x, x,x,x,x, x},
+		{x,x,x,x, x,x,x,x, x,x,x,x, x,x,x,x, x,x,x,x, x,x,x,x, x,x,x,x, x,x,x,x, x,x,x,x, x,x,x,x, x,x,x,x, T,T,T,T, T,x,x,x, x,x,x,x, x,x,x,x, x,x,x,x, x,x,x,x, x,x,x,x, x,x,x,x, x,x,x,x, x,x,x,x, x,x,x,x, x,x,x,x, x,x,x,x, x,x,x,x, x,x,x,x, x,x,x,x, x,x,x,x, x,x,x,x, x,x,x,x, x,x,x,x, x,x,x,x, x},
+		{T,x,x,x, x,x,x,x, x,x,x,T, T,T,T,T, x,x,x,x, T,T,x,T, x,x,x,x, T,T,T,T, T,x,T,x, T,x,T,x, x,x,T,x, T,T,T,T, T,x,x,T, T,x,x,x, x,x,x,x, x,x,x,x, T,T,T,x, x,x,x,x, x,x,x,x, x,x,x,x, x,x,x,x, x,x,x,x, x,x,x,x, x,x,x,x, x,x,x,x, x,x,x,x, x,x,x,x, x,x,x,x, x,x,x,x, x,x,x,x, x,x,x,x, x,x,x,x, x},
+		{x,x,x,x, x,x,x,x, x,x,x,T, T,x,x,x, x,x,x,x, x,x,x,x, x,x,x,x, x,x,x,x, x,x,x,x, x,x,x,x, x,x,x,x, x,x,x,x, x,x,x,T, T,x,x,x, x,x,x,x, x,x,x,x, x,x,x,x, x,x,x,x, x,x,x,x, x,x,x,x, x,x,x,x, x,x,x,x, x,x,x,x, x,x,x,x, x,x,x,x, x,x,x,x, x,x,x,x, x,x,x,x, x,x,x,x, x,x,x,x, x,x,x,x, x,x,x,x, x},
+		{T,x,x,x, x,x,x,x, x,x,x,x, x,x,x,x, x,x,x,x, x,x,x,x, x,x,x,x, x,x,x,x, x,x,x,x, x,x,x,x, x,x,x,x, T,T,T,T, T,x,x,x, x,x,x,x, x,x,x,x, x,x,x,x, x,x,x,x, x,x,x,x, x,x,x,x, x,x,x,x, x,x,x,x, x,x,x,x, x,x,x,x, x,x,x,x, x,x,x,x, x,x,x,x, x,x,x,x, x,x,x,x, x,x,x,x, x,x,x,x, x,x,x,x, x,x,x,x, x},
+		{x,x,x,x, x,x,x,x, x,x,x,x, T,x,x,x, x,x,x,x, x,x,x,x, x,x,x,x, x,x,x,x, x,x,x,x, x,x,x,x, x,x,x,x, x,x,x,x, x,T,T,T, T,x,x,x, x,x,x,x, x,x,x,x, x,x,x,x, x,x,x,x, x,x,x,x, x,x,x,x, x,x,x,x, x,x,x,x, x,x,x,x, x,x,x,x, x,x,x,x, x,x,x,x, x,x,x,x, x,x,x,x, x,x,x,x, x,x,x,x, x,x,x,x, x,x,x,x, x},
+		{x,T,T,x, x,T,x,x, x,x,x,x, x,x,x,T, x,x,x,x, x,x,x,x, x,x,x,x, x,T,x,x, x,x,x,x, x,x,x,x, x,x,x,x, x,x,x,x, x,x,x,x, x,x,T,T, T,T,T,T, T,T,T,x, x,x,x,x, x,x,x,x, x,x,x,x, x,x,x,x, x,x,x,x, x,x,x,x, x,x,x,x, x,x,x,x, x,x,x,x, x,x,x,x, x,x,x,x, x,x,x,x, x,x,x,x, x,x,x,x, x,x,x,x, x,x,x,x, x},
+		{x,T,x,x, x,T,x,x, x,x,x,x, x,x,x,T, x,x,x,x, x,x,x,x, x,x,x,x, x,x,x,x, x,x,x,x, x,x,x,x, x,x,x,x, x,x,x,x, x,x,x,x, x,x,T,T, T,T,T,T, T,T,T,x, x,x,x,x, x,x,x,x, x,x,x,x, x,x,x,x, x,x,x,x, x,x,x,x, x,x,x,x, x,x,x,x, x,x,x,x, x,x,x,x, x,x,x,x, x,x,x,x, x,x,x,x, x,x,x,x, x,x,x,x, x,x,x,x, x},
+		{T,x,x,x, x,x,x,x, x,x,x,T, T,x,x,x, x,x,x,x, x,x,x,x, x,x,x,x, x,x,x,x, x,x,x,x, x,x,x,x, x,x,x,x, x,x,x,x, x,T,T,T, T,T,x,x, x,x,x,x, x,x,x,x, x,x,x,x, x,x,x,x, x,x,x,x, x,x,x,x, x,x,x,x, x,x,x,x, x,x,x,x, x,x,x,x, x,x,x,x, x,x,x,x, x,x,x,x, x,x,x,x, x,x,x,x, x,x,x,x, x,x,x,x, x,x,x,x, x},
+		{x,T,T,T, T,x,x,x, x,x,x,x, x,T,x,T, x,x,x,x, x,x,x,x, x,x,x,x, x,T,x,x, x,T,T,x, x,x,x,x, x,x,x,x, x,x,x,x, x,x,x,x, x,x,x,x, T,T,T,T, x,T,x,x, x,x,x,T, T,x,x,x, x,x,T,x, T,x,T,x, x,x,x,T, T,x,T,x, x,T,x,x, x,x,x,x, x,x,x,x, x,x,x,x, x,x,x,x, T,x,T,x, x,T,T,T, T,T,T,T, x,x,T,T, T,x,x,x, x},
+		{x,x,x,x, x,x,x,x, x,x,x,x, T,x,x,x, x,x,x,x, x,x,x,x, x,x,x,x, x,x,x,x, x,x,x,x, x,x,x,x, x,x,x,x, x,x,x,x, x,x,T,T, x,T,x,x, x,x,x,x, x,x,x,x, x,x,x,x, x,x,x,x, x,x,x,x, x,x,x,x, x,x,x,x, x,x,x,x, x,x,x,x, x,x,x,x, x,x,x,x, x,x,x,x, x,x,x,x, x,x,x,x, x,x,x,x, x,x,x,x, x,x,x,x, x,x,x,x, x},
+		{x,T,T,T, T,x,x,x, x,x,x,x, x,T,x,T, x,x,x,x, x,x,x,x, x,x,x,x, x,T,x,x, x,T,T,x, x,x,x,x, x,T,x,x, x,x,x,x, x,x,x,x, x,T,x,x, T,T,x,x, x,x,x,x, x,x,x,x, T,T,x,x, T,x,T,x, x,x,T,x, x,T,x,T, T,T,T,T, T,T,x,x, x,x,x,x, x,x,x,x, x,x,x,x, x,x,x,x, x,x,x,x, x,x,T,T, T,T,T,T, x,x,x,x, x,x,x,x, x},
+		{T,x,x,x, x,x,x,x, x,x,x,x, T,x,x,x, x,x,x,x, x,x,x,x, x,x,x,x, x,x,x,x, x,x,x,x, x,x,x,x, x,x,x,x, x,x,x,x, x,T,T,T, T,x,x,x, x,x,x,x, x,x,x,x, x,x,x,x, x,x,x,x, x,x,x,x, x,x,x,x, x,x,x,x, x,x,x,x, x,x,x,x, x,x,x,x, x,x,x,x, x,x,x,x, x,x,x,x, x,x,x,x, x,x,x,x, x,x,x,x, x,x,x,x, x,x,x,x, x},
+		{x,T,T,T, T,x,x,x, x,x,x,x, x,T,x,T, x,x,x,x, x,x,x,x, x,x,x,x, x,T,x,x, x,T,T,x, x,x,x,x, x,x,x,x, x,x,x,x, x,x,x,x, x,x,x,x, T,T,T,T, x,T,x,x, x,x,x,x, T,x,x,x, x,x,T,x, T,x,T,x, x,x,x,T, T,x,T,x, x,T,x,x, x,x,x,x, x,x,x,x, x,x,x,x, x,x,x,x, T,x,T,x, x,T,T,T, T,T,T,T, x,x,T,T, T,x,x,x, x},
+		{x,T,T,T, T,x,x,x, x,x,x,x, x,T,x,T, x,T,x,x, x,x,x,x, x,x,x,x, x,T,x,x, x,T,T,x, x,x,x,x, x,x,x,x, x,x,x,x, x,x,x,x, x,x,x,x, T,T,T,T, x,T,x,x, x,x,x,T, T,x,x,x, x,x,T,x, T,x,T,x, x,x,x,T, T,x,T,x, x,T,x,x, x,x,x,x, x,x,x,x, x,x,x,x, x,x,x,x, T,x,T,x, x,T,T,T, T,T,T,T, x,x,T,T, T,x,x,x, x},
+		{T,T,T,T, T,x,x,x, x,x,x,x, x,T,x,T, x,x,x,x, x,x,x,x, x,x,x,x, x,T,x,x, x,T,T,x, x,x,x,x, x,T,x,x, x,x,x,x, x,x,x,x, x,T,x,x, T,T,x,x, x,x,x,x, x,x,x,x, T,T,x,x, T,x,T,x, x,x,T,x, x,T,x,T, T,T,T,T, T,T,x,x, x,x,x,x, x,x,x,x, x,x,x,x, x,x,x,x, x,x,x,x, x,x,T,T, T,T,T,T, x,x,x,x, x,x,x,x, x},
+		{x,T,T,T, T,x,x,x, x,x,x,x, x,T,x,T, x,T,x,x, x,x,x,x, x,x,x,x, x,T,x,x, x,T,T,x, x,x,x,x, x,T,x,x, x,x,x,x, x,x,x,x, x,x,x,x, T,T,T,T, x,T,x,x, x,x,x,x, T,x,x,x, x,x,T,x, T,x,T,x, x,x,x,T, T,x,T,x, x,T,x,x, x,x,x,x, x,x,x,x, x,x,x,x, x,x,x,x, T,x,T,x, x,T,T,T, T,T,T,T, x,x,T,T, T,x,x,x, x},
+		{x,T,T,T, T,x,x,x, x,x,x,x, x,T,x,T, x,T,x,x, x,x,x,x, x,x,x,x, x,T,x,x, x,T,T,x, x,x,x,x, x,x,x,x, x,x,x,x, x,x,x,x, x,x,x,x, T,T,T,T, x,T,x,x, x,x,x,x, T,x,x,x, x,x,T,x, T,x,T,x, x,x,x,T, T,x,T,x, x,T,x,x, x,x,x,x, x,x,x,x, x,x,x,x, x,x,x,x, T,x,T,x, x,T,T,T, T,T,T,T, x,x,T,T, T,x,x,x, x},
+		{x,T,T,T, T,x,x,x, x,x,x,x, x,T,T,T, x,x,x,x, x,x,x,x, x,x,x,x, x,T,x,x, x,T,T,x, x,x,x,x, x,T,x,x, x,x,x,x, x,x,x,x, x,T,x,x, T,T,x,x, x,x,x,x, x,x,x,x, T,T,x,x, T,x,T,x, x,x,T,x, T,T,x,T, T,T,T,T, T,T,x,x, x,x,x,x, x,x,x,x, x,x,x,x, x,x,x,x, x,x,x,x, x,x,T,T, T,T,T,T, x,x,x,x, x,x,x,x, x},
+		{x,T,T,T, T,x,x,x, x,x,x,x, x,T,T,T, x,x,x,x, x,x,x,x, x,x,x,x, x,T,x,x, x,T,T,x, x,x,x,x, x,T,x,x, x,x,x,x, x,x,T,T, x,T,x,x, T,T,x,x, x,x,x,x, x,x,x,x, T,T,x,x, T,x,T,x, x,x,T,x, T,T,x,T, T,T,T,T, T,T,x,x, x,x,x,x, x,x,x,x, x,x,x,x, x,x,x,x, x,x,x,x, x,x,T,T, T,T,T,T, x,x,x,x, x,x,x,x, x},
+		{x,x,x,x, x,x,x,x, x,x,x,x, x,x,x,x, x,x,x,x, x,x,x,x, x,x,x,x, x,x,x,x, x,x,x,x, x,T,x,x, x,x,T,T, x,x,x,x, x,x,x,x, x,x,x,x, x,x,x,x, x,x,x,x, x,x,x,x, x,x,x,x, x,x,x,x, x,x,x,x, x,x,x,x, x,x,x,x, x,x,x,T, T,T,T,T, T,T,T,T, T,T,T,x, x,x,x,x, x,x,x,x, x,x,x,x, x,x,x,x, x,x,x,x, x,x,x,x, x},
+		{x,T,T,T, T,x,x,x, x,x,x,x, x,T,x,T, x,x,x,x, x,x,x,x, x,x,x,x, x,T,x,x, x,T,T,x, x,x,x,x, x,T,x,x, x,x,x,x, x,x,x,x, x,x,x,x, T,T,T,T, x,T,x,x, x,x,x,T, T,x,x,x, x,x,T,x, T,x,T,x, x,x,x,T, T,x,T,x, x,T,x,x, x,x,x,x, x,x,x,x, x,x,x,x, x,x,x,x, T,x,T,x, x,T,T,T, T,T,T,T, x,x,T,T, T,x,x,x, x},
+		{x,T,T,T, T,x,x,x, x,x,x,x, x,T,x,T, x,T,x,x, x,x,x,x, x,x,x,x, x,T,x,x, x,T,T,x, x,x,x,x, x,x,x,x, x,x,x,x, x,x,x,x, x,x,x,x, T,T,T,T, x,T,x,x, x,x,x,x, T,x,x,x, x,x,T,T, T,x,T,x, x,x,x,T, T,x,T,x, x,T,x,x, x,x,x,x, x,x,x,x, x,x,x,x, x,x,x,x, T,x,T,x, x,T,T,T, T,T,T,T, x,x,T,T, T,x,x,x, x},
+		{x,x,T,T, T,x,x,x, x,x,x,x, x,x,x,T, x,x,x,x, x,x,x,x, x,x,x,x, x,x,x,x, x,T,x,x, x,x,x,x, x,x,x,x, x,x,x,x, x,x,x,x, x,x,x,x, T,T,x,x, x,x,x,x, x,x,x,x, x,x,x,x, x,x,x,x, x,x,x,x, x,x,x,x, x,x,x,x, x,x,x,x, x,x,x,x, x,x,x,x, x,x,x,x, x,x,x,x, x,x,x,x, x,x,T,T, T,T,T,T, x,x,x,x, x,x,x,x, x},
+		{x,x,x,x, x,x,x,x, x,x,x,x, x,x,x,x, x,x,x,x, x,x,x,x, x,x,x,x, x,x,x,x, x,x,x,x, x,x,x,x, x,x,x,x, x,x,x,x, x,T,T,x, T,x,x,x, x,x,x,x, x,x,x,x, x,x,x,x, x,x,x,x, x,x,x,x, x,x,x,x, x,x,T,x, x,x,x,x, x,x,x,x, x,x,x,x, x,x,x,x, x,x,x,x, x,x,x,x, x,x,x,x, x,x,x,x, x,x,x,x, x,x,x,x, x,x,x,x, x},
+		{x,x,x,x, x,x,x,x, x,x,x,x, x,x,x,x, x,x,x,x, x,x,x,x, x,x,x,x, x,x,x,x, x,x,x,x, x,x,x,x, x,x,x,x, x,x,x,x, x,x,x,x, x,x,x,x, x,x,x,x, x,x,x,x, x,x,x,x, x,x,x,x, x,x,x,x, x,x,x,x, x,x,x,x, x,x,x,x, x,x,x,x, x,x,x,x, x,x,x,T, T,T,T,x, x,x,x,x, x,x,x,x, x,x,x,x, x,x,x,x, x,x,x,x, x,x,x,x, x},
+		{x,x,x,x, x,x,x,x, x,x,x,x, x,x,x,x, x,x,x,x, x,x,x,x, x,x,x,x, x,x,x,x, x,x,x,x, x,x,x,x, x,x,x,x, x,x,x,x, x,x,x,x, x,x,x,x, x,x,x,x, x,x,x,x, x,x,x,x, x,x,x,x, x,x,x,x, x,x,x,x, x,x,x,x, x,x,x,x, x,x,x,x, x,x,x,x, x,x,x,x, x,x,x,T, T,T,T,x, x,x,x,x, x,x,x,x, x,x,x,x, x,x,x,x, x,x,x,x, x},
+		{x,x,x,x, x,x,x,x, x,x,x,x, x,x,x,x, x,x,T,x, x,x,x,x, x,x,x,x, x,x,x,x, x,x,x,x, x,T,x,x, x,x,T,T, x,x,x,x, x,x,x,x, x,x,x,x, x,x,x,x, x,x,x,x, x,x,x,x, x,x,x,x, x,x,x,x, x,x,x,x, x,x,x,x, x,x,x,x, x,x,x,T, T,T,T,T, T,x,x,x, x,x,x,x, x,x,x,T, T,x,x,x, x,x,x,x, x,x,x,x, x,x,x,x, x,x,x,x, x},
+		{x,T,T,T, T,x,x,T, T,T,T,T, T,T,T,T, T,T,T,x, x,x,x,x, x,x,x,x, x,T,x,x, x,T,T,T, x,T,x,x, x,T,T,T, x,x,x,x, x,T,T,T, T,T,x,x, T,T,x,x, x,x,x,T, x,x,x,T, T,T,x,T, T,T,T,x, T,T,T,T, T,T,T,T, T,T,T,T, T,T,x,T, T,T,T,T, T,T,T,T, T,T,T,T, T,T,T,T, T,T,T,T, T,x,T,T, T,T,T,T, T,T,x,x, x,T,T,x, x},
+		{x,T,T,T, T,x,T,x, x,x,x,x, x,T,x,T, x,x,x,x, x,x,x,x, x,x,x,x, x,T,x,x, x,T,T,x, x,x,x,x, x,x,x,x, x,x,x,x, x,x,x,x, x,x,x,x, T,T,T,T, x,T,x,x, x,x,x,x, T,x,x,x, x,x,T,x, T,x,T,x, x,x,x,T, T,x,T,x, x,T,x,x, x,x,x,x, x,x,x,x, x,x,x,x, x,x,x,x, T,x,T,x, x,T,T,T, T,T,T,T, x,x,T,T, T,x,x,x, x}
 
 	};
 } // end Parser
@@ -3829,230 +3989,231 @@ public class Errors {
 			case 6: s = "string expected"; break;
 			case 7: s = "colon expected"; break;
 			case 8: s = "semi expected"; break;
-			case 9: s = "lbrace expected"; break;
-			case 10: s = "rbrace expected"; break;
-			case 11: s = "openparen expected"; break;
-			case 12: s = "closeparen expected"; break;
-			case 13: s = "star expected"; break;
-			case 14: s = "notIn expected"; break;
-			case 15: s = "\"include\" expected"; break;
-			case 16: s = "\"abstract\" expected"; break;
-			case 17: s = "\"module\" expected"; break;
-			case 18: s = "\"refines\" expected"; break;
-			case 19: s = "\"import\" expected"; break;
-			case 20: s = "\"opened\" expected"; break;
-			case 21: s = "\"=\" expected"; break;
-			case 22: s = "\"as\" expected"; break;
-			case 23: s = "\"default\" expected"; break;
-			case 24: s = "\"class\" expected"; break;
-			case 25: s = "\"ghost\" expected"; break;
-			case 26: s = "\"static\" expected"; break;
-			case 27: s = "\"datatype\" expected"; break;
-			case 28: s = "\"codatatype\" expected"; break;
-			case 29: s = "\"|\" expected"; break;
-			case 30: s = "\"var\" expected"; break;
-			case 31: s = "\",\" expected"; break;
-			case 32: s = "\"type\" expected"; break;
-			case 33: s = "\"==\" expected"; break;
-			case 34: s = "\"iterator\" expected"; break;
-			case 35: s = "\"yields\" expected"; break;
-			case 36: s = "\"returns\" expected"; break;
-			case 37: s = "\"...\" expected"; break;
-			case 38: s = "\"<\" expected"; break;
-			case 39: s = "\">\" expected"; break;
-			case 40: s = "\"method\" expected"; break;
-			case 41: s = "\"lemma\" expected"; break;
-			case 42: s = "\"colemma\" expected"; break;
-			case 43: s = "\"comethod\" expected"; break;
-			case 44: s = "\"constructor\" expected"; break;
-			case 45: s = "\"modifies\" expected"; break;
-			case 46: s = "\"free\" expected"; break;
-			case 47: s = "\"requires\" expected"; break;
-			case 48: s = "\"ensures\" expected"; break;
-			case 49: s = "\"decreases\" expected"; break;
-			case 50: s = "\"reads\" expected"; break;
-			case 51: s = "\"yield\" expected"; break;
-			case 52: s = "\"bool\" expected"; break;
-			case 53: s = "\"nat\" expected"; break;
-			case 54: s = "\"int\" expected"; break;
-			case 55: s = "\"real\" expected"; break;
-			case 56: s = "\"set\" expected"; break;
-			case 57: s = "\"multiset\" expected"; break;
-			case 58: s = "\"seq\" expected"; break;
-			case 59: s = "\"map\" expected"; break;
-			case 60: s = "\"object\" expected"; break;
-			case 61: s = "\".\" expected"; break;
-			case 62: s = "\"function\" expected"; break;
-			case 63: s = "\"predicate\" expected"; break;
-			case 64: s = "\"copredicate\" expected"; break;
-			case 65: s = "\"`\" expected"; break;
-			case 66: s = "\"label\" expected"; break;
-			case 67: s = "\"break\" expected"; break;
-			case 68: s = "\"where\" expected"; break;
-			case 69: s = "\":=\" expected"; break;
-			case 70: s = "\"return\" expected"; break;
-			case 71: s = "\":|\" expected"; break;
-			case 72: s = "\"assume\" expected"; break;
-			case 73: s = "\"new\" expected"; break;
-			case 74: s = "\"[\" expected"; break;
-			case 75: s = "\"]\" expected"; break;
-			case 76: s = "\"if\" expected"; break;
-			case 77: s = "\"else\" expected"; break;
-			case 78: s = "\"case\" expected"; break;
-			case 79: s = "\"=>\" expected"; break;
-			case 80: s = "\"while\" expected"; break;
-			case 81: s = "\"invariant\" expected"; break;
-			case 82: s = "\"match\" expected"; break;
-			case 83: s = "\"assert\" expected"; break;
-			case 84: s = "\"print\" expected"; break;
-			case 85: s = "\"forall\" expected"; break;
-			case 86: s = "\"parallel\" expected"; break;
-			case 87: s = "\"modify\" expected"; break;
-			case 88: s = "\"calc\" expected"; break;
-			case 89: s = "\"#\" expected"; break;
-			case 90: s = "\"<=\" expected"; break;
-			case 91: s = "\">=\" expected"; break;
-			case 92: s = "\"!=\" expected"; break;
-			case 93: s = "\"\\u2260\" expected"; break;
-			case 94: s = "\"\\u2264\" expected"; break;
-			case 95: s = "\"\\u2265\" expected"; break;
-			case 96: s = "\"<==>\" expected"; break;
-			case 97: s = "\"\\u21d4\" expected"; break;
-			case 98: s = "\"==>\" expected"; break;
-			case 99: s = "\"\\u21d2\" expected"; break;
-			case 100: s = "\"<==\" expected"; break;
-			case 101: s = "\"\\u21d0\" expected"; break;
-			case 102: s = "\"&&\" expected"; break;
-			case 103: s = "\"\\u2227\" expected"; break;
-			case 104: s = "\"||\" expected"; break;
-			case 105: s = "\"\\u2228\" expected"; break;
-			case 106: s = "\"in\" expected"; break;
-			case 107: s = "\"!\" expected"; break;
-			case 108: s = "\"+\" expected"; break;
-			case 109: s = "\"-\" expected"; break;
-			case 110: s = "\"/\" expected"; break;
-			case 111: s = "\"%\" expected"; break;
-			case 112: s = "\"\\u00ac\" expected"; break;
-			case 113: s = "\"false\" expected"; break;
-			case 114: s = "\"true\" expected"; break;
-			case 115: s = "\"null\" expected"; break;
-			case 116: s = "\"this\" expected"; break;
-			case 117: s = "\"fresh\" expected"; break;
-			case 118: s = "\"old\" expected"; break;
-			case 119: s = "\"then\" expected"; break;
-			case 120: s = "\"..\" expected"; break;
-			case 121: s = "\"\\u2200\" expected"; break;
-			case 122: s = "\"exists\" expected"; break;
-			case 123: s = "\"\\u2203\" expected"; break;
-			case 124: s = "\"::\" expected"; break;
-			case 125: s = "\"\\u2022\" expected"; break;
-			case 126: s = "??? expected"; break;
-			case 127: s = "this symbol not expected in SubModuleDecl"; break;
-			case 128: s = "invalid SubModuleDecl"; break;
-			case 129: s = "this symbol not expected in ClassDecl"; break;
-			case 130: s = "this symbol not expected in DatatypeDecl"; break;
-			case 131: s = "invalid DatatypeDecl"; break;
-			case 132: s = "this symbol not expected in DatatypeDecl"; break;
-			case 133: s = "invalid OtherTypeDecl"; break;
-			case 134: s = "this symbol not expected in OtherTypeDecl"; break;
-			case 135: s = "this symbol not expected in IteratorDecl"; break;
-			case 136: s = "invalid IteratorDecl"; break;
-			case 137: s = "invalid ClassMemberDecl"; break;
-			case 138: s = "invalid IdentOrDigitsSuffix"; break;
-			case 139: s = "this symbol not expected in FieldDecl"; break;
+			case 9: s = "darrow expected"; break;
+			case 10: s = "arrow expected"; break;
+			case 11: s = "reads expected"; break;
+			case 12: s = "requires expected"; break;
+			case 13: s = "lbrace expected"; break;
+			case 14: s = "rbrace expected"; break;
+			case 15: s = "openparen expected"; break;
+			case 16: s = "closeparen expected"; break;
+			case 17: s = "star expected"; break;
+			case 18: s = "notIn expected"; break;
+			case 19: s = "\"include\" expected"; break;
+			case 20: s = "\"abstract\" expected"; break;
+			case 21: s = "\"module\" expected"; break;
+			case 22: s = "\"refines\" expected"; break;
+			case 23: s = "\"import\" expected"; break;
+			case 24: s = "\"opened\" expected"; break;
+			case 25: s = "\"=\" expected"; break;
+			case 26: s = "\"as\" expected"; break;
+			case 27: s = "\"default\" expected"; break;
+			case 28: s = "\"class\" expected"; break;
+			case 29: s = "\"ghost\" expected"; break;
+			case 30: s = "\"static\" expected"; break;
+			case 31: s = "\"datatype\" expected"; break;
+			case 32: s = "\"codatatype\" expected"; break;
+			case 33: s = "\"|\" expected"; break;
+			case 34: s = "\"var\" expected"; break;
+			case 35: s = "\",\" expected"; break;
+			case 36: s = "\"type\" expected"; break;
+			case 37: s = "\"==\" expected"; break;
+			case 38: s = "\"iterator\" expected"; break;
+			case 39: s = "\"yields\" expected"; break;
+			case 40: s = "\"returns\" expected"; break;
+			case 41: s = "\"...\" expected"; break;
+			case 42: s = "\"<\" expected"; break;
+			case 43: s = "\">\" expected"; break;
+			case 44: s = "\"method\" expected"; break;
+			case 45: s = "\"lemma\" expected"; break;
+			case 46: s = "\"colemma\" expected"; break;
+			case 47: s = "\"comethod\" expected"; break;
+			case 48: s = "\"constructor\" expected"; break;
+			case 49: s = "\"modifies\" expected"; break;
+			case 50: s = "\"free\" expected"; break;
+			case 51: s = "\"ensures\" expected"; break;
+			case 52: s = "\"decreases\" expected"; break;
+			case 53: s = "\"yield\" expected"; break;
+			case 54: s = "\"bool\" expected"; break;
+			case 55: s = "\"nat\" expected"; break;
+			case 56: s = "\"int\" expected"; break;
+			case 57: s = "\"real\" expected"; break;
+			case 58: s = "\"set\" expected"; break;
+			case 59: s = "\"multiset\" expected"; break;
+			case 60: s = "\"seq\" expected"; break;
+			case 61: s = "\"map\" expected"; break;
+			case 62: s = "\"object\" expected"; break;
+			case 63: s = "\".\" expected"; break;
+			case 64: s = "\"function\" expected"; break;
+			case 65: s = "\"predicate\" expected"; break;
+			case 66: s = "\"copredicate\" expected"; break;
+			case 67: s = "\"`\" expected"; break;
+			case 68: s = "\"label\" expected"; break;
+			case 69: s = "\"break\" expected"; break;
+			case 70: s = "\"where\" expected"; break;
+			case 71: s = "\":=\" expected"; break;
+			case 72: s = "\"return\" expected"; break;
+			case 73: s = "\":|\" expected"; break;
+			case 74: s = "\"assume\" expected"; break;
+			case 75: s = "\"new\" expected"; break;
+			case 76: s = "\"[\" expected"; break;
+			case 77: s = "\"]\" expected"; break;
+			case 78: s = "\"if\" expected"; break;
+			case 79: s = "\"else\" expected"; break;
+			case 80: s = "\"case\" expected"; break;
+			case 81: s = "\"while\" expected"; break;
+			case 82: s = "\"invariant\" expected"; break;
+			case 83: s = "\"match\" expected"; break;
+			case 84: s = "\"assert\" expected"; break;
+			case 85: s = "\"print\" expected"; break;
+			case 86: s = "\"forall\" expected"; break;
+			case 87: s = "\"parallel\" expected"; break;
+			case 88: s = "\"modify\" expected"; break;
+			case 89: s = "\"calc\" expected"; break;
+			case 90: s = "\"#\" expected"; break;
+			case 91: s = "\"<=\" expected"; break;
+			case 92: s = "\">=\" expected"; break;
+			case 93: s = "\"!=\" expected"; break;
+			case 94: s = "\"\\u2260\" expected"; break;
+			case 95: s = "\"\\u2264\" expected"; break;
+			case 96: s = "\"\\u2265\" expected"; break;
+			case 97: s = "\"<==>\" expected"; break;
+			case 98: s = "\"\\u21d4\" expected"; break;
+			case 99: s = "\"==>\" expected"; break;
+			case 100: s = "\"\\u21d2\" expected"; break;
+			case 101: s = "\"<==\" expected"; break;
+			case 102: s = "\"\\u21d0\" expected"; break;
+			case 103: s = "\"&&\" expected"; break;
+			case 104: s = "\"\\u2227\" expected"; break;
+			case 105: s = "\"||\" expected"; break;
+			case 106: s = "\"\\u2228\" expected"; break;
+			case 107: s = "\"in\" expected"; break;
+			case 108: s = "\"!\" expected"; break;
+			case 109: s = "\"+\" expected"; break;
+			case 110: s = "\"-\" expected"; break;
+			case 111: s = "\"/\" expected"; break;
+			case 112: s = "\"%\" expected"; break;
+			case 113: s = "\"\\u00ac\" expected"; break;
+			case 114: s = "\"false\" expected"; break;
+			case 115: s = "\"true\" expected"; break;
+			case 116: s = "\"null\" expected"; break;
+			case 117: s = "\"this\" expected"; break;
+			case 118: s = "\"fresh\" expected"; break;
+			case 119: s = "\"old\" expected"; break;
+			case 120: s = "\"then\" expected"; break;
+			case 121: s = "\"..\" expected"; break;
+			case 122: s = "\"\\u2200\" expected"; break;
+			case 123: s = "\"exists\" expected"; break;
+			case 124: s = "\"\\u2203\" expected"; break;
+			case 125: s = "\"::\" expected"; break;
+			case 126: s = "\"\\u2022\" expected"; break;
+			case 127: s = "??? expected"; break;
+			case 128: s = "this symbol not expected in SubModuleDecl"; break;
+			case 129: s = "invalid SubModuleDecl"; break;
+			case 130: s = "this symbol not expected in ClassDecl"; break;
+			case 131: s = "this symbol not expected in DatatypeDecl"; break;
+			case 132: s = "invalid DatatypeDecl"; break;
+			case 133: s = "this symbol not expected in DatatypeDecl"; break;
+			case 134: s = "invalid OtherTypeDecl"; break;
+			case 135: s = "this symbol not expected in OtherTypeDecl"; break;
+			case 136: s = "this symbol not expected in IteratorDecl"; break;
+			case 137: s = "invalid IteratorDecl"; break;
+			case 138: s = "invalid ClassMemberDecl"; break;
+			case 139: s = "invalid IdentOrDigitsSuffix"; break;
 			case 140: s = "this symbol not expected in FieldDecl"; break;
-			case 141: s = "invalid FunctionDecl"; break;
+			case 141: s = "this symbol not expected in FieldDecl"; break;
 			case 142: s = "invalid FunctionDecl"; break;
 			case 143: s = "invalid FunctionDecl"; break;
 			case 144: s = "invalid FunctionDecl"; break;
-			case 145: s = "this symbol not expected in MethodDecl"; break;
-			case 146: s = "invalid MethodDecl"; break;
+			case 145: s = "invalid FunctionDecl"; break;
+			case 146: s = "this symbol not expected in MethodDecl"; break;
 			case 147: s = "invalid MethodDecl"; break;
-			case 148: s = "invalid FIdentType"; break;
-			case 149: s = "invalid TypeIdentOptional"; break;
-			case 150: s = "invalid TypeAndToken"; break;
-			case 151: s = "this symbol not expected in IteratorSpec"; break;
+			case 148: s = "invalid MethodDecl"; break;
+			case 149: s = "invalid FIdentType"; break;
+			case 150: s = "invalid TypeIdentOptional"; break;
+			case 151: s = "invalid TypeAndToken"; break;
 			case 152: s = "this symbol not expected in IteratorSpec"; break;
 			case 153: s = "this symbol not expected in IteratorSpec"; break;
 			case 154: s = "this symbol not expected in IteratorSpec"; break;
 			case 155: s = "this symbol not expected in IteratorSpec"; break;
-			case 156: s = "invalid IteratorSpec"; break;
-			case 157: s = "this symbol not expected in IteratorSpec"; break;
-			case 158: s = "invalid IteratorSpec"; break;
-			case 159: s = "this symbol not expected in MethodSpec"; break;
+			case 156: s = "this symbol not expected in IteratorSpec"; break;
+			case 157: s = "invalid IteratorSpec"; break;
+			case 158: s = "this symbol not expected in IteratorSpec"; break;
+			case 159: s = "invalid IteratorSpec"; break;
 			case 160: s = "this symbol not expected in MethodSpec"; break;
 			case 161: s = "this symbol not expected in MethodSpec"; break;
 			case 162: s = "this symbol not expected in MethodSpec"; break;
-			case 163: s = "invalid MethodSpec"; break;
-			case 164: s = "this symbol not expected in MethodSpec"; break;
-			case 165: s = "invalid MethodSpec"; break;
-			case 166: s = "invalid FrameExpression"; break;
-			case 167: s = "invalid ReferenceType"; break;
-			case 168: s = "this symbol not expected in FunctionSpec"; break;
+			case 163: s = "this symbol not expected in MethodSpec"; break;
+			case 164: s = "invalid MethodSpec"; break;
+			case 165: s = "this symbol not expected in MethodSpec"; break;
+			case 166: s = "invalid MethodSpec"; break;
+			case 167: s = "invalid FrameExpression"; break;
+			case 168: s = "invalid ReferenceType"; break;
 			case 169: s = "this symbol not expected in FunctionSpec"; break;
 			case 170: s = "this symbol not expected in FunctionSpec"; break;
 			case 171: s = "this symbol not expected in FunctionSpec"; break;
 			case 172: s = "this symbol not expected in FunctionSpec"; break;
-			case 173: s = "invalid FunctionSpec"; break;
-			case 174: s = "invalid PossiblyWildFrameExpression"; break;
-			case 175: s = "invalid PossiblyWildExpression"; break;
-			case 176: s = "this symbol not expected in OneStmt"; break;
-			case 177: s = "invalid OneStmt"; break;
-			case 178: s = "this symbol not expected in OneStmt"; break;
-			case 179: s = "invalid OneStmt"; break;
-			case 180: s = "invalid AssertStmt"; break;
-			case 181: s = "invalid AssumeStmt"; break;
-			case 182: s = "invalid UpdateStmt"; break;
+			case 173: s = "this symbol not expected in FunctionSpec"; break;
+			case 174: s = "invalid FunctionSpec"; break;
+			case 175: s = "invalid PossiblyWildFrameExpression"; break;
+			case 176: s = "invalid PossiblyWildExpression"; break;
+			case 177: s = "this symbol not expected in OneStmt"; break;
+			case 178: s = "invalid OneStmt"; break;
+			case 179: s = "this symbol not expected in OneStmt"; break;
+			case 180: s = "invalid OneStmt"; break;
+			case 181: s = "invalid AssertStmt"; break;
+			case 182: s = "invalid AssumeStmt"; break;
 			case 183: s = "invalid UpdateStmt"; break;
-			case 184: s = "invalid IfStmt"; break;
+			case 184: s = "invalid UpdateStmt"; break;
 			case 185: s = "invalid IfStmt"; break;
-			case 186: s = "invalid WhileStmt"; break;
+			case 186: s = "invalid IfStmt"; break;
 			case 187: s = "invalid WhileStmt"; break;
-			case 188: s = "invalid MatchStmt"; break;
-			case 189: s = "invalid ForallStmt"; break;
+			case 188: s = "invalid WhileStmt"; break;
+			case 189: s = "invalid MatchStmt"; break;
 			case 190: s = "invalid ForallStmt"; break;
-			case 191: s = "this symbol not expected in ModifyStmt"; break;
-			case 192: s = "invalid ModifyStmt"; break;
-			case 193: s = "invalid ReturnStmt"; break;
-			case 194: s = "invalid Rhs"; break;
-			case 195: s = "invalid Lhs"; break;
-			case 196: s = "invalid Guard"; break;
-			case 197: s = "this symbol not expected in LoopSpec"; break;
+			case 191: s = "invalid ForallStmt"; break;
+			case 192: s = "this symbol not expected in ModifyStmt"; break;
+			case 193: s = "invalid ModifyStmt"; break;
+			case 194: s = "invalid ReturnStmt"; break;
+			case 195: s = "invalid Rhs"; break;
+			case 196: s = "invalid Lhs"; break;
+			case 197: s = "invalid Guard"; break;
 			case 198: s = "this symbol not expected in LoopSpec"; break;
 			case 199: s = "this symbol not expected in LoopSpec"; break;
 			case 200: s = "this symbol not expected in LoopSpec"; break;
 			case 201: s = "this symbol not expected in LoopSpec"; break;
-			case 202: s = "this symbol not expected in Invariant"; break;
-			case 203: s = "invalid AttributeArg"; break;
-			case 204: s = "invalid CalcOp"; break;
-			case 205: s = "invalid EquivOp"; break;
-			case 206: s = "invalid ImpliesOp"; break;
-			case 207: s = "invalid ExpliesOp"; break;
-			case 208: s = "invalid AndOp"; break;
-			case 209: s = "invalid OrOp"; break;
-			case 210: s = "invalid RelOp"; break;
-			case 211: s = "invalid AddOp"; break;
-			case 212: s = "invalid UnaryExpression"; break;
+			case 202: s = "this symbol not expected in LoopSpec"; break;
+			case 203: s = "this symbol not expected in Invariant"; break;
+			case 204: s = "invalid AttributeArg"; break;
+			case 205: s = "invalid CalcOp"; break;
+			case 206: s = "invalid EquivOp"; break;
+			case 207: s = "invalid ImpliesOp"; break;
+			case 208: s = "invalid ExpliesOp"; break;
+			case 209: s = "invalid AndOp"; break;
+			case 210: s = "invalid OrOp"; break;
+			case 211: s = "invalid RelOp"; break;
+			case 212: s = "invalid AddOp"; break;
 			case 213: s = "invalid UnaryExpression"; break;
-			case 214: s = "invalid MulOp"; break;
-			case 215: s = "invalid NegOp"; break;
-			case 216: s = "invalid EndlessExpression"; break;
-			case 217: s = "invalid Suffix"; break;
+			case 214: s = "invalid UnaryExpression"; break;
+			case 215: s = "invalid MulOp"; break;
+			case 216: s = "invalid NegOp"; break;
+			case 217: s = "invalid EndlessExpression"; break;
 			case 218: s = "invalid Suffix"; break;
 			case 219: s = "invalid Suffix"; break;
-			case 220: s = "invalid DisplayExpr"; break;
-			case 221: s = "invalid MultiSetExpr"; break;
-			case 222: s = "invalid ConstAtomExpression"; break;
-			case 223: s = "invalid Nat"; break;
-			case 224: s = "invalid ParensExpression"; break;
-			case 225: s = "invalid QSep"; break;
-			case 226: s = "invalid MatchExpression"; break;
-			case 227: s = "invalid QuantifierGuts"; break;
-			case 228: s = "invalid StmtInExpr"; break;
-			case 229: s = "invalid LetExpr"; break;
-			case 230: s = "invalid CasePattern"; break;
-			case 231: s = "invalid Forall"; break;
-			case 232: s = "invalid Exists"; break;
+			case 220: s = "invalid Suffix"; break;
+			case 221: s = "invalid DisplayExpr"; break;
+			case 222: s = "invalid MultiSetExpr"; break;
+			case 223: s = "invalid ConstAtomExpression"; break;
+			case 224: s = "invalid Nat"; break;
+			case 225: s = "invalid LambdaArrow"; break;
+			case 226: s = "invalid QSep"; break;
+			case 227: s = "invalid MatchExpression"; break;
+			case 228: s = "invalid QuantifierGuts"; break;
+			case 229: s = "invalid StmtInExpr"; break;
+			case 230: s = "invalid LetExpr"; break;
+			case 231: s = "invalid CasePattern"; break;
+			case 232: s = "invalid Forall"; break;
+			case 233: s = "invalid Exists"; break;
 
 			default: s = "error " + n; break;
 		}
