Test/hofs/Consequence.dfy
@@ -1,0 +1,9 @@
+// RUN: %dafny /compile:0 "%s" > "%t"
+// RUN: %diff "%s.expect" "%t"
+
+method Check() {
+  var f : nat -> nat;
+  assume f.requires(0);
+  var i : nat := f(0);
+}
+
