Test/hofs/LambdaParsefail2.dfy
@@ -1,0 +1,8 @@
+// RUN: %dafny /compile:0 /print:"%t.print" "%s" > "%t"
+// RUN: %diff "%s.expect" "%t"
+
+
+method Fail2() {
+    var g4 := (x, y : A) => (y, x : B); // RHS should fail!
+}
+
