Test/hofs/MutableField.dfy
@@ -1,0 +1,15 @@
+// RUN: %dafny /compile:0 /print:"%t.print" "%s" > "%t"
+// RUN: %diff "%s.expect" "%t"
+
+
+class C {
+  function method f(x : int) : int { x }
+
+  var g : int -> int;
+
+  method M() modifies this;
+  {
+    f := g; // not ok
+  }
+}
+
