Test/hofs/Naked.dfy
@@ -1,0 +1,51 @@
+// RUN: %dafny /compile:0 "%s" > "%t"
+// RUN: %diff "%s.expect" "%t"
+
+module Functions {
+  function f(x: nat): nat
+  {
+    if x == 0 then 0 else
+    if var b: bool :| true; b then
+      var h := f;
+      h(x-1)
+    else
+      (f)(x-1)
+  }
+
+  function f1(x: nat): nat { if x == 0 then 0 else f2(x - 1) }
+
+  function f2(x: nat): nat { if x == 0 then 0 else (f1)(x - 1) }
+}
+
+module Requires {
+  function t(x: nat): nat
+  requires !t.requires(x);
+  { x }
+
+  function g(x: nat): nat
+  requires !(g).requires(x);
+  { x }
+
+  function g2(x: int): int { h(x) }
+
+  function h(x: int): int
+    requires !g2.requires(x);
+  { x }
+}
+
+module Reads {
+  function t(x: nat): nat
+  reads t.reads(x);
+  { x }
+
+  function g(x: nat): nat
+  reads (g).reads(x);
+  { x }
+
+  function g2(x: int): int { h(x) }
+
+  function h(x: int): int
+    reads g2.reads(x);
+  { x }
+}
+
