Test/hofs/ReadsReads.dfy
@@ -1,0 +1,59 @@
+// RUN: %dafny /compile:0 /print:"%t.print" /dprint:"%t.dprint" "%s" > "%t"
+// RUN: %diff "%s.expect" "%t"
+
+function MyReadsOk(f : A -> B, a : A) : set<object>
+  reads f.reads(a);
+{
+  f.reads(a)
+}
+
+function MyReadsOk2(f : A -> B, a : A) : set<object>
+  reads f.reads(a);
+{
+  (f.reads)(a)
+}
+
+function MyReadsOk3(f : A -> B, a : A) : set<object>
+  reads (f.reads)(a);
+{
+  f.reads(a)
+}
+
+function MyReadsOk4(f : A -> B, a : A) : set<object>
+  reads (f.reads)(a);
+{
+  (f.reads)(a)
+}
+
+function MyReadsBad(f : A -> B, a : A) : set<object>
+{
+  f.reads(a)
+}
+
+function MyReadsBad2(f : A -> B, a : A) : set<object>
+{
+  (f.reads)(a)
+}
+
+function MyReadsOk'(f : A -> B, a : A, o : object) : bool
+  reads f.reads(a);
+{
+  o in f.reads(a)
+}
+
+function MyReadsBad'(f : A -> B, a : A, o : object) : bool
+{
+  o in f.reads(a)
+}
+
+function MyRequiresOk(f : A -> B, a : A) : bool
+  reads f.reads(a);
+{
+  f.requires(a)
+}
+
+function MyRequiresBad(f : A -> B, a : A) : bool
+{
+  f.requires(a)
+}
+
